@prefix dct: <http://purl.org/dc/terms/> .
@prefix dpvo: <https://w3id.org/dpv/dpv-owl#> .
@prefix dpvo-risk: <https://w3id.org/dpv/dpv-owl/risk#> .
@prefix owl: <http://www.w3.org/2002/07/owl#> .
@prefix rdf: <http://www.w3.org/1999/02/22-rdf-syntax-ns#> .
@prefix rdfs: <http://www.w3.org/2000/01/rdf-schema#> .
@prefix sw: <http://www.w3.org/2003/06/sw-vocab-status/ns#> .
@prefix vann: <http://purl.org/vocab/vann/> .
@prefix xsd: <http://www.w3.org/2001/XMLSchema#> .

<https://w3id.org/dpv/dpv-owl/risk> a owl:Ontology ;
    dct:abstract "Risk Extension for DPV-OWL"@en ;
    dct:contributor "Beatriz Esteves",
        "Georg P Krog",
        "Harshvardhan J. Pandit",
        "Julian Flake",
        "Paul Ryan" ;
    dct:created "2022-08-14"^^xsd:date ;
    dct:creator "Harshvardhan J. Pandit" ;
    dct:description "The Risk extension to Data Privacy Vocabulary provides terms (classes and properties) related to risk management, assessment, and consequences."@en ;
    dct:license <https://www.w3.org/Consortium/Legal/2015/doc-license> ;
    dct:modified "2022-10-06"^^xsd:date ;
    dct:source <https://www.w3.org/community/dpvcg/> ;
    dct:title "Risk Extension for DPV-OWL"@en ;
    vann:preferredNamespacePrefix "dpvs-risk" ;
    vann:preferredNamespaceUri "https://w3id.org/dpv/dpv-owl/risk#"^^xsd:string ;
    owl:imports <https://w3id.org/dpv/dpv-owl> ;
    owl:versionInfo "0.8.2"^^xsd:string .

dpvo-risk:ACSC-ISM a owl:NamedIndividual,
        dpvo-risk:RiskManagementMethodology ;
    rdfs:label "ACSC-ISM"@en ;
    dct:created "2022-08-18"^^xsd:date ;
    dct:creator "Harshvardhan J. Pandit"^^xsd:string ;
    dct:description "The Australian Cyber Security Centre (ACSC) published the Australian Government Information Security Manual (ISM) which adopts the use of a risk management framework that draws from NIST 800-37, and includes six steps: define the system, select security controls, implement security controls, assess security controls, authorise the system and monitor the system"@en ;
    dct:source <https://www.enisa.europa.eu/publications/compendium-of-risk-management-frameworks> ;
    rdfs:isDefinedBy dpvo-risk: ;
    sw:term_status "accepted"@en .

dpvo-risk:ALARA a owl:NamedIndividual,
        dpvo-risk:QualitativeRiskAssessmentTechnique,
        dpvo-risk:QuantitativeRiskAssessmentTechnique ;
    rdfs:label "ALARA"@en ;
    dct:created "2022-08-18"^^xsd:date ;
    dct:creator "Harshvardhan J. Pandit"^^xsd:string ;
    dct:description "As Low as Resonably Achievable (ALARP) - A criteria for deciding significance of risk and means of evaluating tolerability of risk"@en ;
    dct:source <https://www.iso.org/standard/72140.html> ;
    rdfs:isDefinedBy dpvo-risk: ;
    sw:term_status "accepted"@en .

dpvo-risk:ALARP a owl:NamedIndividual,
        dpvo-risk:QualitativeRiskAssessmentTechnique,
        dpvo-risk:QuantitativeRiskAssessmentTechnique ;
    rdfs:label "ALARP"@en ;
    dct:created "2022-08-18"^^xsd:date ;
    dct:creator "Harshvardhan J. Pandit"^^xsd:string ;
    dct:description "As Low as Resonably Possible (ALARP) - A criteria for deciding significance of risk and means of evaluating tolerability of risk"@en ;
    dct:source <https://www.iso.org/standard/72140.html> ;
    rdfs:isDefinedBy dpvo-risk: ;
    sw:term_status "accepted"@en .

<https://w3id.org/dpv/dpv-owl/risk#ANSI-ISA-62443-3‑2-2020> a owl:NamedIndividual,
        dpvo-risk:RiskManagementMethodology ;
    rdfs:label "ANSI/ISA-62443-3‑2-2020"@en ;
    dct:created "2022-08-18"^^xsd:date ;
    dct:creator "Harshvardhan J. Pandit"^^xsd:string ;
    dct:description "ANSI/ISA-62443-3-2-2020 standard, entitled ‘Security for industrial automation and control systems, Part 3-2: Security risk assessment for system design’, from the International Society of Automation (ISA), dedicates an entire part to the assessment of security risk for system design targeting Security and IT professionals"@en ;
    dct:source <https://www.enisa.europa.eu/publications/compendium-of-risk-management-frameworks> ;
    rdfs:isDefinedBy dpvo-risk: ;
    sw:term_status "accepted"@en .

dpvo-risk:AbusiveContentUtilisation a owl:Class ;
    rdfs:label "Abusive Content Utilisation"@en ;
    dct:created "2022-08-17"^^xsd:date ;
    dct:creator "Harshvardhan J. Pandit"^^xsd:string ;
    dct:description ""@en ;
    dct:source <https://www.enisa.europa.eu/publications/reference-incident-classification-taxonomy/> ;
    rdfs:isDefinedBy dpvo-risk: ;
    rdfs:subClassOf dpvo:Harm ;
    sw:term_status "accepted"@en .

dpvo-risk:AttackonPrivateLife a owl:Class ;
    rdfs:label "Attack on Private Life"@en ;
    dct:created "2022-08-17"^^xsd:date ;
    dct:creator "Harshvardhan J. Pandit"^^xsd:string ;
    dct:description ""@en ;
    dct:source <https://www.iso.org/standard/75281.html> ;
    rdfs:isDefinedBy dpvo-risk: ;
    rdfs:subClassOf dpvo:Harm ;
    sw:term_status "accepted"@en .

dpvo-risk:AuthorisationFailure a owl:Class ;
    rdfs:label "Authorisation Failure"@en ;
    dct:created "2022-08-17"^^xsd:date ;
    dct:creator "Harshvardhan J. Pandit"^^xsd:string ;
    dct:description ""@en ;
    dct:source <https://www.enisa.europa.eu/publications/trust-services-security-incidents-2021> ;
    rdfs:isDefinedBy dpvo-risk: ;
    rdfs:subClassOf dpvo:Detriment ;
    sw:term_status "accepted"@en .

dpvo-risk:AvoidSource a owl:Class ;
    rdfs:label "Avoid Source"@en ;
    dct:created "2022-08-21"^^xsd:date ;
    dct:creator "Harshvardhan J. Pandit"^^xsd:string ;
    dct:description "Risk Control that avoids the risk source"@en ;
    rdfs:isDefinedBy dpvo-risk: ;
    rdfs:subClassOf dpvo-risk:ControlRiskSource ;
    sw:term_status "accepted"@en .

dpvo-risk:BSI-200-2 a owl:NamedIndividual,
        dpvo-risk:RiskManagementMethodology ;
    rdfs:label "BSI Standard 200-2"@en ;
    dct:created "2022-08-18"^^xsd:date ;
    dct:creator "Harshvardhan J. Pandit"^^xsd:string ;
    dct:description "The BSI-Standard 200-2 (‘IT-Grundschutz Methodology’) provides a methodology for the management of information security which can be adapted to the requirements of organisations of various types and sizes"@en ;
    dct:source <https://www.enisa.europa.eu/publications/compendium-of-risk-management-frameworks> ;
    rdfs:isDefinedBy dpvo-risk: ;
    sw:term_status "accepted"@en .

dpvo-risk:BayesianAnalysis a owl:NamedIndividual,
        dpvo-risk:QuantitativeRiskAssessmentTechnique ;
    rdfs:label "Bayesian Analysis"@en ;
    dct:created "2022-08-18"^^xsd:date ;
    dct:creator "Harshvardhan J. Pandit"^^xsd:string ;
    dct:description "A means of making inference about model parameters using Bayes' theorem which has the capability of incorporating empirical data into prior judgements about probabilities"@en ;
    dct:source <https://www.iso.org/standard/72140.html> ;
    rdfs:isDefinedBy dpvo-risk: ;
    sw:term_status "accepted"@en .

dpvo-risk:BayesianNetworks a owl:NamedIndividual,
        dpvo-risk:QuantitativeRiskAssessmentTechnique ;
    rdfs:label "Bayesian Networks"@en ;
    dct:created "2022-08-18"^^xsd:date ;
    dct:creator "Harshvardhan J. Pandit"^^xsd:string ;
    dct:description "A graphical model of variables and their cause-effect relationships expressed using probabilities"@en ;
    dct:source <https://www.iso.org/standard/72140.html> ;
    rdfs:isDefinedBy dpvo-risk: ;
    sw:term_status "accepted"@en .

dpvo-risk:Blackmail a owl:Class ;
    rdfs:label "Blackmail"@en ;
    dct:created "2022-08-17"^^xsd:date ;
    dct:creator "Harshvardhan J. Pandit"^^xsd:string ;
    dct:description ""@en ;
    dct:source <https://www.iso.org/standard/75281.html> ;
    rdfs:isDefinedBy dpvo-risk: ;
    rdfs:subClassOf dpvo:Harm ;
    sw:term_status "accepted"@en .

dpvo-risk:BowTie a owl:NamedIndividual,
        dpvo-risk:QualitativeRiskAssessmentTechnique,
        dpvo-risk:QuantitativeRiskAssessmentTechnique ;
    rdfs:label "Bow Tie Analysis"@en ;
    dct:created "2022-08-18"^^xsd:date ;
    dct:creator "Harshvardhan J. Pandit"^^xsd:string ;
    dct:description "A diagrammatic way of describing the pathways from sources of risk to outcomes, and of reviewing controls"@en ;
    dct:source <https://www.iso.org/standard/72140.html> ;
    rdfs:isDefinedBy dpvo-risk: ;
    sw:term_status "accepted"@en .

dpvo-risk:Brainstorming a owl:NamedIndividual,
        dpvo-risk:QualitativeRiskAssessmentTechnique ;
    rdfs:label "Brainstorming"@en ;
    dct:created "2022-08-18"^^xsd:date ;
    dct:creator "Harshvardhan J. Pandit"^^xsd:string ;
    dct:description "Technique used in workshops to encourage imaginative thinking"@en ;
    dct:source <https://www.iso.org/standard/72140.html> ;
    rdfs:isDefinedBy dpvo-risk: ;
    sw:term_status "accepted"@en .

dpvo-risk:BruteForceAuthorisations a owl:Class ;
    rdfs:label "Brute Force Authorisations"@en ;
    dct:created "2022-08-17"^^xsd:date ;
    dct:creator "Harshvardhan J. Pandit"^^xsd:string ;
    dct:description ""@en ;
    dct:source <https://www.enisa.europa.eu/publications/reference-incident-classification-taxonomy/> ;
    rdfs:isDefinedBy dpvo-risk: ;
    rdfs:subClassOf dpvo:Detriment ;
    sw:term_status "accepted"@en .

dpvo-risk:BusinessImpact a owl:Class ;
    rdfs:label "Business impact"@en ;
    dct:created "2022-08-17"^^xsd:date ;
    dct:creator "Harshvardhan J. Pandit"^^xsd:string ;
    dct:description ""@en ;
    dct:source <https://www.enisa.europa.eu/publications/methodology-for-a-sectoral-cybersecurity-assessment> ;
    rdfs:isDefinedBy dpvo-risk: ;
    rdfs:subClassOf dpvo:Impact ;
    sw:term_status "accepted"@en .

dpvo-risk:BusinessImpactAnalysis a owl:NamedIndividual,
        dpvo-risk:QualitativeRiskAssessmentTechnique,
        dpvo-risk:QuantitativeRiskAssessmentTechnique ;
    rdfs:label "Business Impact Analysis"@en ;
    dct:created "2022-08-18"^^xsd:date ;
    dct:creator "Harshvardhan J. Pandit"^^xsd:string ;
    dct:description "A process that analyses the consequences of a disruptive incident on the organization which determines the recovery priorities of an organization's products and services and, thereby, the priorities of the activities and resources which deliver them"@en ;
    dct:source <https://www.iso.org/standard/72140.html> ;
    rdfs:isDefinedBy dpvo-risk: ;
    sw:term_status "accepted"@en .

dpvo-risk:BusinessPerformanceImpairment a owl:Class ;
    rdfs:label "Business Performance Impairment"@en ;
    dct:created "2022-08-17"^^xsd:date ;
    dct:creator "Harshvardhan J. Pandit"^^xsd:string ;
    dct:description ""@en ;
    dct:source <https://www.iso.org/standard/75281.html> ;
    rdfs:isDefinedBy dpvo-risk: ;
    rdfs:subClassOf dpvo:Detriment ;
    sw:term_status "accepted"@en .

dpvo-risk:Businessdisruption a owl:Class ;
    rdfs:label "Business disruption"@en ;
    dct:created "2022-08-17"^^xsd:date ;
    dct:creator "Harshvardhan J. Pandit"^^xsd:string ;
    dct:description ""@en ;
    dct:source <https://www.iso.org/standard/75281.html> ;
    rdfs:isDefinedBy dpvo-risk: ;
    rdfs:subClassOf dpvo:Detriment ;
    sw:term_status "accepted"@en .

dpvo-risk:CCRACII a owl:NamedIndividual,
        dpvo-risk:RiskManagementMethodology ;
    rdfs:label "CCRACII"@en ;
    dct:created "2022-08-18"^^xsd:date ;
    dct:creator "Harshvardhan J. Pandit"^^xsd:string ;
    dct:description "The Guide to Conducting Cybersecurity Risk Assessment for Critical Information Infrastructure (CCRACII) defines commonly used terms such as threat event, vulnerability, likelihood, impact and risk, roles, and responsibilities, in addition to a range for risk levels, ranging from low to very high with different level of risk toleranc"@en ;
    dct:source <https://www.enisa.europa.eu/publications/compendium-of-risk-management-frameworks> ;
    rdfs:isDefinedBy dpvo-risk: ;
    sw:term_status "accepted"@en .

dpvo-risk:CORAS a owl:NamedIndividual,
        dpvo-risk:RiskManagementMethodology ;
    rdfs:label "CORAS"@en ;
    dct:created "2022-08-18"^^xsd:date ;
    dct:creator "Harshvardhan J. Pandit"^^xsd:string ;
    dct:description "The CORAS method was developed and is supported by SourceForge. It is a method for conducting the analysis and management of security risk. It provides a customised language for modelling threats and risks as well as detailed guidelines explaining how the language should be used to capture and model relevant information during the various stages of the security analysis"@en ;
    dct:source <https://www.enisa.europa.eu/publications/compendium-of-risk-management-frameworks> ;
    rdfs:isDefinedBy dpvo-risk: ;
    sw:term_status "accepted"@en .

dpvo-risk:CRAMM a owl:NamedIndividual,
        dpvo-risk:RiskManagementMethodology ;
    rdfs:label "CRAMM"@en ;
    dct:created "2022-08-18"^^xsd:date ;
    dct:creator "Harshvardhan J. Pandit"^^xsd:string ;
    dct:description "CCTA Risk Assessment and Management Methodology (CRAMM) is a method that an analyst or group of analysts may use to evaluate the security and risk level of an organisation by analysing and combining the diverse knowledge distributed in the local corporate environment"@en ;
    dct:source <https://www.enisa.europa.eu/publications/risk-management-standards> ;
    rdfs:isDefinedBy dpvo-risk: ;
    sw:term_status "accepted"@en .

dpvo-risk:CVaR a owl:NamedIndividual,
        dpvo-risk:QuantitativeRiskAssessmentTechnique ;
    rdfs:label "Conditional Value at Risk (CVaR)"@en ;
    dct:created "2022-08-18"^^xsd:date ;
    dct:creator "Harshvardhan J. Pandit"^^xsd:string ;
    dct:description "A measure of the expected loss from a financial portfolio in the worst a % of cases. Also called expected shortfall (ES)"@en ;
    dct:source <https://www.iso.org/standard/72140.html> ;
    rdfs:isDefinedBy dpvo-risk: ;
    sw:term_status "accepted"@en .

dpvo-risk:CausalMapping a owl:NamedIndividual,
        dpvo-risk:QualitativeRiskAssessmentTechnique ;
    rdfs:label "Causal Mapping"@en ;
    dct:created "2022-08-18"^^xsd:date ;
    dct:creator "Harshvardhan J. Pandit"^^xsd:string ;
    dct:description "A network diagram representing events, causes and effects and their relationships."@en ;
    dct:source <https://www.iso.org/standard/72140.html> ;
    rdfs:isDefinedBy dpvo-risk: ;
    sw:term_status "accepted"@en .

dpvo-risk:CauseConsequenceAnalysis a owl:NamedIndividual,
        dpvo-risk:QuantitativeRiskAssessmentTechnique ;
    rdfs:label "Cause-Consequence Analysis"@en ;
    dct:created "2022-08-18"^^xsd:date ;
    dct:creator "Harshvardhan J. Pandit"^^xsd:string ;
    dct:description "A combination of fault and event tree analysis that allows inclusion of time delays. Both causes and consequences of an initiating event are considered."@en ;
    dct:source <https://www.iso.org/standard/72140.html> ;
    rdfs:isDefinedBy dpvo-risk: ;
    sw:term_status "accepted"@en .

dpvo-risk:ChangeConsequence a owl:Class ;
    rdfs:label "Change Consequence"@en ;
    dct:created "2022-08-25"^^xsd:date ;
    dct:creator "Harshvardhan J. Pandit"^^xsd:string ;
    dct:description "Risk Control that changes Consequence"@en ;
    rdfs:isDefinedBy dpvo-risk: ;
    rdfs:subClassOf dpvo-risk:ControlConsequence ;
    sw:term_status "accepted"@en .

dpvo-risk:ChangeImpact a owl:Class ;
    rdfs:label "Change Impact"@en ;
    dct:created "2022-08-26"^^xsd:date ;
    dct:creator "Harshvardhan J. Pandit"^^xsd:string ;
    dct:description "Risk Control that changes Impact"@en ;
    rdfs:isDefinedBy dpvo-risk: ;
    rdfs:subClassOf dpvo-risk:ControlConsequence ;
    sw:term_status "accepted"@en .

dpvo-risk:Checklists a owl:NamedIndividual,
        dpvo-risk:QualitativeRiskAssessmentTechnique ;
    rdfs:label "Checklists"@en ;
    dct:created "2022-08-18"^^xsd:date ;
    dct:creator "Harshvardhan J. Pandit"^^xsd:string ;
    dct:description "A checklist based on experience or on concepts and models that can be used to help identify risks or controls."@en ;
    dct:source <https://www.iso.org/standard/72140.html> ;
    rdfs:isDefinedBy dpvo-risk: ;
    sw:term_status "accepted"@en .

dpvo-risk:ChildViolence a owl:Class ;
    rdfs:label "Child Violence"@en ;
    dct:created "2022-08-17"^^xsd:date ;
    dct:creator "Harshvardhan J. Pandit"^^xsd:string ;
    dct:description ""@en ;
    dct:source <https://www.enisa.europa.eu/publications/reference-incident-classification-taxonomy/> ;
    rdfs:isDefinedBy dpvo-risk: ;
    rdfs:subClassOf dpvo:Harm ;
    sw:term_status "accepted"@en .

dpvo-risk:Cindynic a owl:NamedIndividual,
        dpvo-risk:QualitativeRiskAssessmentTechnique ;
    rdfs:label "Cindynic Approach"@en ;
    dct:created "2022-08-18"^^xsd:date ;
    dct:creator "Harshvardhan J. Pandit"^^xsd:string ;
    dct:description "Considers goals, values, rules, data and models of stakeholders and identifies inconsistencies, ambiguities, omissions and ignorance. These form systemic sources and drivers of risk."@en ;
    dct:source <https://www.iso.org/standard/72140.html> ;
    rdfs:isDefinedBy dpvo-risk: ;
    sw:term_status "accepted"@en .

dpvo-risk:CitizensImpact a owl:Class ;
    rdfs:label "Citizens impact"@en ;
    dct:created "2022-08-17"^^xsd:date ;
    dct:creator "Harshvardhan J. Pandit"^^xsd:string ;
    dct:description ""@en ;
    dct:source <https://www.enisa.europa.eu/publications/methodology-for-a-sectoral-cybersecurity-assessment> ;
    rdfs:isDefinedBy dpvo-risk: ;
    rdfs:subClassOf dpvo:Impact ;
    sw:term_status "accepted"@en .

dpvo-risk:Classifications a owl:NamedIndividual,
        dpvo-risk:QualitativeRiskAssessmentTechnique ;
    rdfs:label "Classifications"@en ;
    dct:created "2022-08-18"^^xsd:date ;
    dct:creator "Harshvardhan J. Pandit"^^xsd:string ;
    dct:description "A classification list based on experience or on concepts and models that can be used to help identify risks or controls."@en ;
    dct:source <https://www.iso.org/standard/72140.html> ;
    rdfs:isDefinedBy dpvo-risk: ;
    sw:term_status "accepted"@en .

dpvo-risk:Coercion a owl:Class ;
    rdfs:label "Coercion"@en ;
    dct:created "2022-08-17"^^xsd:date ;
    dct:creator "Harshvardhan J. Pandit"^^xsd:string ;
    dct:description ""@en ;
    dct:source <https://www.enisa.europa.eu/topics/threat-risk-management/threats-and-trends/enisa-threat-landscape/threat-taxonomy/view> ;
    rdfs:isDefinedBy dpvo-risk: ;
    rdfs:subClassOf dpvo:Harm ;
    sw:term_status "accepted"@en .

dpvo-risk:ComplianceImpact a owl:Class ;
    rdfs:label "Compliance impact"@en ;
    dct:created "2022-08-17"^^xsd:date ;
    dct:creator "Harshvardhan J. Pandit"^^xsd:string ;
    dct:description ""@en ;
    dct:source <https://www.enisa.europa.eu/publications/methodology-for-a-sectoral-cybersecurity-assessment> ;
    rdfs:isDefinedBy dpvo-risk: ;
    rdfs:subClassOf dpvo:Impact ;
    sw:term_status "accepted"@en .

dpvo-risk:CompromiseAccount a owl:Class ;
    rdfs:label "Compromise Account"@en ;
    dct:created "2022-08-17"^^xsd:date ;
    dct:creator "Harshvardhan J. Pandit"^^xsd:string ;
    dct:description ""@en ;
    dct:source <https://www.enisa.europa.eu/publications/reference-incident-classification-taxonomy/> ;
    rdfs:isDefinedBy dpvo-risk: ;
    rdfs:subClassOf dpvo:Harm ;
    sw:term_status "accepted"@en .

dpvo-risk:CompromiseAccountCredentials a owl:Class ;
    rdfs:label "Compromise Account Credentials"@en ;
    dct:created "2022-08-17"^^xsd:date ;
    dct:creator "Harshvardhan J. Pandit"^^xsd:string ;
    dct:description ""@en ;
    dct:source <https://www.enisa.europa.eu/publications/reference-incident-classification-taxonomy/> ;
    rdfs:isDefinedBy dpvo-risk: ;
    rdfs:subClassOf dpvo:Harm ;
    sw:term_status "accepted"@en .

dpvo-risk:CompromiseAccountSecurity a owl:Class ;
    rdfs:label "Compromise Account Security"@en ;
    dct:created "2022-08-17"^^xsd:date ;
    dct:creator "Harshvardhan J. Pandit"^^xsd:string ;
    dct:description ""@en ;
    dct:source <https://www.enisa.europa.eu/publications/reference-incident-classification-taxonomy/> ;
    rdfs:isDefinedBy dpvo-risk: ;
    rdfs:subClassOf dpvo:NonMaterialDamage ;
    sw:term_status "accepted"@en .

dpvo-risk:ConfidentialityBreach a owl:Class ;
    rdfs:label "Confidentiality Breach"@en ;
    dct:created "2022-08-17"^^xsd:date ;
    dct:creator "Harshvardhan J. Pandit"^^xsd:string ;
    dct:description ""@en ;
    dct:source <https://www.iso.org/standard/75281.html> ;
    rdfs:isDefinedBy dpvo-risk: ;
    rdfs:subClassOf dpvo:Detriment ;
    sw:term_status "accepted"@en .

dpvo-risk:ConsequenceForDataSubject a owl:Class ;
    rdfs:label "Consequence for Data Subject"@en ;
    dct:created "2022-10-22"^^xsd:date ;
    dct:creator "Georg P Krog"^^xsd:string,
        "Harshvardhan J. Pandit"^^xsd:string ;
    dct:description ""@en ;
    rdfs:isDefinedBy dpvo-risk: ;
    rdfs:subClassOf dpvo:Consequence ;
    sw:term_status "accepted"@en .

dpvo-risk:ConsequenceOnDataSecurity a owl:Class ;
    rdfs:label "Consequence on Data Security"@en ;
    dct:created "2022-10-22"^^xsd:date ;
    dct:creator "Georg P Krog"^^xsd:string,
        "Harshvardhan J. Pandit"^^xsd:string ;
    dct:description ""@en ;
    rdfs:isDefinedBy dpvo-risk: ;
    rdfs:subClassOf dpvo:Consequence ;
    sw:term_status "accepted"@en .

dpvo-risk:CopyrightViolation a owl:Class ;
    rdfs:label "Copyright Violation"@en ;
    dct:created "2022-08-17"^^xsd:date ;
    dct:creator "Harshvardhan J. Pandit"^^xsd:string ;
    dct:description ""@en ;
    dct:source <https://www.enisa.europa.eu/publications/reference-incident-classification-taxonomy/> ;
    rdfs:isDefinedBy dpvo-risk: ;
    rdfs:subClassOf dpvo:NonMaterialDamage ;
    sw:term_status "accepted"@en .

dpvo-risk:CorruptionData a owl:Class ;
    rdfs:label "Corruption of Data"@en ;
    dct:created "2022-08-17"^^xsd:date ;
    dct:creator "Harshvardhan J. Pandit"^^xsd:string ;
    dct:description ""@en ;
    dct:source <https://www.iso.org/standard/75281.html> ;
    rdfs:isDefinedBy dpvo-risk: ;
    rdfs:subClassOf dpvo:Damage ;
    sw:term_status "accepted"@en .

dpvo-risk:CostAcquisition a owl:Class ;
    rdfs:label "Cost of Acquisition"@en ;
    dct:created "2022-08-17"^^xsd:date ;
    dct:creator "Harshvardhan J. Pandit"^^xsd:string ;
    dct:description ""@en ;
    dct:source <https://www.iso.org/standard/75281.html> ;
    rdfs:isDefinedBy dpvo-risk: ;
    rdfs:subClassOf dpvo:Detriment ;
    sw:term_status "accepted"@en .

dpvo-risk:CostBackup a owl:Class ;
    rdfs:label "Cost of Backup"@en ;
    dct:created "2022-08-17"^^xsd:date ;
    dct:creator "Harshvardhan J. Pandit"^^xsd:string ;
    dct:description ""@en ;
    dct:source <https://www.iso.org/standard/75281.html> ;
    rdfs:isDefinedBy dpvo-risk: ;
    rdfs:subClassOf dpvo:Detriment ;
    sw:term_status "accepted"@en .

dpvo-risk:CostBenefitAnalysis a owl:NamedIndividual,
        dpvo-risk:QuantitativeRiskAssessmentTechnique ;
    rdfs:label "Cost/benefit Analysis"@en ;
    dct:created "2022-08-18"^^xsd:date ;
    dct:creator "Harshvardhan J. Pandit"^^xsd:string ;
    dct:description "Uses money as a scale for estimating positive and negative, tangible and intangible, consequences of different options."@en ;
    dct:source <https://www.iso.org/standard/72140.html> ;
    rdfs:isDefinedBy dpvo-risk: ;
    sw:term_status "accepted"@en .

dpvo-risk:CostConfiguration a owl:Class ;
    rdfs:label "Cost of Configuration"@en ;
    dct:created "2022-08-17"^^xsd:date ;
    dct:creator "Harshvardhan J. Pandit"^^xsd:string ;
    dct:description ""@en ;
    dct:source <https://www.iso.org/standard/75281.html> ;
    rdfs:isDefinedBy dpvo-risk: ;
    rdfs:subClassOf dpvo:Detriment ;
    sw:term_status "accepted"@en .

dpvo-risk:CostInstallation a owl:Class ;
    rdfs:label "Cost of Installation"@en ;
    dct:created "2022-08-17"^^xsd:date ;
    dct:creator "Harshvardhan J. Pandit"^^xsd:string ;
    dct:description ""@en ;
    dct:source <https://www.iso.org/standard/75281.html> ;
    rdfs:isDefinedBy dpvo-risk: ;
    rdfs:subClassOf dpvo:Detriment ;
    sw:term_status "accepted"@en .

dpvo-risk:CostJudicialPenalties a owl:Class ;
    rdfs:label "Cost of Judicial Penalties"@en ;
    dct:created "2022-08-17"^^xsd:date ;
    dct:creator "Harshvardhan J. Pandit"^^xsd:string ;
    dct:description ""@en ;
    dct:source <https://www.iso.org/standard/75281.html> ;
    rdfs:isDefinedBy dpvo-risk: ;
    rdfs:subClassOf dpvo:Detriment ;
    sw:term_status "accepted"@en .

dpvo-risk:CostJudicialProceedings a owl:Class ;
    rdfs:label "Cost of Judicial Proceedings"@en ;
    dct:created "2022-08-17"^^xsd:date ;
    dct:creator "Harshvardhan J. Pandit"^^xsd:string ;
    dct:description ""@en ;
    dct:source <https://www.iso.org/standard/75281.html> ;
    rdfs:isDefinedBy dpvo-risk: ;
    rdfs:subClassOf dpvo:Detriment ;
    sw:term_status "accepted"@en .

dpvo-risk:CostOperationInterruption a owl:Class ;
    rdfs:label "Cost of Operation Interruption"@en ;
    dct:created "2022-08-17"^^xsd:date ;
    dct:creator "Harshvardhan J. Pandit"^^xsd:string ;
    dct:description ""@en ;
    dct:source <https://www.iso.org/standard/75281.html> ;
    rdfs:isDefinedBy dpvo-risk: ;
    rdfs:subClassOf dpvo:Detriment ;
    sw:term_status "accepted"@en .

dpvo-risk:CostSuspendedOperations a owl:Class ;
    rdfs:label "Cost of Suspended Operations"@en ;
    dct:created "2022-08-17"^^xsd:date ;
    dct:creator "Harshvardhan J. Pandit"^^xsd:string ;
    dct:description ""@en ;
    dct:source <https://www.iso.org/standard/75281.html> ;
    rdfs:isDefinedBy dpvo-risk: ;
    rdfs:subClassOf dpvo:Detriment ;
    sw:term_status "accepted"@en .

dpvo-risk:CrossImpactAnalysis a owl:NamedIndividual,
        dpvo-risk:QuantitativeRiskAssessmentTechnique ;
    rdfs:label "Cross Impact Analysis"@en ;
    dct:created "2022-08-18"^^xsd:date ;
    dct:creator "Harshvardhan J. Pandit"^^xsd:string ;
    dct:description "Evaluates changes in the probability of the occurrence of a given set of events consequent on the actual occurrence of one of them."@en ;
    dct:source <https://www.iso.org/standard/72140.html> ;
    rdfs:isDefinedBy dpvo-risk: ;
    sw:term_status "accepted"@en .

dpvo-risk:Cryptojacking a owl:Class ;
    rdfs:label "Cryptojacking"@en ;
    dct:created "2022-08-17"^^xsd:date ;
    dct:creator "Harshvardhan J. Pandit"^^xsd:string ;
    dct:description "Cryptojacking or hidden cryptomining is a type of cybercrime where a criminal secretly uses a victim’s computing power to generate cryptocurrency"@en ;
    dct:source <https://www.enisa.europa.eu/publications/enisa-threat-landscape-2021> ;
    rdfs:isDefinedBy dpvo-risk: ;
    rdfs:subClassOf dpvo:Detriment ;
    sw:term_status "accepted"@en .

dpvo-risk:CyberSpying a owl:Class ;
    rdfs:label "Cyber Spying"@en ;
    dct:created "2022-08-17"^^xsd:date ;
    dct:creator "Harshvardhan J. Pandit"^^xsd:string ;
    dct:description ""@en ;
    dct:source <https://www.iso.org/standard/75281.html> ;
    rdfs:isDefinedBy dpvo-risk: ;
    rdfs:subClassOf dpvo:NonMaterialDamage ;
    sw:term_status "accepted"@en .

dpvo-risk:CyberStalking a owl:Class ;
    rdfs:label "Cyber Stalking"@en ;
    dct:created "2022-08-17"^^xsd:date ;
    dct:creator "Harshvardhan J. Pandit"^^xsd:string ;
    dct:description ""@en ;
    dct:source <https://www.iso.org/standard/75281.html> ;
    rdfs:isDefinedBy dpvo-risk: ;
    rdfs:subClassOf dpvo:NonMaterialDamage ;
    sw:term_status "accepted"@en .

dpvo-risk:DPIA a owl:NamedIndividual,
        dpvo-risk:QualitativeRiskAssessmentTechnique ;
    rdfs:label "Data Protection Impact Assessment (DPIA)"@en ;
    dct:created "2022-08-18"^^xsd:date ;
    dct:creator "Harshvardhan J. Pandit"^^xsd:string ;
    dct:description "Analyses how incidents and events could affect the protection of data and its effects on persons and identifies and quantifies the capabilities that would be needed to manage it."@en ;
    dct:source <https://www.iso.org/standard/72140.html> ;
    rdfs:isDefinedBy dpvo-risk: ;
    sw:term_status "accepted"@en .

dpvo-risk:DamageByThirdParty a owl:Class ;
    rdfs:label "Damage by Third Party"@en ;
    dct:created "2022-08-17"^^xsd:date ;
    dct:creator "Harshvardhan J. Pandit"^^xsd:string ;
    dct:description ""@en ;
    dct:source <https://www.enisa.europa.eu/topics/threat-risk-management/threats-and-trends/enisa-threat-landscape/threat-taxonomy/view> ;
    rdfs:isDefinedBy dpvo-risk: ;
    rdfs:subClassOf dpvo:Damage ;
    sw:term_status "accepted"@en .

dpvo-risk:DangertoCustomers a owl:Class ;
    rdfs:label "Danger to Customers"@en ;
    dct:created "2022-08-17"^^xsd:date ;
    dct:creator "Harshvardhan J. Pandit"^^xsd:string ;
    dct:description ""@en ;
    dct:source <https://www.iso.org/standard/75281.html> ;
    rdfs:isDefinedBy dpvo-risk: ;
    rdfs:subClassOf dpvo:Harm ;
    sw:term_status "accepted"@en .

dpvo-risk:DangertoPersonnel a owl:Class ;
    rdfs:label "Danger to Personnel"@en ;
    dct:created "2022-08-17"^^xsd:date ;
    dct:creator "Harshvardhan J. Pandit"^^xsd:string ;
    dct:description ""@en ;
    dct:source <https://www.iso.org/standard/75281.html> ;
    rdfs:isDefinedBy dpvo-risk: ;
    rdfs:subClassOf dpvo:Harm ;
    sw:term_status "accepted"@en .

dpvo-risk:DataBreach a owl:Class ;
    rdfs:label "Data Breach"@en ;
    dct:created "2022-08-17"^^xsd:date ;
    dct:creator "Harshvardhan J. Pandit"^^xsd:string ;
    dct:description ""@en ;
    dct:source <https://www.iso.org/standard/75281.html> ;
    rdfs:isDefinedBy dpvo-risk: ;
    rdfs:subClassOf dpvo:Damage ;
    sw:term_status "accepted"@en .

dpvo-risk:DecisionTreeAnalysis a owl:NamedIndividual,
        dpvo-risk:QuantitativeRiskAssessmentTechnique ;
    rdfs:label "Decision Tree Analysis"@en ;
    dct:created "2022-08-18"^^xsd:date ;
    dct:creator "Harshvardhan J. Pandit"^^xsd:string ;
    dct:description "Uses a tree-like representation or model of decisions and their possible consequences. Outcomes are usually expressed in monetary terms or in terms of utility."@en ;
    dct:source <https://www.iso.org/standard/72140.html> ;
    rdfs:isDefinedBy dpvo-risk: ;
    sw:term_status "accepted"@en .

dpvo-risk:DelphiTechnique a owl:NamedIndividual,
        dpvo-risk:QualitativeRiskAssessmentTechnique ;
    rdfs:label "Delphi Technique"@en ;
    dct:created "2022-08-18"^^xsd:date ;
    dct:creator "Harshvardhan J. Pandit"^^xsd:string ;
    dct:description "Collects judgements through a set of sequential questionnaires. People participate individually but receive feedback on the responses of others after each set of questions."@en ;
    dct:source <https://www.iso.org/standard/72140.html> ;
    rdfs:isDefinedBy dpvo-risk: ;
    sw:term_status "accepted"@en .

dpvo-risk:DenialServiceAttack a owl:Class ;
    rdfs:label "Denial of Service Attack (DoS)"@en ;
    dct:created "2022-08-17"^^xsd:date ;
    dct:creator "Harshvardhan J. Pandit"^^xsd:string ;
    dct:description ""@en ;
    dct:source <https://www.iso.org/standard/75281.html> ;
    rdfs:isDefinedBy dpvo-risk: ;
    rdfs:subClassOf dpvo:Detriment ;
    sw:term_status "accepted"@en .

dpvo-risk:DetrimentToRecovery a owl:Class ;
    rdfs:label "Detriment to Recovery"@en ;
    dct:created "2022-08-17"^^xsd:date ;
    dct:creator "Harshvardhan J. Pandit"^^xsd:string ;
    dct:description ""@en ;
    dct:source <https://www.enisa.europa.eu/topics/threat-risk-management/threats-and-trends/enisa-threat-landscape/threat-taxonomy/view> ;
    rdfs:isDefinedBy dpvo-risk: ;
    rdfs:subClassOf dpvo:Detriment ;
    sw:term_status "accepted"@en .

dpvo-risk:Discrimination a owl:Class ;
    rdfs:label "Discrimination"@en ;
    dct:created "2022-08-19"^^xsd:date ;
    dct:creator "Georg P Krog"^^xsd:string ;
    dct:description ""@en ;
    rdfs:isDefinedBy dpvo-risk: ;
    rdfs:subClassOf dpvo:Harm ;
    sw:term_status "accepted"@en .

dpvo-risk:DistributedDenialServiceAttack a owl:Class ;
    rdfs:label "Distributed Denial of Service Attack (DDoS)"@en ;
    dct:created "2022-08-17"^^xsd:date ;
    dct:creator "Harshvardhan J. Pandit"^^xsd:string ;
    dct:description ""@en ;
    dct:source <https://www.iso.org/standard/75281.html> ;
    rdfs:isDefinedBy dpvo-risk: ;
    rdfs:subClassOf dpvo:Detriment ;
    sw:term_status "accepted"@en .

dpvo-risk:EBIOS a owl:NamedIndividual,
        dpvo-risk:RiskManagementMethodology ;
    rdfs:label "EBIOS"@en ;
    dct:created "2022-08-18"^^xsd:date ;
    dct:creator "Harshvardhan J. Pandit"^^xsd:string ;
    dct:description "Expression des Besoins et Identification des Objectifs de Sécurité (EBIOS) Risk Manager is an information security risk management method, created under the French General Secretariat of National Defence, consistent with ISO 31000 and ISO/IEC 27005, and enables the risk management requirements of ISO/IEC 27001 to be met"@en ;
    dct:source <https://www.enisa.europa.eu/publications/risk-management-standards> ;
    rdfs:isDefinedBy dpvo-risk: ;
    sw:term_status "accepted"@en .

dpvo-risk:ERM-IF a owl:NamedIndividual,
        dpvo-risk:RiskManagementMethodology ;
    rdfs:label "ERM-IF"@en ;
    dct:created "2022-08-18"^^xsd:date ;
    dct:creator "Harshvardhan J. Pandit"^^xsd:string ;
    dct:description "Enterprise Risk Management - Integrated Framework (ERM-IF) defines the essential components of enterprise risk management. It is based on a set of principles and concepts for the enterprise and has as its objective to offer a common language for enterprise risk"@en ;
    dct:source <https://www.enisa.europa.eu/publications/compendium-of-risk-management-frameworks> ;
    rdfs:isDefinedBy dpvo-risk: ;
    sw:term_status "accepted"@en .

dpvo-risk:ETSI-TS-102-165-1 a owl:NamedIndividual,
        dpvo-risk:RiskManagementMethodology ;
    rdfs:label "ETSI TS 102 165-1"@en ;
    dct:created "2022-08-18"^^xsd:date ;
    dct:creator "Harshvardhan J. Pandit"^^xsd:string ;
    dct:description "ETSI TS 102 165-1 offers methodology and pro-forma for threat, vulnerability and risk analysis (TVRA). According to ETSI TS 102 165-1, threat vulnerability and risk analysis (TVRA) is used to identify risk to an information system based upon the product of the likelihood of an attack and the impact that such an attack will have on the system"@en ;
    dct:source <https://www.enisa.europa.eu/publications/compendium-of-risk-management-frameworks> ;
    rdfs:isDefinedBy dpvo-risk: ;
    sw:term_status "accepted"@en .

dpvo-risk:EU-ITSRM a owl:NamedIndividual,
        dpvo-risk:RiskManagementMethodology ;
    rdfs:label "ITSRM²"@en ;
    dct:created "2022-08-18"^^xsd:date ;
    dct:creator "Harshvardhan J. Pandit"^^xsd:string ;
    dct:description "ITSRM² IT Security Risk Management Methodology is a methodology provided by DG DIGIT and the European Commission as part of a set of standards for information security"@en ;
    dct:source <https://www.enisa.europa.eu/publications/compendium-of-risk-management-frameworks> ;
    rdfs:isDefinedBy dpvo-risk: ;
    sw:term_status "accepted"@en .

dpvo-risk:Eavesdropping a owl:Class ;
    rdfs:label "Eavesdropping"@en ;
    dct:created "2022-08-17"^^xsd:date ;
    dct:creator "Harshvardhan J. Pandit"^^xsd:string ;
    dct:description ""@en ;
    dct:source <https://www.iso.org/standard/75281.html> ;
    rdfs:isDefinedBy dpvo-risk: ;
    rdfs:subClassOf dpvo:NonMaterialDamage ;
    sw:term_status "accepted"@en .

dpvo-risk:EconomicDisadvantage a owl:Class ;
    rdfs:label "Economic Disadvantage"@en ;
    dct:created "2022-08-19"^^xsd:date ;
    dct:creator "Georg P Krog"^^xsd:string ;
    dct:description ""@en ;
    rdfs:isDefinedBy dpvo-risk: ;
    rdfs:subClassOf dpvo:Impact ;
    sw:term_status "accepted"@en .

dpvo-risk:EnvironmentalSafetyEndangerment a owl:Class ;
    rdfs:label "Environmental Safety Endangerment"@en ;
    dct:created "2022-08-17"^^xsd:date ;
    dct:creator "Harshvardhan J. Pandit"^^xsd:string ;
    dct:description ""@en ;
    dct:source <https://www.iso.org/standard/75281.html> ;
    rdfs:isDefinedBy dpvo-risk: ;
    rdfs:subClassOf dpvo:Harm ;
    sw:term_status "accepted"@en .

dpvo-risk:EquipmentFailure a owl:Class ;
    rdfs:label "Equipment Failure"@en ;
    dct:created "2022-08-17"^^xsd:date ;
    dct:creator "Harshvardhan J. Pandit"^^xsd:string ;
    dct:description ""@en ;
    dct:source <https://www.iso.org/standard/75281.html> ;
    rdfs:isDefinedBy dpvo-risk: ;
    rdfs:subClassOf dpvo:Damage ;
    sw:term_status "accepted"@en .

dpvo-risk:EquipmentMalfunction a owl:Class ;
    rdfs:label "Equipment Malfunction"@en ;
    dct:created "2022-08-17"^^xsd:date ;
    dct:creator "Harshvardhan J. Pandit"^^xsd:string ;
    dct:description ""@en ;
    dct:source <https://www.iso.org/standard/75281.html> ;
    rdfs:isDefinedBy dpvo-risk: ;
    rdfs:subClassOf dpvo:Detriment ;
    sw:term_status "accepted"@en .

dpvo-risk:ErrornousSystemUse a owl:Class ;
    rdfs:label "Errornous System Use"@en ;
    dct:created "2022-08-17"^^xsd:date ;
    dct:creator "Harshvardhan J. Pandit"^^xsd:string ;
    dct:description ""@en ;
    dct:source <https://www.iso.org/standard/75281.html> ;
    rdfs:isDefinedBy dpvo-risk: ;
    rdfs:subClassOf dpvo:Detriment ;
    sw:term_status "accepted"@en .

dpvo-risk:EventTreeAnalysis a owl:NamedIndividual,
        dpvo-risk:QualitativeRiskAssessmentTechnique,
        dpvo-risk:QuantitativeRiskAssessmentTechnique ;
    rdfs:label "Event Tree Analysis"@en ;
    dct:created "2022-08-18"^^xsd:date ;
    dct:creator "Harshvardhan J. Pandit"^^xsd:string ;
    dct:description "Models the possible outcomes from a given initiating event and the status of controls thus analysing the frequency or probability of the various possible outcomes."@en ;
    dct:source <https://www.iso.org/standard/72140.html> ;
    rdfs:isDefinedBy dpvo-risk: ;
    sw:term_status "accepted"@en .

dpvo-risk:Extorsion a owl:Class ;
    rdfs:label "Extorsion"@en ;
    dct:created "2022-08-17"^^xsd:date ;
    dct:creator "Harshvardhan J. Pandit"^^xsd:string ;
    dct:description ""@en ;
    dct:source <https://www.enisa.europa.eu/topics/threat-risk-management/threats-and-trends/enisa-threat-landscape/threat-taxonomy/view> ;
    rdfs:isDefinedBy dpvo-risk: ;
    rdfs:subClassOf dpvo:Harm ;
    sw:term_status "accepted"@en .

dpvo-risk:FAIR a owl:NamedIndividual,
        dpvo-risk:RiskManagementMethodology ;
    rdfs:label "FAIR"@en ;
    dct:created "2022-08-18"^^xsd:date ;
    dct:creator "Harshvardhan J. Pandit"^^xsd:string ;
    dct:description "The purpose of the FAIR (Factor Analysis of Information Risk) model is to help organisations understand, analyse, and measure information risk. The model provides an approach to quantify risk and defines the necessary building blocks for implementing effective cyber risk management programmes"@en ;
    dct:source <https://www.enisa.europa.eu/publications/compendium-of-risk-management-frameworks> ;
    rdfs:isDefinedBy dpvo-risk: ;
    sw:term_status "accepted"@en .

dpvo-risk:FAIR-Privacy a owl:NamedIndividual,
        dpvo-risk:RiskManagementMethodology ;
    rdfs:label "FAIR Privacy"@en ;
    dct:created "2022-08-18"^^xsd:date ;
    dct:creator "Harshvardhan J. Pandit"^^xsd:string ;
    dct:description "Factors Analysis in Information Risk (FAIR Privacy) is a quantitative privacy risk framework based on FAIR (Factors Analysis in Information Risk) that examines personal privacy risks (to individuals), not organisational risks"@en ;
    dct:source <https://www.enisa.europa.eu/publications/risk-management-standards> ;
    rdfs:isDefinedBy dpvo-risk: ;
    sw:term_status "accepted"@en .

dpvo-risk:FMEA a owl:NamedIndividual,
        dpvo-risk:QualitativeRiskAssessmentTechnique,
        dpvo-risk:QuantitativeRiskAssessmentTechnique ;
    rdfs:label "Failure Modes And Effects Analysis (FMEA)"@en ;
    dct:created "2022-08-18"^^xsd:date ;
    dct:creator "Harshvardhan J. Pandit"^^xsd:string ;
    dct:description "Considers the ways in which each component of a system might fail and the failure causes and effects."@en ;
    dct:source <https://www.iso.org/standard/72140.html> ;
    rdfs:isDefinedBy dpvo-risk: ;
    sw:term_status "accepted"@en .

dpvo-risk:FMECA a owl:NamedIndividual,
        dpvo-risk:QualitativeRiskAssessmentTechnique,
        dpvo-risk:QuantitativeRiskAssessmentTechnique ;
    rdfs:label "Failure Modes And Effects And Criticality Analysis (FMECA)"@en ;
    dct:created "2022-08-18"^^xsd:date ;
    dct:creator "Harshvardhan J. Pandit"^^xsd:string ;
    dct:description "Considers the ways in which each component of a system might fail and the failure causes and effects. FMEA followed by a criticality analysis which defines the significance of each failure mode (FMECA)."@en ;
    dct:source <https://www.iso.org/standard/72140.html> ;
    rdfs:isDefinedBy dpvo-risk: ;
    sw:term_status "accepted"@en .

dpvo-risk:FNDiagrams a owl:NamedIndividual,
        dpvo-risk:QuantitativeRiskAssessmentTechnique ;
    rdfs:label "F-N Diagrams"@en ;
    dct:created "2022-08-18"^^xsd:date ;
    dct:creator "Harshvardhan J. Pandit"^^xsd:string ;
    dct:description "Special case of quantitative consequence/likelihood graph applied to consideration of tolerability of risk to human life."@en ;
    dct:source <https://www.iso.org/standard/72140.html> ;
    rdfs:isDefinedBy dpvo-risk: ;
    sw:term_status "accepted"@en .

dpvo-risk:FaultTreeAnalysis a owl:NamedIndividual,
        dpvo-risk:QualitativeRiskAssessmentTechnique,
        dpvo-risk:QuantitativeRiskAssessmentTechnique ;
    rdfs:label "Fault Tree Analysis"@en ;
    dct:created "2022-08-18"^^xsd:date ;
    dct:creator "Harshvardhan J. Pandit"^^xsd:string ;
    dct:description "Analyses causes of a focus event using Boolean logic to describe combinations of faults. Variations include a success tree where the top event is desired and a cause tree used to investigate past events."@en ;
    dct:source <https://www.iso.org/standard/72140.html> ;
    rdfs:isDefinedBy dpvo-risk: ;
    sw:term_status "accepted"@en .

dpvo-risk:FinancialEquipmentCosts a owl:Class ;
    rdfs:label "Financial Equipment Costs"@en ;
    dct:created "2022-08-17"^^xsd:date ;
    dct:creator "Harshvardhan J. Pandit"^^xsd:string ;
    dct:description ""@en ;
    dct:source <https://www.iso.org/standard/75281.html> ;
    rdfs:isDefinedBy dpvo-risk: ;
    rdfs:subClassOf dpvo:Detriment ;
    sw:term_status "accepted"@en .

dpvo-risk:FinancialInvestigationCosts a owl:Class ;
    rdfs:label "Financial Investigation Costs"@en ;
    dct:created "2022-08-17"^^xsd:date ;
    dct:creator "Harshvardhan J. Pandit"^^xsd:string ;
    dct:description ""@en ;
    dct:source <https://www.iso.org/standard/75281.html> ;
    rdfs:isDefinedBy dpvo-risk: ;
    rdfs:subClassOf dpvo:Detriment ;
    sw:term_status "accepted"@en .

dpvo-risk:FinancialLoss a owl:Class ;
    rdfs:label "Financial Loss"@en ;
    dct:created "2022-08-17"^^xsd:date ;
    dct:creator "Harshvardhan J. Pandit"^^xsd:string ;
    dct:description ""@en ;
    dct:source <https://www.iso.org/standard/75281.html> ;
    rdfs:isDefinedBy dpvo-risk: ;
    rdfs:subClassOf dpvo:Damage ;
    sw:term_status "accepted"@en .

dpvo-risk:FinancialPersonnelCosts a owl:Class ;
    rdfs:label "Financial Personnel Costs"@en ;
    dct:created "2022-08-17"^^xsd:date ;
    dct:creator "Harshvardhan J. Pandit"^^xsd:string ;
    dct:description ""@en ;
    dct:source <https://www.iso.org/standard/75281.html> ;
    rdfs:isDefinedBy dpvo-risk: ;
    rdfs:subClassOf dpvo:Detriment ;
    sw:term_status "accepted"@en .

dpvo-risk:FinancialRepairCosts a owl:Class ;
    rdfs:label "Financial Repair Costs"@en ;
    dct:created "2022-08-17"^^xsd:date ;
    dct:creator "Harshvardhan J. Pandit"^^xsd:string ;
    dct:description ""@en ;
    dct:source <https://www.iso.org/standard/75281.html> ;
    rdfs:isDefinedBy dpvo-risk: ;
    rdfs:subClassOf dpvo:Detriment ;
    sw:term_status "accepted"@en .

dpvo-risk:Fishbone a owl:NamedIndividual,
        dpvo-risk:QualitativeRiskAssessmentTechnique ;
    rdfs:label "Ishikawa (Fishbone)"@en ;
    dct:created "2022-08-18"^^xsd:date ;
    dct:creator "Harshvardhan J. Pandit"^^xsd:string ;
    dct:description "Identifies contributory factors to a defined outcome (wanted or unwanted). Contributory factors are usually divided into predefined categories and displayed in a tree structure or a fishbone diagram."@en ;
    dct:source <https://www.iso.org/standard/72140.html> ;
    rdfs:isDefinedBy dpvo-risk: ;
    sw:term_status "accepted"@en .

dpvo-risk:Fraud a owl:Class ;
    rdfs:label "Fraud"@en ;
    dct:created "2022-08-17"^^xsd:date ;
    dct:creator "Harshvardhan J. Pandit"^^xsd:string ;
    dct:description ""@en ;
    dct:source <https://www.iso.org/standard/75281.html> ;
    rdfs:isDefinedBy dpvo-risk: ;
    rdfs:subClassOf dpvo:Harm ;
    sw:term_status "accepted"@en .

dpvo-risk:GCSOS a owl:NamedIndividual,
        dpvo-risk:RiskManagementMethodology ;
    rdfs:label "GCSOS"@en ;
    dct:created "2022-08-18"^^xsd:date ;
    dct:creator "Harshvardhan J. Pandit"^^xsd:string ;
    dct:description "The Guidelines on Cyber Security Onboard Ships (GCSOS) guidelines explain why and how cyber risks should be managed in a shipping context. They outline the risk assessment process with an explanation of the part played by each component of cyber risk and offer advice on how to respond to and recover from cyber incidents"@en ;
    dct:source <https://www.enisa.europa.eu/publications/compendium-of-risk-management-frameworks> ;
    rdfs:isDefinedBy dpvo-risk: ;
    sw:term_status "accepted"@en .

dpvo-risk:GameTheory a owl:NamedIndividual,
        dpvo-risk:QuantitativeRiskAssessmentTechnique ;
    rdfs:label "Game Theory"@en ;
    dct:created "2022-08-18"^^xsd:date ;
    dct:creator "Harshvardhan J. Pandit"^^xsd:string ;
    dct:description "The study of strategic decision making to model the impact of the decisions of different players involved in the game. Example application area can be risk based pricing."@en ;
    dct:source <https://www.iso.org/standard/72140.html> ;
    rdfs:isDefinedBy dpvo-risk: ;
    sw:term_status "accepted"@en .

dpvo-risk:GovernmentCrisis a owl:Class ;
    rdfs:label "Government Crisis"@en ;
    dct:created "2022-08-17"^^xsd:date ;
    dct:creator "Harshvardhan J. Pandit"^^xsd:string ;
    dct:description ""@en ;
    dct:source <https://www.iso.org/standard/75281.html> ;
    rdfs:isDefinedBy dpvo-risk: ;
    rdfs:subClassOf dpvo:Detriment ;
    sw:term_status "accepted"@en .

dpvo-risk:HACCP a owl:NamedIndividual,
        dpvo-risk:QualitativeRiskAssessmentTechnique ;
    rdfs:label "Hazard Analysis And Critical Control Points (HACCP)"@en ;
    dct:created "2022-08-18"^^xsd:date ;
    dct:creator "Harshvardhan J. Pandit"^^xsd:string ;
    dct:description "Analyses the risk reduction that can be achieved by various layers of protection."@en ;
    dct:source <https://www.iso.org/standard/72140.html> ;
    rdfs:isDefinedBy dpvo-risk: ;
    sw:term_status "accepted"@en .

dpvo-risk:HAZOP a owl:NamedIndividual,
        dpvo-risk:QualitativeRiskAssessmentTechnique ;
    rdfs:label "Hazard And Operability Studies (HAZOP)"@en ;
    dct:created "2022-08-18"^^xsd:date ;
    dct:creator "Harshvardhan J. Pandit"^^xsd:string ;
    dct:description "A structured and systematic examination of a planned or existing process or operation in order to identify and evaluate problems that might represent risk to personnel or equipment, or prevent efficient operation"@en ;
    dct:source <https://www.iso.org/standard/72140.html> ;
    rdfs:isDefinedBy dpvo-risk: ;
    sw:term_status "accepted"@en .

dpvo-risk:HITRUST-CSF a owl:NamedIndividual,
        dpvo-risk:RiskManagementMethodology ;
    rdfs:label "HITRUST-CSF"@en ;
    dct:created "2022-08-18"^^xsd:date ;
    dct:creator "Harshvardhan J. Pandit"^^xsd:string ;
    dct:description "The HITRUST Cyber-Security Framework (CSF) is a framework created by security industry experts to safeguard sensitive information and manage information risk for organisations across all industries and throughout the third-party supply chain"@en ;
    dct:source <https://www.enisa.europa.eu/publications/compendium-of-risk-management-frameworks> ;
    rdfs:isDefinedBy dpvo-risk: ;
    sw:term_status "accepted"@en .

dpvo-risk:HaltSource a owl:Class ;
    rdfs:label "Halt Source"@en ;
    dct:created "2022-08-19"^^xsd:date ;
    dct:creator "Harshvardhan J. Pandit"^^xsd:string ;
    dct:description "Risk Control that halts the risk source or prevents it from materialising"@en ;
    rdfs:isDefinedBy dpvo-risk: ;
    rdfs:subClassOf dpvo-risk:ControlRiskSource ;
    sw:term_status "accepted"@en .

dpvo-risk:HarmfulSpeech a owl:Class ;
    rdfs:label "Harmful Spech"@en ;
    dct:created "2022-08-17"^^xsd:date ;
    dct:creator "Harshvardhan J. Pandit"^^xsd:string ;
    dct:description ""@en ;
    dct:source <https://www.enisa.europa.eu/publications/reference-incident-classification-taxonomy/> ;
    rdfs:isDefinedBy dpvo-risk: ;
    rdfs:subClassOf dpvo:Harm ;
    sw:term_status "accepted"@en .

dpvo-risk:HealthLifeImpact a owl:Class ;
    rdfs:label "Health and life impact"@en ;
    dct:created "2022-08-17"^^xsd:date ;
    dct:creator "Harshvardhan J. Pandit"^^xsd:string ;
    dct:description ""@en ;
    dct:source <https://www.enisa.europa.eu/publications/methodology-for-a-sectoral-cybersecurity-assessment> ;
    rdfs:isDefinedBy dpvo-risk: ;
    rdfs:subClassOf dpvo:Impact ;
    sw:term_status "accepted"@en .

dpvo-risk:HumanErrors a owl:Class ;
    rdfs:label "Human Errors"@en ;
    dct:created "2022-08-17"^^xsd:date ;
    dct:creator "Harshvardhan J. Pandit"^^xsd:string ;
    dct:description ""@en ;
    dct:source <https://www.enisa.europa.eu/publications/reference-incident-classification-taxonomy/> ;
    rdfs:isDefinedBy dpvo-risk: ;
    rdfs:subClassOf dpvo:Detriment ;
    sw:term_status "accepted"@en .

dpvo-risk:HumanReliabilityAnalysis a owl:NamedIndividual,
        dpvo-risk:QualitativeRiskAssessmentTechnique,
        dpvo-risk:QuantitativeRiskAssessmentTechnique ;
    rdfs:label "Human Reliability Analysis"@en ;
    dct:created "2022-08-18"^^xsd:date ;
    dct:creator "Harshvardhan J. Pandit"^^xsd:string ;
    dct:description "A set of techniques for identifying the potential for human error and estimating the likelihood of failure."@en ;
    dct:source <https://www.iso.org/standard/72140.html> ;
    rdfs:isDefinedBy dpvo-risk: ;
    sw:term_status "accepted"@en .

dpvo-risk:IMO-MSC-FAL1-CIRC3 a owl:NamedIndividual,
        dpvo-risk:RiskManagementMethodology ;
    rdfs:label "IMO MSC-FAL.1/CIRC.3"@en ;
    dct:created "2022-08-18"^^xsd:date ;
    dct:creator "Harshvardhan J. Pandit"^^xsd:string ;
    dct:description "The official International Maritime Organization guidelines IMO MSC-FAL.1/CIRC.3 provide a high-level approach to the management pf maritime cyber risk which refers to the extent a technology asset is exposed to risks during an event that could result in shipping-related operational failure"@en ;
    dct:source <https://www.enisa.europa.eu/publications/compendium-of-risk-management-frameworks> ;
    rdfs:isDefinedBy dpvo-risk: ;
    sw:term_status "accepted"@en .

dpvo-risk:IRAM2 a owl:NamedIndividual,
        dpvo-risk:RiskManagementMethodology ;
    rdfs:label "IRAM2"@en ;
    dct:created "2022-08-18"^^xsd:date ;
    dct:creator "Harshvardhan J. Pandit"^^xsd:string ;
    dct:description "Information Risk Assessment Methodology (IRAM2) supports risk assessment and treatment and entails a six-phase process, and is is implemented by an automated toolset"@en ;
    dct:source <https://www.enisa.europa.eu/publications/compendium-of-risk-management-frameworks> ;
    rdfs:isDefinedBy dpvo-risk: ;
    sw:term_status "accepted"@en .

dpvo-risk:IS-BM a owl:NamedIndividual,
        dpvo-risk:RiskManagementMethodology ;
    rdfs:label "IS-BM"@en ;
    dct:created "2022-08-18"^^xsd:date ;
    dct:creator "Harshvardhan J. Pandit"^^xsd:string ;
    dct:description "The IS risk analysis method is based on a business model using a quantitative approach. The values of IS assets come from their importance towards operational continuity, as well as from their replacement costs"@en ;
    dct:source <https://www.enisa.europa.eu/publications/compendium-of-risk-management-frameworks> ;
    rdfs:isDefinedBy dpvo-risk: ;
    sw:term_status "accepted"@en .

dpvo-risk:ISACA-RISK-IT a owl:NamedIndividual,
        dpvo-risk:RiskManagementMethodology ;
    rdfs:label "ISACA-RISK-IT"@en ;
    dct:created "2022-08-18"^^xsd:date ;
    dct:creator "Harshvardhan J. Pandit"^^xsd:string ;
    dct:description "The ISACA Risk IT Framework provides a set of guiding principles and supporting practices for enterprise management, combined to deliver a comprehensive process model for governing and managing IT risk"@en ;
    dct:source <https://www.enisa.europa.eu/publications/compendium-of-risk-management-frameworks> ;
    rdfs:isDefinedBy dpvo-risk: ;
    sw:term_status "accepted"@en .

dpvo-risk:ISAMM a owl:NamedIndividual,
        dpvo-risk:RiskManagementMethodology ;
    rdfs:label "ISAMM"@en ;
    dct:created "2022-08-18"^^xsd:date ;
    dct:creator "Harshvardhan J. Pandit"^^xsd:string ;
    dct:description "Information Security Assessment and Monitoring Method (ISAMM) is a quantitative type of risk management methodology that can be applied by various organisations such as governmental agencies, large companies and small and medium size enterprises"@en ;
    dct:source <https://www.enisa.europa.eu/publications/risk-management-standards> ;
    rdfs:isDefinedBy dpvo-risk: ;
    sw:term_status "accepted"@en .

dpvo-risk:ISO-IEC-27005-2018 a owl:NamedIndividual,
        dpvo-risk:RiskManagementMethodology ;
    rdfs:label "ISO/IEC 27005:2018"@en ;
    dct:created "2022-08-18"^^xsd:date ;
    dct:creator "Harshvardhan J. Pandit"^^xsd:string ;
    dct:description "ISO/IEC 27005:2018 ‘Information technology — Security techniques — Information security risk management’ is a risk management framework applicable to all types of organisations (e.g. commercial enterprises, government agencies, non-profit organisations) which intend to manage risks that could compromise the organisation’s information security"@en ;
    dct:source <https://www.enisa.europa.eu/publications/compendium-of-risk-management-frameworks> ;
    rdfs:isDefinedBy dpvo-risk: ;
    sw:term_status "accepted"@en .

dpvo-risk:ISRAM a owl:NamedIndividual,
        dpvo-risk:RiskManagementMethodology ;
    rdfs:label "ISRAM"@en ;
    dct:created "2022-08-18"^^xsd:date ;
    dct:creator "Harshvardhan J. Pandit"^^xsd:string ;
    dct:description "ISRAM is a quantitative, paper-based risk analysis method that is designed to allow effective participation of managers and staff in the process"@en ;
    dct:source <https://www.enisa.europa.eu/publications/compendium-of-risk-management-frameworks> ;
    rdfs:isDefinedBy dpvo-risk: ;
    sw:term_status "accepted"@en .

dpvo-risk:IT-Grundschutz a owl:NamedIndividual,
        dpvo-risk:RiskManagementMethodology ;
    rdfs:label "IT-Grundschutz"@en ;
    dct:created "2022-08-18"^^xsd:date ;
    dct:creator "Harshvardhan J. Pandit"^^xsd:string ;
    dct:description "IT-Grundschutz has been developed by the Federal Office for Information Security in Germany. IT-Grundschutz provides a configuration for the establishment of an integrated and effective IT security managemen"@en ;
    dct:source <https://www.enisa.europa.eu/publications/risk-management-standards> ;
    rdfs:isDefinedBy dpvo-risk: ;
    sw:term_status "accepted"@en .

dpvo-risk:IdentityDispute a owl:Class ;
    rdfs:label "Identity Dispute"@en ;
    dct:created "2022-08-24"^^xsd:date ;
    dct:creator "Harshvardhan J. Pandit"^^xsd:string ;
    dct:description ""@en ;
    rdfs:isDefinedBy dpvo-risk: ;
    rdfs:subClassOf dpvo:Detriment ;
    sw:term_status "accepted"@en .

dpvo-risk:IdentityFraud a owl:Class ;
    rdfs:label "Identity Fraud"@en ;
    dct:created "2022-08-17"^^xsd:date ;
    dct:creator "Harshvardhan J. Pandit"^^xsd:string ;
    dct:description ""@en ;
    dct:source <https://www.enisa.europa.eu/topics/threat-risk-management/threats-and-trends/enisa-threat-landscape/threat-taxonomy/view> ;
    rdfs:isDefinedBy dpvo-risk: ;
    rdfs:subClassOf dpvo:Harm ;
    sw:term_status "accepted"@en .

dpvo-risk:IdentityTheft a owl:Class ;
    rdfs:label "Identity Theft"@en ;
    dct:created "2022-08-17"^^xsd:date ;
    dct:creator "Harshvardhan J. Pandit"^^xsd:string ;
    dct:description ""@en ;
    dct:source <https://www.enisa.europa.eu/topics/threat-risk-management/threats-and-trends/enisa-threat-landscape/threat-taxonomy/view> ;
    rdfs:isDefinedBy dpvo-risk: ;
    rdfs:subClassOf dpvo:Harm ;
    sw:term_status "accepted"@en .

dpvo-risk:IllegalProcessingData a owl:Class ;
    rdfs:label "Illegal Processing of Data"@en ;
    dct:created "2022-08-17"^^xsd:date ;
    dct:creator "Harshvardhan J. Pandit"^^xsd:string ;
    dct:description ""@en ;
    dct:source <https://www.iso.org/standard/75281.html> ;
    rdfs:isDefinedBy dpvo-risk: ;
    rdfs:subClassOf dpvo:Damage ;
    sw:term_status "accepted"@en .

dpvo-risk:ImpactOnDataSubject a owl:Class ;
    rdfs:label "Impact on Data Subject"@en ;
    dct:created "2022-10-22"^^xsd:date ;
    dct:creator "Georg P Krog"^^xsd:string,
        "Harshvardhan J. Pandit"^^xsd:string ;
    dct:description ""@en ;
    rdfs:isDefinedBy dpvo-risk: ;
    rdfs:subClassOf dpvo:Impact ;
    sw:term_status "accepted"@en .

dpvo-risk:ImpacttoRights a owl:Class ;
    rdfs:label "Impact to Rights"@en ;
    dct:created "2022-08-17"^^xsd:date ;
    dct:creator "Harshvardhan J. Pandit"^^xsd:string ;
    dct:description ""@en ;
    dct:source <https://www.iso.org/standard/75281.html> ;
    rdfs:isDefinedBy dpvo-risk: ;
    rdfs:subClassOf dpvo:Impact ;
    sw:term_status "accepted"@en .

dpvo-risk:IncreaseInternalCost a owl:Class ;
    rdfs:label "Increase Internal Cost"@en ;
    dct:created "2022-08-17"^^xsd:date ;
    dct:creator "Harshvardhan J. Pandit"^^xsd:string ;
    dct:description ""@en ;
    dct:source <https://www.iso.org/standard/75281.html> ;
    rdfs:isDefinedBy dpvo-risk: ;
    rdfs:subClassOf dpvo:Detriment ;
    sw:term_status "accepted"@en .

dpvo-risk:IndustrialCrisis a owl:Class ;
    rdfs:label "Industrial Crisis"@en ;
    dct:created "2022-08-17"^^xsd:date ;
    dct:creator "Harshvardhan J. Pandit"^^xsd:string ;
    dct:description ""@en ;
    dct:source <https://www.iso.org/standard/75281.html> ;
    rdfs:isDefinedBy dpvo-risk: ;
    rdfs:subClassOf dpvo:Detriment ;
    sw:term_status "accepted"@en .

dpvo-risk:InfluenceDiagrams a owl:NamedIndividual,
        dpvo-risk:QuantitativeRiskAssessmentTechnique ;
    rdfs:label "Influence Diagrams"@en ;
    dct:created "2022-08-18"^^xsd:date ;
    dct:creator "Harshvardhan J. Pandit"^^xsd:string ;
    dct:description "An extended version of Bayesian networks that includes variables representing uncertainties, consequences and actions"@en ;
    dct:source <https://www.iso.org/standard/72140.html> ;
    rdfs:isDefinedBy dpvo-risk: ;
    sw:term_status "accepted"@en .

dpvo-risk:Injury a owl:Class ;
    rdfs:label "Injury"@en ;
    dct:created "2022-08-17"^^xsd:date ;
    dct:creator "Harshvardhan J. Pandit"^^xsd:string ;
    dct:description ""@en ;
    dct:source <https://www.iso.org/standard/75281.html> ;
    rdfs:isDefinedBy dpvo-risk: ;
    rdfs:subClassOf dpvo:Harm ;
    sw:term_status "accepted"@en .

dpvo-risk:InterceptionCommunications a owl:Class ;
    rdfs:label "Interception of Communications"@en ;
    dct:created "2022-08-17"^^xsd:date ;
    dct:creator "Harshvardhan J. Pandit"^^xsd:string ;
    dct:description ""@en ;
    dct:source <https://www.iso.org/standard/75281.html> ;
    rdfs:isDefinedBy dpvo-risk: ;
    rdfs:subClassOf dpvo:Damage ;
    sw:term_status "accepted"@en .

dpvo-risk:InternalOperationDisruption a owl:Class ;
    rdfs:label "Internal Operation Disruption"@en ;
    dct:created "2022-08-17"^^xsd:date ;
    dct:creator "Harshvardhan J. Pandit"^^xsd:string ;
    dct:description ""@en ;
    dct:source <https://www.iso.org/standard/75281.html> ;
    rdfs:isDefinedBy dpvo-risk: ;
    rdfs:subClassOf dpvo:Detriment ;
    sw:term_status "accepted"@en .

dpvo-risk:Interviews a owl:NamedIndividual,
        dpvo-risk:QualitativeRiskAssessmentTechnique ;
    rdfs:label "Interviews"@en ;
    dct:created "2022-08-18"^^xsd:date ;
    dct:creator "Harshvardhan J. Pandit"^^xsd:string ;
    dct:description "Structured or semi- structured one-to-one conversations to elicit views."@en ;
    dct:source <https://www.iso.org/standard/72140.html> ;
    rdfs:isDefinedBy dpvo-risk: ;
    sw:term_status "accepted"@en .

dpvo-risk:KnownVulnerabilityExploited a owl:Class ;
    rdfs:label "Known Vulnerability Exploited"@en ;
    dct:created "2022-08-17"^^xsd:date ;
    dct:creator "Harshvardhan J. Pandit"^^xsd:string ;
    dct:description ""@en ;
    dct:source <https://www.enisa.europa.eu/publications/reference-incident-classification-taxonomy/> ;
    rdfs:isDefinedBy dpvo-risk: ;
    rdfs:subClassOf dpvo:Detriment ;
    sw:term_status "accepted"@en .

dpvo-risk:LOPA a owl:NamedIndividual,
        dpvo-risk:QualitativeRiskAssessmentTechnique,
        dpvo-risk:QuantitativeRiskAssessmentTechnique ;
    rdfs:label "Layer Protection Analysis (LOPA)"@en ;
    dct:created "2022-08-18"^^xsd:date ;
    dct:creator "Harshvardhan J. Pandit"^^xsd:string ;
    dct:description "Analyses the risk reduction that can be achieved by various layers of protection."@en ;
    dct:source <https://www.iso.org/standard/72140.html> ;
    rdfs:isDefinedBy dpvo-risk: ;
    sw:term_status "accepted"@en .

dpvo-risk:LawEnforcementAdverseEffects a owl:Class ;
    rdfs:label "Law Enforcement Adverse Effects"@en ;
    dct:created "2022-08-17"^^xsd:date ;
    dct:creator "Harshvardhan J. Pandit"^^xsd:string ;
    dct:description ""@en ;
    dct:source <https://www.iso.org/standard/75281.html> ;
    rdfs:isDefinedBy dpvo-risk: ;
    rdfs:subClassOf dpvo:Detriment ;
    sw:term_status "accepted"@en .

dpvo-risk:LimitationOfRights a owl:Class ;
    rdfs:label "Limitation of Rights"@en ;
    dct:created "2022-08-18"^^xsd:date ;
    dct:creator "Georg P Krog"^^xsd:string,
        "Harshvardhan J. Pandit"^^xsd:string ;
    dct:description ""@en ;
    rdfs:isDefinedBy dpvo-risk: ;
    rdfs:subClassOf dpvo:Harm ;
    sw:term_status "accepted"@en .

dpvo-risk:LossAssets a owl:Class ;
    rdfs:label "Loss of Assets"@en ;
    dct:created "2022-08-17"^^xsd:date ;
    dct:creator "Harshvardhan J. Pandit"^^xsd:string ;
    dct:description ""@en ;
    dct:source <https://www.iso.org/standard/75281.html> ;
    rdfs:isDefinedBy dpvo-risk: ;
    rdfs:subClassOf dpvo:MaterialDamage ;
    sw:term_status "accepted"@en .

dpvo-risk:LossCompetitiveAdvantage a owl:Class ;
    rdfs:label "Loss of Competitive Advantage"@en ;
    dct:created "2022-08-17"^^xsd:date ;
    dct:creator "Harshvardhan J. Pandit"^^xsd:string ;
    dct:description ""@en ;
    dct:source <https://www.iso.org/standard/75281.html> ;
    rdfs:isDefinedBy dpvo-risk: ;
    rdfs:subClassOf dpvo:NonMaterialDamage ;
    sw:term_status "accepted"@en .

dpvo-risk:LossControlOverData a owl:Class ;
    rdfs:label "Loss of Control over Data"@en ;
    dct:created "2022-08-19"^^xsd:date ;
    dct:creator "Georg P Krog"^^xsd:string,
        "Harshvardhan J. Pandit"^^xsd:string ;
    dct:description ""@en ;
    rdfs:isDefinedBy dpvo-risk: ;
    rdfs:subClassOf dpvo:NonMaterialDamage ;
    sw:term_status "accepted"@en .

dpvo-risk:LossCredibility a owl:Class ;
    rdfs:label "Loss of Credibility"@en ;
    dct:created "2022-08-17"^^xsd:date ;
    dct:creator "Harshvardhan J. Pandit"^^xsd:string ;
    dct:description ""@en ;
    dct:source <https://www.iso.org/standard/75281.html> ;
    rdfs:isDefinedBy dpvo-risk: ;
    rdfs:subClassOf dpvo:Detriment ;
    sw:term_status "accepted"@en .

dpvo-risk:LossCustomerConfidence a owl:Class ;
    rdfs:label "Loss of Customer Confidence"@en ;
    dct:created "2022-08-17"^^xsd:date ;
    dct:creator "Harshvardhan J. Pandit"^^xsd:string ;
    dct:description ""@en ;
    dct:source <https://www.iso.org/standard/75281.html> ;
    rdfs:isDefinedBy dpvo-risk: ;
    rdfs:subClassOf dpvo:Detriment ;
    sw:term_status "accepted"@en .

dpvo-risk:LossCustomers a owl:Class ;
    rdfs:label "Loss of Customers"@en ;
    dct:created "2022-08-17"^^xsd:date ;
    dct:creator "Harshvardhan J. Pandit"^^xsd:string ;
    dct:description ""@en ;
    dct:source <https://www.iso.org/standard/75281.html> ;
    rdfs:isDefinedBy dpvo-risk: ;
    rdfs:subClassOf dpvo:NonMaterialDamage ;
    sw:term_status "accepted"@en .

dpvo-risk:LossData a owl:Class ;
    rdfs:label "Loss of Data"@en ;
    dct:created "2022-08-17"^^xsd:date ;
    dct:creator "Harshvardhan J. Pandit"^^xsd:string ;
    dct:description ""@en ;
    dct:source <https://www.enisa.europa.eu/topics/threat-risk-management/threats-and-trends/enisa-threat-landscape/threat-taxonomy/view> ;
    rdfs:isDefinedBy dpvo-risk: ;
    rdfs:subClassOf dpvo:NonMaterialDamage ;
    sw:term_status "accepted"@en .

dpvo-risk:LossFunds a owl:Class ;
    rdfs:label "Loss of Funds"@en ;
    dct:created "2022-08-17"^^xsd:date ;
    dct:creator "Harshvardhan J. Pandit"^^xsd:string ;
    dct:description ""@en ;
    dct:source <https://www.iso.org/standard/75281.html> ;
    rdfs:isDefinedBy dpvo-risk: ;
    rdfs:subClassOf dpvo:MaterialDamage ;
    sw:term_status "accepted"@en .

dpvo-risk:LossGoods a owl:Class ;
    rdfs:label "Loss of Goods"@en ;
    dct:created "2022-08-17"^^xsd:date ;
    dct:creator "Harshvardhan J. Pandit"^^xsd:string ;
    dct:description ""@en ;
    dct:source <https://www.iso.org/standard/75281.html> ;
    rdfs:isDefinedBy dpvo-risk: ;
    rdfs:subClassOf dpvo:MaterialDamage ;
    sw:term_status "accepted"@en .

dpvo-risk:LossGoodwill a owl:Class ;
    rdfs:label "Loss of Goodwill"@en ;
    dct:created "2022-08-17"^^xsd:date ;
    dct:creator "Harshvardhan J. Pandit"^^xsd:string ;
    dct:description ""@en ;
    dct:source <https://www.iso.org/standard/75281.html> ;
    rdfs:isDefinedBy dpvo-risk: ;
    rdfs:subClassOf dpvo:Detriment ;
    sw:term_status "accepted"@en .

dpvo-risk:LossNegotiatingCapacity a owl:Class ;
    rdfs:label "Loss of Negotiating Capacity"@en ;
    dct:created "2022-08-17"^^xsd:date ;
    dct:creator "Harshvardhan J. Pandit"^^xsd:string ;
    dct:description ""@en ;
    dct:source <https://www.iso.org/standard/75281.html> ;
    rdfs:isDefinedBy dpvo-risk: ;
    rdfs:subClassOf dpvo:Detriment ;
    sw:term_status "accepted"@en .

dpvo-risk:LossOpportunity a owl:Class ;
    rdfs:label "Loss of Opportunity"@en ;
    dct:created "2022-08-17"^^xsd:date ;
    dct:creator "Harshvardhan J. Pandit"^^xsd:string ;
    dct:description ""@en ;
    dct:source <https://www.iso.org/standard/75281.html> ;
    rdfs:isDefinedBy dpvo-risk: ;
    rdfs:subClassOf dpvo:Detriment ;
    sw:term_status "accepted"@en .

dpvo-risk:LossProprietaryInformation a owl:Class ;
    rdfs:label "Loss of Proprietary Information"@en ;
    dct:created "2022-08-17"^^xsd:date ;
    dct:creator "Harshvardhan J. Pandit"^^xsd:string ;
    dct:description ""@en ;
    dct:source <https://www.iso.org/standard/75281.html> ;
    rdfs:isDefinedBy dpvo-risk: ;
    rdfs:subClassOf dpvo:NonMaterialDamage ;
    sw:term_status "accepted"@en .

dpvo-risk:LossReputation a owl:Class ;
    rdfs:label "Loss of Reputation"@en ;
    dct:created "2022-08-17"^^xsd:date ;
    dct:creator "Harshvardhan J. Pandit"^^xsd:string ;
    dct:description ""@en ;
    dct:source <https://www.iso.org/standard/75281.html> ;
    rdfs:isDefinedBy dpvo-risk: ;
    rdfs:subClassOf dpvo:Detriment ;
    sw:term_status "accepted"@en .

dpvo-risk:LossResources a owl:Class ;
    rdfs:label "Loss of Resources"@en ;
    dct:created "2022-08-17"^^xsd:date ;
    dct:creator "Harshvardhan J. Pandit"^^xsd:string ;
    dct:description ""@en ;
    dct:source <https://www.enisa.europa.eu/topics/threat-risk-management/threats-and-trends/enisa-threat-landscape/threat-taxonomy/view> ;
    rdfs:isDefinedBy dpvo-risk: ;
    rdfs:subClassOf dpvo:NonMaterialDamage ;
    sw:term_status "accepted"@en .

dpvo-risk:LossSuppliers a owl:Class ;
    rdfs:label "Loss of Suppliers"@en ;
    dct:created "2022-08-17"^^xsd:date ;
    dct:creator "Harshvardhan J. Pandit"^^xsd:string ;
    dct:description ""@en ;
    dct:source <https://www.iso.org/standard/75281.html> ;
    rdfs:isDefinedBy dpvo-risk: ;
    rdfs:subClassOf dpvo:NonMaterialDamage ;
    sw:term_status "accepted"@en .

dpvo-risk:LossTechnologicalAdvantage a owl:Class ;
    rdfs:label "Loss of Technological Advantage"@en ;
    dct:created "2022-08-17"^^xsd:date ;
    dct:creator "Harshvardhan J. Pandit"^^xsd:string ;
    dct:description ""@en ;
    dct:source <https://www.iso.org/standard/75281.html> ;
    rdfs:isDefinedBy dpvo-risk: ;
    rdfs:subClassOf dpvo:NonMaterialDamage ;
    sw:term_status "accepted"@en .

dpvo-risk:LossTrust a owl:Class ;
    rdfs:label "Loss of Trust"@en ;
    dct:created "2022-08-17"^^xsd:date ;
    dct:creator "Harshvardhan J. Pandit"^^xsd:string ;
    dct:description ""@en ;
    dct:source <https://www.iso.org/standard/75281.html> ;
    rdfs:isDefinedBy dpvo-risk: ;
    rdfs:subClassOf dpvo:Detriment ;
    sw:term_status "accepted"@en .

dpvo-risk:MAGERIT a owl:NamedIndividual,
        dpvo-risk:RiskManagementMethodology ;
    rdfs:label "MAGERIT"@en ;
    dct:created "2022-08-18"^^xsd:date ;
    dct:creator "Harshvardhan J. Pandit"^^xsd:string ;
    dct:description "Method for the Harmonised Analysis of Risk (MAGERIT) is an open methodology for risk analysis and management developed by the Spanish Higher Council for Electronic Government and offered as a framework and guide to the public administration"@en ;
    dct:source <https://www.enisa.europa.eu/publications/risk-management-standards> ;
    rdfs:isDefinedBy dpvo-risk: ;
    sw:term_status "accepted"@en .

dpvo-risk:MCA a owl:NamedIndividual,
        dpvo-risk:QualitativeRiskAssessmentTechnique ;
    rdfs:label "Multi-criteria Analysis (MCA)"@en ;
    dct:created "2022-08-18"^^xsd:date ;
    dct:creator "Harshvardhan J. Pandit"^^xsd:string ;
    dct:description "Compares options in a way that makes trade-offs explicit. Provides an alternative to cost/benefit analysis that does not need a monetary value to be allocated to all inputs."@en ;
    dct:source <https://www.iso.org/standard/72140.html> ;
    rdfs:isDefinedBy dpvo-risk: ;
    sw:term_status "accepted"@en .

dpvo-risk:MEHARI a owl:NamedIndividual,
        dpvo-risk:RiskManagementMethodology ;
    rdfs:label "MEHARI"@en ;
    dct:created "2022-08-18"^^xsd:date ;
    dct:creator "Harshvardhan J. Pandit"^^xsd:string ;
    dct:description "MEHARI is a free of charge qualitative risk analysis and management method developed by CLUSIF (Club for the Security of Information in France/Club de la Sécurité de l'Information Français)"@en ;
    dct:source <https://www.enisa.europa.eu/publications/risk-management-standards> ;
    rdfs:isDefinedBy dpvo-risk: ;
    sw:term_status "accepted"@en .

dpvo-risk:MONARC a owl:NamedIndividual,
        dpvo-risk:RiskManagementMethodology ;
    rdfs:label "MONARC"@en ;
    dct:created "2022-08-18"^^xsd:date ;
    dct:creator "Harshvardhan J. Pandit"^^xsd:string ;
    dct:description "MONARC (Méthode Optimisée d’analyse des risques CASES – ‘Method for an Optimised Analysis of Risks by CASES’ is a tool and a method allowing precise and repeatable risk assessments to take place"@en ;
    dct:source <https://www.enisa.europa.eu/publications/compendium-of-risk-management-frameworks> ;
    rdfs:isDefinedBy dpvo-risk: ;
    sw:term_status "accepted"@en .

dpvo-risk:MaliciousCodeAttack a owl:Class ;
    rdfs:label "Malicious Code Attack"@en ;
    dct:created "2022-08-17"^^xsd:date ;
    dct:creator "Harshvardhan J. Pandit"^^xsd:string ;
    dct:description "Intentional use of software by including or inserting in a system for a harmful purpose"@en ;
    dct:source <https://www.enisa.europa.eu/publications/reference-incident-classification-taxonomy/> ;
    rdfs:isDefinedBy dpvo-risk: ;
    rdfs:subClassOf dpvo:Detriment ;
    sw:term_status "accepted"@en .

dpvo-risk:MalwareAttack a owl:Class ;
    rdfs:label "Malware Attack"@en ;
    dct:created "2022-08-17"^^xsd:date ;
    dct:creator "Harshvardhan J. Pandit"^^xsd:string ;
    dct:description "Malware is software or firmware intended to perform an unauthorised process that will have an adverse impact on the confidentiality, integrity, or availability of a system"@en ;
    dct:source <https://www.enisa.europa.eu/publications/methodology-for-a-sectoral-cybersecurity-assessment> ;
    rdfs:isDefinedBy dpvo-risk: ;
    rdfs:subClassOf dpvo:Detriment ;
    sw:term_status "accepted"@en .

dpvo-risk:MarkovAnalysis a owl:NamedIndividual,
        dpvo-risk:QuantitativeRiskAssessmentTechnique ;
    rdfs:label "Markov Analysis"@en ;
    dct:created "2022-08-18"^^xsd:date ;
    dct:creator "Harshvardhan J. Pandit"^^xsd:string ;
    dct:description "Calculates the probability that a system that has the capacity to be in one of a number of states will be in a particular state at a time t in the future."@en ;
    dct:source <https://www.iso.org/standard/72140.html> ;
    rdfs:isDefinedBy dpvo-risk: ;
    sw:term_status "accepted"@en .

dpvo-risk:MisinformationDisinformation a owl:Class ;
    rdfs:label "MisinformationDisinformation"@en ;
    dct:created "2022-08-17"^^xsd:date ;
    dct:creator "Harshvardhan J. Pandit"^^xsd:string ;
    dct:description "Information that is untrue, misleading, or false and used intentionally (disinformation) or unintentionally (misinformation)"@en ;
    dct:source <https://www.enisa.europa.eu/publications/enisa-threat-landscape-2021> ;
    rdfs:isDefinedBy dpvo-risk: ;
    rdfs:subClassOf dpvo:Detriment ;
    sw:term_status "accepted"@en .

dpvo-risk:MisuseBreachedInformation a owl:Class ;
    rdfs:label "Misuse of Breached Information"@en ;
    dct:created "2022-08-17"^^xsd:date ;
    dct:creator "Harshvardhan J. Pandit"^^xsd:string ;
    dct:description ""@en ;
    dct:source <https://www.iso.org/standard/75281.html> ;
    rdfs:isDefinedBy dpvo-risk: ;
    rdfs:subClassOf dpvo:Detriment ;
    sw:term_status "accepted"@en .

dpvo-risk:MonitorConsequence a owl:Class ;
    rdfs:label "Monitor Consequence"@en ;
    dct:created "2022-09-03"^^xsd:date ;
    dct:creator "Harshvardhan J. Pandit"^^xsd:string ;
    dct:description "Risk Control that monitors a Risk Consequence"@en ;
    rdfs:isDefinedBy dpvo-risk: ;
    rdfs:subClassOf dpvo-risk:ControlMonitors ;
    sw:term_status "accepted"@en .

dpvo-risk:MonitorImpact a owl:Class ;
    rdfs:label "Monitor Impact"@en ;
    dct:created "2022-09-04"^^xsd:date ;
    dct:creator "Harshvardhan J. Pandit"^^xsd:string ;
    dct:description "Risk Control that monitors a Risk Impact"@en ;
    rdfs:isDefinedBy dpvo-risk: ;
    rdfs:subClassOf dpvo-risk:ControlMonitors ;
    sw:term_status "accepted"@en .

dpvo-risk:MonitorRisk a owl:Class ;
    rdfs:label "Monitor Risk"@en ;
    dct:created "2022-08-31"^^xsd:date ;
    dct:creator "Harshvardhan J. Pandit"^^xsd:string ;
    dct:description "Risk Control that monitors a Risk"@en ;
    rdfs:isDefinedBy dpvo-risk: ;
    rdfs:subClassOf dpvo-risk:ControlMonitors ;
    sw:term_status "accepted"@en .

dpvo-risk:MonitorRiskControl a owl:Class ;
    rdfs:label "Monitor Risk Control"@en ;
    dct:created "2022-09-05"^^xsd:date ;
    dct:creator "Harshvardhan J. Pandit"^^xsd:string ;
    dct:description "Risk Control that monitors another Risk Control"@en ;
    rdfs:isDefinedBy dpvo-risk: ;
    rdfs:subClassOf dpvo-risk:ControlMonitors ;
    sw:term_status "accepted"@en .

dpvo-risk:MonitorRiskSource a owl:Class ;
    rdfs:label "Monitor Risk Source"@en ;
    dct:created "2022-09-01"^^xsd:date ;
    dct:creator "Harshvardhan J. Pandit"^^xsd:string ;
    dct:description "Risk Control that monitors a Risk Source"@en ;
    rdfs:isDefinedBy dpvo-risk: ;
    rdfs:subClassOf dpvo-risk:ControlMonitors ;
    sw:term_status "accepted"@en .

dpvo-risk:MonitorVulnerabilities a owl:Class ;
    rdfs:label "Monitor Vulnerabilities"@en ;
    dct:created "2022-09-02"^^xsd:date ;
    dct:creator "Harshvardhan J. Pandit"^^xsd:string ;
    dct:description "Risk Control that monitors a Risk Vulnerability"@en ;
    rdfs:isDefinedBy dpvo-risk: ;
    rdfs:subClassOf dpvo-risk:ControlMonitors ;
    sw:term_status "accepted"@en .

dpvo-risk:MonteCarloSimulation a owl:NamedIndividual,
        dpvo-risk:QuantitativeRiskAssessmentTechnique ;
    rdfs:label "Monte Carlo Simulation"@en ;
    dct:created "2022-08-18"^^xsd:date ;
    dct:creator "Harshvardhan J. Pandit"^^xsd:string ;
    dct:description "Calculates the probability of outcomes by running multiple simulations using random variables."@en ;
    dct:source <https://www.iso.org/standard/72140.html> ;
    rdfs:isDefinedBy dpvo-risk: ;
    sw:term_status "accepted"@en .

dpvo-risk:NIST-SP-800-30 a owl:NamedIndividual,
        dpvo-risk:RiskManagementMethodology ;
    rdfs:label "NIST SP 800-30"@en ;
    dct:created "2022-08-18"^^xsd:date ;
    dct:creator "Harshvardhan J. Pandit"^^xsd:string ;
    dct:description "NIST 800-30 is a free guide that provides a foundation for the development of an effective risk management programme, containing both the definitions and the practical guidance necessary for assessing and mitigating risks identified within IT systems"@en ;
    dct:source <https://www.enisa.europa.eu/publications/risk-management-standards> ;
    rdfs:isDefinedBy dpvo-risk: ;
    sw:term_status "accepted"@en .

dpvo-risk:NIST-SP-800-37 a owl:NamedIndividual,
        dpvo-risk:RiskManagementMethodology ;
    rdfs:label "NIST SP 800-37"@en ;
    dct:created "2022-08-18"^^xsd:date ;
    dct:creator "Harshvardhan J. Pandit"^^xsd:string ;
    dct:description "NIST SP 800-37 Rev. 2 is an asset-based RMF which comprises 7 steps, namely Prepare, Categorise, Select, Implement, Assess, Authorise and Monitor. It does not adopt a specific risk assessment methodology, although the NIST 800-30 guide is extensively referenced"@en ;
    dct:source <https://www.enisa.europa.eu/publications/risk-management-standards> ;
    rdfs:isDefinedBy dpvo-risk: ;
    sw:term_status "accepted"@en .

dpvo-risk:NIST-SP-800-39 a owl:NamedIndividual,
        dpvo-risk:RiskManagementMethodology ;
    rdfs:label "NIST SP 800–39"@en ;
    dct:created "2022-08-18"^^xsd:date ;
    dct:creator "Harshvardhan J. Pandit"^^xsd:string ;
    dct:description "The purpose of NIST SP 800-39 is to provide a structured, yet flexible approach for an integrated, enterprise-wide programme for managing the risk to information security of organisational operations (i.e. mission, functions, image, and reputation) and assets, individuals, other organisations etc. on an ongoing basis"@en ;
    dct:source <https://www.enisa.europa.eu/publications/risk-management-standards> ;
    rdfs:isDefinedBy dpvo-risk: ;
    sw:term_status "accepted"@en .

dpvo-risk:NIST-SP-800-82 a owl:NamedIndividual,
        dpvo-risk:RiskManagementMethodology ;
    rdfs:label "NIST SP 800–82"@en ;
    dct:created "2022-08-18"^^xsd:date ;
    dct:creator "Harshvardhan J. Pandit"^^xsd:string ;
    dct:description "NIST SP 800-82 Rev. 2 (Stouffer, et al., 2015), entitled ‘Guide to industrial control systems (ISC) security’, is an Industrial Control Systems Security Guide"@en ;
    dct:source <https://www.enisa.europa.eu/publications/compendium-of-risk-management-frameworks> ;
    rdfs:isDefinedBy dpvo-risk: ;
    sw:term_status "accepted"@en .

dpvo-risk:NominalGroupTechnique a owl:NamedIndividual,
        dpvo-risk:QualitativeRiskAssessmentTechnique ;
    rdfs:label "Nominal Group Technique"@en ;
    dct:created "2022-08-18"^^xsd:date ;
    dct:creator "Harshvardhan J. Pandit"^^xsd:string ;
    dct:description "Technique for eliciting views from a group of people where initial participation is as individuals with no interaction, then group discussion of ideas follows."@en ;
    dct:source <https://www.iso.org/standard/72140.html> ;
    rdfs:isDefinedBy dpvo-risk: ;
    sw:term_status "accepted"@en .

dpvo-risk:O-RA a owl:NamedIndividual,
        dpvo-risk:RiskManagementMethodology ;
    rdfs:label "O-RA"@en ;
    dct:created "2022-08-18"^^xsd:date ;
    dct:creator "Harshvardhan J. Pandit"^^xsd:string ;
    dct:description "The Open Group Standard for Risk Analysis (O-RA) provides a set of standards for various aspects of information security risk analysis that is based on the Open FAIR framework and can be applied to any risk scenario"@en ;
    dct:source <https://www.enisa.europa.eu/publications/compendium-of-risk-management-frameworks> ;
    rdfs:isDefinedBy dpvo-risk: ;
    sw:term_status "accepted"@en .

dpvo-risk:OCTAVE a owl:NamedIndividual,
        dpvo-risk:RiskManagementMethodology ;
    rdfs:label "OCTAVE"@en ;
    dct:created "2022-08-18"^^xsd:date ;
    dct:creator "Harshvardhan J. Pandit"^^xsd:string ;
    dct:description "Operationally Critical Threat, Asset, and Vulnerability Evaluation (OCTAVE) is a free of charge approach to evaluations of information security risk that is comprehensive, systematic, context-driven, and self-directed"@en ;
    dct:source <https://www.enisa.europa.eu/publications/risk-management-standards> ;
    rdfs:isDefinedBy dpvo-risk: ;
    sw:term_status "accepted"@en .

dpvo-risk:OCTAVE-ALLEGRO a owl:NamedIndividual,
        dpvo-risk:RiskManagementMethodology ;
    rdfs:label "OCTAVE ALLEGRO"@en ;
    dct:created "2022-08-18"^^xsd:date ;
    dct:creator "Harshvardhan J. Pandit"^^xsd:string ;
    dct:description "OCTAVE Allegro is designed to allow broad assessment of an organisation’s operational risk environment, with the goal of producing robust results without the need for extensive knowledge of risk assessment"@en ;
    dct:source <https://www.enisa.europa.eu/publications/compendium-of-risk-management-frameworks> ;
    rdfs:isDefinedBy dpvo-risk: ;
    sw:term_status "accepted"@en .

dpvo-risk:OCTAVE-FORTE a owl:NamedIndividual,
        dpvo-risk:RiskManagementMethodology ;
    rdfs:label "OCTAVE FORTE"@en ;
    dct:created "2022-08-18"^^xsd:date ;
    dct:creator "Harshvardhan J. Pandit"^^xsd:string ;
    dct:description "The OCTAVE FORTE process model was developed to support organisations in evaluating their security risks. It applies Enterprise Risk Management (ERM) principles to bridge the gap between executives and practitioners acting as decision makers"@en ;
    dct:source <https://www.enisa.europa.eu/publications/compendium-of-risk-management-frameworks> ;
    rdfs:isDefinedBy dpvo-risk: ;
    sw:term_status "accepted"@en .

dpvo-risk:OCTAVE-S a owl:NamedIndividual,
        dpvo-risk:RiskManagementMethodology ;
    rdfs:label "OCTAVE-S"@en ;
    dct:created "2022-08-18"^^xsd:date ;
    dct:creator "Harshvardhan J. Pandit"^^xsd:string ;
    dct:description "The OCTAVE-S is based on the OCTAVE approach and is a self-directed approach, meaning that people from an organisation assume responsibility for setting the organisation’s security strategy"@en ;
    dct:source <https://www.enisa.europa.eu/publications/compendium-of-risk-management-frameworks> ;
    rdfs:isDefinedBy dpvo-risk: ;
    sw:term_status "accepted"@en .

dpvo-risk:OrganisationDisruption a owl:Class ;
    rdfs:label "Organisation Disruption"@en ;
    dct:created "2022-08-17"^^xsd:date ;
    dct:creator "Harshvardhan J. Pandit"^^xsd:string ;
    dct:description ""@en ;
    dct:source <https://www.iso.org/standard/75281.html> ;
    rdfs:isDefinedBy dpvo-risk: ;
    rdfs:subClassOf dpvo:Detriment ;
    sw:term_status "accepted"@en .

dpvo-risk:PIA a owl:NamedIndividual,
        dpvo-risk:QualitativeRiskAssessmentTechnique ;
    rdfs:label "Privacy Impact Analysis (PIA)"@en ;
    dct:created "2022-08-18"^^xsd:date ;
    dct:creator "Harshvardhan J. Pandit"^^xsd:string ;
    dct:description "Analyses how incidents and events could affect a person's privacy and identifies and quantifies the capabilities that would be needed to manage it."@en ;
    dct:source <https://www.iso.org/standard/72140.html> ;
    rdfs:isDefinedBy dpvo-risk: ;
    sw:term_status "accepted"@en .

dpvo-risk:ParetoCharts a owl:NamedIndividual,
        dpvo-risk:QuantitativeRiskAssessmentTechnique ;
    rdfs:label "Pareto Charts"@en ;
    dct:created "2022-08-18"^^xsd:date ;
    dct:creator "Harshvardhan J. Pandit"^^xsd:string ;
    dct:description "The Pareto principle (the 80–20 rule) states that, for many events, roughly 80 % of the effects come from 20 % of the causes."@en ;
    dct:source <https://www.iso.org/standard/72140.html> ;
    rdfs:isDefinedBy dpvo-risk: ;
    sw:term_status "accepted"@en .

dpvo-risk:PersonalSafetyEndangerment a owl:Class ;
    rdfs:label "Personal Safety Endangerment"@en ;
    dct:created "2022-08-17"^^xsd:date ;
    dct:creator "Harshvardhan J. Pandit"^^xsd:string ;
    dct:description ""@en ;
    dct:source <https://www.iso.org/standard/75281.html> ;
    rdfs:isDefinedBy dpvo-risk: ;
    rdfs:subClassOf dpvo:Harm ;
    sw:term_status "accepted"@en .

dpvo-risk:PersonnelAbsence a owl:Class ;
    rdfs:label "Personnel Absence"@en ;
    dct:created "2022-08-17"^^xsd:date ;
    dct:creator "Harshvardhan J. Pandit"^^xsd:string ;
    dct:description ""@en ;
    dct:source <https://www.enisa.europa.eu/topics/threat-risk-management/threats-and-trends/enisa-threat-landscape/threat-taxonomy/view> ;
    rdfs:isDefinedBy dpvo-risk: ;
    rdfs:subClassOf dpvo:NonMaterialDamage ;
    sw:term_status "accepted"@en .

dpvo-risk:PhishingScam a owl:Class ;
    rdfs:label "Phishing Scam"@en ;
    dct:created "2022-08-17"^^xsd:date ;
    dct:creator "Harshvardhan J. Pandit"^^xsd:string ;
    dct:description "A type of social engineering attack involving deceptive messages intended to reveal sensitive information"@en ;
    dct:source <https://www.enisa.europa.eu/publications/enisa-threat-landscape-for-ransomware-attacks> ;
    rdfs:isDefinedBy dpvo-risk: ;
    rdfs:subClassOf dpvo:Harm ;
    sw:term_status "accepted"@en .

dpvo-risk:PhysicalAssault a owl:Class ;
    rdfs:label "Physical Assault"@en ;
    dct:created "2022-08-17"^^xsd:date ;
    dct:creator "Harshvardhan J. Pandit"^^xsd:string ;
    dct:description ""@en ;
    dct:source <https://www.iso.org/standard/75281.html> ;
    rdfs:isDefinedBy dpvo-risk: ;
    rdfs:subClassOf dpvo:Harm ;
    sw:term_status "accepted"@en .

dpvo-risk:PhysicalSpying a owl:Class ;
    rdfs:label "Physical Spying"@en ;
    dct:created "2022-08-17"^^xsd:date ;
    dct:creator "Harshvardhan J. Pandit"^^xsd:string ;
    dct:description ""@en ;
    dct:source <https://www.iso.org/standard/75281.html> ;
    rdfs:isDefinedBy dpvo-risk: ;
    rdfs:subClassOf dpvo:NonMaterialDamage ;
    sw:term_status "accepted"@en .

dpvo-risk:PhysicalStalking a owl:Class ;
    rdfs:label "Physical Stalking"@en ;
    dct:created "2022-08-17"^^xsd:date ;
    dct:creator "Harshvardhan J. Pandit"^^xsd:string ;
    dct:description ""@en ;
    dct:source <https://www.iso.org/standard/75281.html> ;
    rdfs:isDefinedBy dpvo-risk: ;
    rdfs:subClassOf dpvo:NonMaterialDamage ;
    sw:term_status "accepted"@en .

dpvo-risk:PreventExercisingOfRights a owl:Class ;
    rdfs:label "Prevent Exercising of Rights"@en ;
    dct:created "2022-08-18"^^xsd:date ;
    dct:creator "Georg P Krog"^^xsd:string,
        "Harshvardhan J. Pandit"^^xsd:string ;
    dct:description ""@en ;
    rdfs:isDefinedBy dpvo-risk: ;
    rdfs:subClassOf dpvo:Harm ;
    sw:term_status "accepted"@en .

dpvo-risk:PrivacyImpact a owl:Class ;
    rdfs:label "Privacy impact"@en ;
    dct:created "2022-08-17"^^xsd:date ;
    dct:creator "Harshvardhan J. Pandit"^^xsd:string ;
    dct:description ""@en ;
    dct:source <https://www.enisa.europa.eu/publications/methodology-for-a-sectoral-cybersecurity-assessment> ;
    rdfs:isDefinedBy dpvo-risk: ;
    rdfs:subClassOf dpvo:Impact ;
    sw:term_status "accepted"@en .

dpvo-risk:PsychologicalHarm a owl:Class ;
    rdfs:label "Psychological Harm"@en ;
    dct:created "2022-08-17"^^xsd:date ;
    dct:creator "Harshvardhan J. Pandit"^^xsd:string ;
    dct:description ""@en ;
    dct:source <https://www.enisa.europa.eu/publications/reference-incident-classification-taxonomy/> ;
    rdfs:isDefinedBy dpvo-risk: ;
    rdfs:subClassOf dpvo:Harm ;
    sw:term_status "accepted"@en .

dpvo-risk:PublicOrderBreach a owl:Class ;
    rdfs:label "Public Order Breach"@en ;
    dct:created "2022-08-17"^^xsd:date ;
    dct:creator "Harshvardhan J. Pandit"^^xsd:string ;
    dct:description ""@en ;
    dct:source <https://www.iso.org/standard/75281.html> ;
    rdfs:isDefinedBy dpvo-risk: ;
    rdfs:subClassOf dpvo:Damage ;
    sw:term_status "accepted"@en .

dpvo-risk:RM3x3S1L1 a owl:NamedIndividual,
        dpvo-risk:RiskMatrix3x3 ;
    rdfs:label "Low Risk (RM3x3 S:1 L:1)"@en ;
    dct:created "2022-08-17"^^xsd:date ;
    dct:creator "Harshvardhan J. Pandit"^^xsd:string ;
    dct:description "Node in a 3x3 Risk Matrix with Risk Severity: Low; Likelihood: Low; and Risk Level: Low"@en ;
    rdf:value 0.11 ;
    rdfs:isDefinedBy dpvo-risk: ;
    sw:term_status "accepted"@en ;
    dpvo:hasLikelihood dpvo-risk:LowLikelihood ;
    dpvo:hasRiskLevel dpvo-risk:LowRisk ;
    dpvo:hasSeverity dpvo-risk:LowSeverity .

dpvo-risk:RM3x3S1L2 a owl:NamedIndividual,
        dpvo-risk:RiskMatrix3x3 ;
    rdfs:label "Low Risk (RM3x3 S:1 L:2)"@en ;
    dct:created "2022-08-17"^^xsd:date ;
    dct:creator "Harshvardhan J. Pandit"^^xsd:string ;
    dct:description "Node in a 3x3 Risk Matrix with Risk Severity: Low; Likelihood: Moderate; and Risk Level: Low"@en ;
    rdf:value 0.22 ;
    rdfs:isDefinedBy dpvo-risk: ;
    sw:term_status "accepted"@en ;
    dpvo:hasLikelihood dpvo-risk:ModerateLikelihood ;
    dpvo:hasRiskLevel dpvo-risk:LowRisk ;
    dpvo:hasSeverity dpvo-risk:LowSeverity .

dpvo-risk:RM3x3S1L3 a owl:NamedIndividual,
        dpvo-risk:RiskMatrix3x3 ;
    rdfs:label "Moderate Risk (RM3x3 S:1 L:3)"@en ;
    dct:created "2022-08-17"^^xsd:date ;
    dct:creator "Harshvardhan J. Pandit"^^xsd:string ;
    dct:description "Node in a 3x3 Risk Matrix with Risk Severity: Low; Likelihood: High; and Risk Level: Moderate"@en ;
    rdf:value 0.33 ;
    rdfs:isDefinedBy dpvo-risk: ;
    sw:term_status "accepted"@en ;
    dpvo:hasLikelihood dpvo-risk:HighLikelihood ;
    dpvo:hasRiskLevel dpvo-risk:ModerateRisk ;
    dpvo:hasSeverity dpvo-risk:LowSeverity .

dpvo-risk:RM3x3S2L1 a owl:NamedIndividual,
        dpvo-risk:RiskMatrix3x3 ;
    rdfs:label "Low Risk (RM3x3 S:2 L:1)"@en ;
    dct:created "2022-08-17"^^xsd:date ;
    dct:creator "Harshvardhan J. Pandit"^^xsd:string ;
    dct:description "Node in a 3x3 Risk Matrix with Risk Severity: Moderate; Likelihood: Low; and Risk Level: Low"@en ;
    rdf:value 0.22 ;
    rdfs:isDefinedBy dpvo-risk: ;
    sw:term_status "accepted"@en ;
    dpvo:hasLikelihood dpvo-risk:LowLikelihood ;
    dpvo:hasRiskLevel dpvo-risk:LowRisk ;
    dpvo:hasSeverity dpvo-risk:ModerateSeverity .

dpvo-risk:RM3x3S2L2 a owl:NamedIndividual,
        dpvo-risk:RiskMatrix3x3 ;
    rdfs:label "Moderate Risk (RM3x3 S:2 L:2)"@en ;
    dct:created "2022-08-17"^^xsd:date ;
    dct:creator "Harshvardhan J. Pandit"^^xsd:string ;
    dct:description "Node in a 3x3 Risk Matrix with Risk Severity: Moderate; Likelihood: Moderate; and Risk Level: Moderate"@en ;
    rdf:value 0.44 ;
    rdfs:isDefinedBy dpvo-risk: ;
    sw:term_status "accepted"@en ;
    dpvo:hasLikelihood dpvo-risk:ModerateLikelihood ;
    dpvo:hasRiskLevel dpvo-risk:ModerateRisk ;
    dpvo:hasSeverity dpvo-risk:ModerateSeverity .

dpvo-risk:RM3x3S2L3 a owl:NamedIndividual,
        dpvo-risk:RiskMatrix3x3 ;
    rdfs:label "High Risk (RM3x3 S:2 L:3)"@en ;
    dct:created "2022-08-17"^^xsd:date ;
    dct:creator "Harshvardhan J. Pandit"^^xsd:string ;
    dct:description "Node in a 3x3 Risk Matrix with Risk Severity: Moderate; Likelihood: High; and Risk Level: High"@en ;
    rdf:value 0.67 ;
    rdfs:isDefinedBy dpvo-risk: ;
    sw:term_status "accepted"@en ;
    dpvo:hasLikelihood dpvo-risk:HighLikelihood ;
    dpvo:hasRiskLevel dpvo-risk:HighRisk ;
    dpvo:hasSeverity dpvo-risk:ModerateSeverity .

dpvo-risk:RM3x3S3L1 a owl:NamedIndividual,
        dpvo-risk:RiskMatrix3x3 ;
    rdfs:label "Moderate Risk (RM3x3 S:3 L:1)"@en ;
    dct:created "2022-08-17"^^xsd:date ;
    dct:creator "Harshvardhan J. Pandit"^^xsd:string ;
    dct:description "Node in a 3x3 Risk Matrix with Risk Severity: High; Likelihood: Low; and Risk Level: Moderate"@en ;
    rdf:value 0.33 ;
    rdfs:isDefinedBy dpvo-risk: ;
    sw:term_status "accepted"@en ;
    dpvo:hasLikelihood dpvo-risk:LowLikelihood ;
    dpvo:hasRiskLevel dpvo-risk:ModerateRisk ;
    dpvo:hasSeverity dpvo-risk:HighSeverity .

dpvo-risk:RM3x3S3L2 a owl:NamedIndividual,
        dpvo-risk:RiskMatrix3x3 ;
    rdfs:label "High Risk (RM3x3 S:3 L:2)"@en ;
    dct:created "2022-08-17"^^xsd:date ;
    dct:creator "Harshvardhan J. Pandit"^^xsd:string ;
    dct:description "Node in a 3x3 Risk Matrix with Risk Severity: High; Likelihood: Moderate; and Risk Level: High"@en ;
    rdf:value 0.67 ;
    rdfs:isDefinedBy dpvo-risk: ;
    sw:term_status "accepted"@en ;
    dpvo:hasLikelihood dpvo-risk:ModerateLikelihood ;
    dpvo:hasRiskLevel dpvo-risk:HighRisk ;
    dpvo:hasSeverity dpvo-risk:HighSeverity .

dpvo-risk:RM3x3S3L3 a owl:NamedIndividual,
        dpvo-risk:RiskMatrix3x3 ;
    rdfs:label "High Risk (RM3x3 S:3 L:3)"@en ;
    dct:created "2022-08-17"^^xsd:date ;
    dct:creator "Harshvardhan J. Pandit"^^xsd:string ;
    dct:description "Node in a 3x3 Risk Matrix with Risk Severity: High; Likelihood: High; and Risk Level: High"@en ;
    rdf:value 1.00 ;
    rdfs:isDefinedBy dpvo-risk: ;
    sw:term_status "accepted"@en ;
    dpvo:hasLikelihood dpvo-risk:HighLikelihood ;
    dpvo:hasRiskLevel dpvo-risk:HighRisk ;
    dpvo:hasSeverity dpvo-risk:HighSeverity .

dpvo-risk:RM5x5S1L1 a owl:NamedIndividual,
        dpvo-risk:RiskMatrix5x5 ;
    rdfs:label "Very Low Risk (RM5x5 S:1 L:1)"@en ;
    dct:created "2022-08-17"^^xsd:date ;
    dct:creator "Harshvardhan J. Pandit"^^xsd:string ;
    dct:description "Node in a 5x5 Risk Matrix with Risk Severity: VeryLow; Likelihood: VeryLow; and Risk Level: VeryLow"@en ;
    rdf:value 0.04 ;
    rdfs:isDefinedBy dpvo-risk: ;
    sw:term_status "accepted"@en ;
    dpvo:hasLikelihood dpvo-risk:VeryLowLikelihood ;
    dpvo:hasRiskLevel dpvo-risk:VeryLowRisk ;
    dpvo:hasSeverity dpvo-risk:VeryLowSeverity .

dpvo-risk:RM5x5S1L2 a owl:NamedIndividual,
        dpvo-risk:RiskMatrix5x5 ;
    rdfs:label "Very Low Risk (RM5x5 S:1 L:2)"@en ;
    dct:created "2022-08-17"^^xsd:date ;
    dct:creator "Harshvardhan J. Pandit"^^xsd:string ;
    dct:description "Node in a 5x5 Risk Matrix with Risk Severity: VeryLow; Likelihood: Low; and Risk Level: VeryLow"@en ;
    rdf:value 0.08 ;
    rdfs:isDefinedBy dpvo-risk: ;
    sw:term_status "accepted"@en ;
    dpvo:hasLikelihood dpvo-risk:LowLikelihood ;
    dpvo:hasRiskLevel dpvo-risk:VeryLowRisk ;
    dpvo:hasSeverity dpvo-risk:VeryLowSeverity .

dpvo-risk:RM5x5S1L3 a owl:NamedIndividual,
        dpvo-risk:RiskMatrix5x5 ;
    rdfs:label "Very Low Risk (RM5x5 S:1 L:3)"@en ;
    dct:created "2022-08-17"^^xsd:date ;
    dct:creator "Harshvardhan J. Pandit"^^xsd:string ;
    dct:description "Node in a 5x5 Risk Matrix with Risk Severity: VeryLow; Likelihood: Moderate; and Risk Level: VeryLow"@en ;
    rdf:value 0.12 ;
    rdfs:isDefinedBy dpvo-risk: ;
    sw:term_status "accepted"@en ;
    dpvo:hasLikelihood dpvo-risk:ModerateLikelihood ;
    dpvo:hasRiskLevel dpvo-risk:VeryLowRisk ;
    dpvo:hasSeverity dpvo-risk:VeryLowSeverity .

dpvo-risk:RM5x5S1L4 a owl:NamedIndividual,
        dpvo-risk:RiskMatrix5x5 ;
    rdfs:label "Low Risk (RM5x5 S:1 L:4)"@en ;
    dct:created "2022-08-17"^^xsd:date ;
    dct:creator "Harshvardhan J. Pandit"^^xsd:string ;
    dct:description "Node in a 5x5 Risk Matrix with Risk Severity: VeryLow; Likelihood: High; and Risk Level: Low"@en ;
    rdf:value 0.16 ;
    rdfs:isDefinedBy dpvo-risk: ;
    sw:term_status "accepted"@en ;
    dpvo:hasLikelihood dpvo-risk:HighLikelihood ;
    dpvo:hasRiskLevel dpvo-risk:LowRisk ;
    dpvo:hasSeverity dpvo-risk:VeryLowSeverity .

dpvo-risk:RM5x5S1L5 a owl:NamedIndividual,
        dpvo-risk:RiskMatrix5x5 ;
    rdfs:label "Low Risk (RM5x5 S:1 L:5)"@en ;
    dct:created "2022-08-17"^^xsd:date ;
    dct:creator "Harshvardhan J. Pandit"^^xsd:string ;
    dct:description "Node in a 5x5 Risk Matrix with Risk Severity: VeryLow; Likelihood: VeryHigh; and Risk Level: Low"@en ;
    rdf:value 0.20 ;
    rdfs:isDefinedBy dpvo-risk: ;
    sw:term_status "accepted"@en ;
    dpvo:hasLikelihood dpvo-risk:VeryHighLikelihood ;
    dpvo:hasRiskLevel dpvo-risk:LowRisk ;
    dpvo:hasSeverity dpvo-risk:VeryLowSeverity .

dpvo-risk:RM5x5S2L1 a owl:NamedIndividual,
        dpvo-risk:RiskMatrix5x5 ;
    rdfs:label "Very Low Risk (RM5x5 S:2 L:1)"@en ;
    dct:created "2022-08-17"^^xsd:date ;
    dct:creator "Harshvardhan J. Pandit"^^xsd:string ;
    dct:description "Node in a 5x5 Risk Matrix with Risk Severity: Low; Likelihood: VeryLow; and Risk Level: VeryLow"@en ;
    rdf:value 0.08 ;
    rdfs:isDefinedBy dpvo-risk: ;
    sw:term_status "accepted"@en ;
    dpvo:hasLikelihood dpvo-risk:VeryLowLikelihood ;
    dpvo:hasRiskLevel dpvo-risk:VeryLowRisk ;
    dpvo:hasSeverity dpvo-risk:LowSeverity .

dpvo-risk:RM5x5S2L2 a owl:NamedIndividual,
        dpvo-risk:RiskMatrix5x5 ;
    rdfs:label "Low Risk (RM5x5 S:2 L:2)"@en ;
    dct:created "2022-08-17"^^xsd:date ;
    dct:creator "Harshvardhan J. Pandit"^^xsd:string ;
    dct:description "Node in a 5x5 Risk Matrix with Risk Severity: Low; Likelihood: Low; and Risk Level: Low"@en ;
    rdf:value 0.16 ;
    rdfs:isDefinedBy dpvo-risk: ;
    sw:term_status "accepted"@en ;
    dpvo:hasLikelihood dpvo-risk:LowLikelihood ;
    dpvo:hasRiskLevel dpvo-risk:LowRisk ;
    dpvo:hasSeverity dpvo-risk:LowSeverity .

dpvo-risk:RM5x5S2L3 a owl:NamedIndividual,
        dpvo-risk:RiskMatrix5x5 ;
    rdfs:label "Moderate Risk (RM5x5 S:2 L:3)"@en ;
    dct:created "2022-08-17"^^xsd:date ;
    dct:creator "Harshvardhan J. Pandit"^^xsd:string ;
    dct:description "Node in a 5x5 Risk Matrix with Risk Severity: Low; Likelihood: Moderate; and Risk Level: Moderate"@en ;
    rdf:value 0.24 ;
    rdfs:isDefinedBy dpvo-risk: ;
    sw:term_status "accepted"@en ;
    dpvo:hasLikelihood dpvo-risk:ModerateLikelihood ;
    dpvo:hasRiskLevel dpvo-risk:ModerateRisk ;
    dpvo:hasSeverity dpvo-risk:LowSeverity .

dpvo-risk:RM5x5S2L4 a owl:NamedIndividual,
        dpvo-risk:RiskMatrix5x5 ;
    rdfs:label "Moderate Risk (RM5x5 S:2 L:4)"@en ;
    dct:created "2022-08-17"^^xsd:date ;
    dct:creator "Harshvardhan J. Pandit"^^xsd:string ;
    dct:description "Node in a 5x5 Risk Matrix with Risk Severity: Low; Likelihood: High; and Risk Level: Moderate"@en ;
    rdf:value 0.32 ;
    rdfs:isDefinedBy dpvo-risk: ;
    sw:term_status "accepted"@en ;
    dpvo:hasLikelihood dpvo-risk:HighLikelihood ;
    dpvo:hasRiskLevel dpvo-risk:ModerateRisk ;
    dpvo:hasSeverity dpvo-risk:LowSeverity .

dpvo-risk:RM5x5S2L5 a owl:NamedIndividual,
        dpvo-risk:RiskMatrix5x5 ;
    rdfs:label "High Risk (RM5x5 S:2 L:5)"@en ;
    dct:created "2022-08-17"^^xsd:date ;
    dct:creator "Harshvardhan J. Pandit"^^xsd:string ;
    dct:description "Node in a 5x5 Risk Matrix with Risk Severity: Low; Likelihood: VeryHigh; and Risk Level: High"@en ;
    rdf:value 0.40 ;
    rdfs:isDefinedBy dpvo-risk: ;
    sw:term_status "accepted"@en ;
    dpvo:hasLikelihood dpvo-risk:VeryHighLikelihood ;
    dpvo:hasRiskLevel dpvo-risk:HighRisk ;
    dpvo:hasSeverity dpvo-risk:LowSeverity .

dpvo-risk:RM5x5S3L1 a owl:NamedIndividual,
        dpvo-risk:RiskMatrix5x5 ;
    rdfs:label "Very Low Risk (RM5x5 S:3 L:1)"@en ;
    dct:created "2022-08-17"^^xsd:date ;
    dct:creator "Harshvardhan J. Pandit"^^xsd:string ;
    dct:description "Node in a 5x5 Risk Matrix with Risk Severity: Moderate; Likelihood: VeryLow; and Risk Level: VeryLow"@en ;
    rdf:value 0.12 ;
    rdfs:isDefinedBy dpvo-risk: ;
    sw:term_status "accepted"@en ;
    dpvo:hasLikelihood dpvo-risk:VeryLowLikelihood ;
    dpvo:hasRiskLevel dpvo-risk:VeryLowRisk ;
    dpvo:hasSeverity dpvo-risk:ModerateSeverity .

dpvo-risk:RM5x5S3L2 a owl:NamedIndividual,
        dpvo-risk:RiskMatrix5x5 ;
    rdfs:label "Moderate Risk (RM5x5 S:3 L:2)"@en ;
    dct:created "2022-08-17"^^xsd:date ;
    dct:creator "Harshvardhan J. Pandit"^^xsd:string ;
    dct:description "Node in a 5x5 Risk Matrix with Risk Severity: Moderate; Likelihood: Low; and Risk Level: Moderate"@en ;
    rdf:value 0.24 ;
    rdfs:isDefinedBy dpvo-risk: ;
    sw:term_status "accepted"@en ;
    dpvo:hasLikelihood dpvo-risk:LowLikelihood ;
    dpvo:hasRiskLevel dpvo-risk:ModerateRisk ;
    dpvo:hasSeverity dpvo-risk:ModerateSeverity .

dpvo-risk:RM5x5S3L3 a owl:NamedIndividual,
        dpvo-risk:RiskMatrix5x5 ;
    rdfs:label "Moderate Risk (RM5x5 S:3 L:3)"@en ;
    dct:created "2022-08-17"^^xsd:date ;
    dct:creator "Harshvardhan J. Pandit"^^xsd:string ;
    dct:description "Node in a 5x5 Risk Matrix with Risk Severity: Moderate; Likelihood: Moderate; and Risk Level: Moderate"@en ;
    rdf:value 0.36 ;
    rdfs:isDefinedBy dpvo-risk: ;
    sw:term_status "accepted"@en ;
    dpvo:hasLikelihood dpvo-risk:ModerateLikelihood ;
    dpvo:hasRiskLevel dpvo-risk:ModerateRisk ;
    dpvo:hasSeverity dpvo-risk:ModerateSeverity .

dpvo-risk:RM5x5S3L4 a owl:NamedIndividual,
        dpvo-risk:RiskMatrix5x5 ;
    rdfs:label "High Risk (RM5x5 S:3 L:4)"@en ;
    dct:created "2022-08-17"^^xsd:date ;
    dct:creator "Harshvardhan J. Pandit"^^xsd:string ;
    dct:description "Node in a 5x5 Risk Matrix with Risk Severity: Moderate; Likelihood: High; and Risk Level: High"@en ;
    rdf:value 0.48 ;
    rdfs:isDefinedBy dpvo-risk: ;
    sw:term_status "accepted"@en ;
    dpvo:hasLikelihood dpvo-risk:HighLikelihood ;
    dpvo:hasRiskLevel dpvo-risk:HighRisk ;
    dpvo:hasSeverity dpvo-risk:ModerateSeverity .

dpvo-risk:RM5x5S3L5 a owl:NamedIndividual,
        dpvo-risk:RiskMatrix5x5 ;
    rdfs:label "Very High Risk (RM5x5 S:3 L:5)"@en ;
    dct:created "2022-08-17"^^xsd:date ;
    dct:creator "Harshvardhan J. Pandit"^^xsd:string ;
    dct:description "Node in a 5x5 Risk Matrix with Risk Severity: Moderate; Likelihood: VeryHigh; and Risk Level: VeryHigh"@en ;
    rdf:value 0.60 ;
    rdfs:isDefinedBy dpvo-risk: ;
    sw:term_status "accepted"@en ;
    dpvo:hasLikelihood dpvo-risk:VeryHighLikelihood ;
    dpvo:hasRiskLevel dpvo-risk:VeryHighRisk ;
    dpvo:hasSeverity dpvo-risk:ModerateSeverity .

dpvo-risk:RM5x5S4L1 a owl:NamedIndividual,
        dpvo-risk:RiskMatrix5x5 ;
    rdfs:label "Low Risk (RM5x5 S:4 L:1)"@en ;
    dct:created "2022-08-17"^^xsd:date ;
    dct:creator "Harshvardhan J. Pandit"^^xsd:string ;
    dct:description "Node in a 5x5 Risk Matrix with Risk Severity: High; Likelihood: VeryLow; and Risk Level: Low"@en ;
    rdf:value 0.16 ;
    rdfs:isDefinedBy dpvo-risk: ;
    sw:term_status "accepted"@en ;
    dpvo:hasLikelihood dpvo-risk:VeryLowLikelihood ;
    dpvo:hasRiskLevel dpvo-risk:LowRisk ;
    dpvo:hasSeverity dpvo-risk:HighSeverity .

dpvo-risk:RM5x5S4L2 a owl:NamedIndividual,
        dpvo-risk:RiskMatrix5x5 ;
    rdfs:label "Moderate Risk (RM5x5 S:4 L:2)"@en ;
    dct:created "2022-08-17"^^xsd:date ;
    dct:creator "Harshvardhan J. Pandit"^^xsd:string ;
    dct:description "Node in a 5x5 Risk Matrix with Risk Severity: High; Likelihood: Low; and Risk Level: Moderate"@en ;
    rdf:value 0.32 ;
    rdfs:isDefinedBy dpvo-risk: ;
    sw:term_status "accepted"@en ;
    dpvo:hasLikelihood dpvo-risk:LowLikelihood ;
    dpvo:hasRiskLevel dpvo-risk:ModerateRisk ;
    dpvo:hasSeverity dpvo-risk:HighSeverity .

dpvo-risk:RM5x5S4L3 a owl:NamedIndividual,
        dpvo-risk:RiskMatrix5x5 ;
    rdfs:label "High Risk (RM5x5 S:4 L:3)"@en ;
    dct:created "2022-08-17"^^xsd:date ;
    dct:creator "Harshvardhan J. Pandit"^^xsd:string ;
    dct:description "Node in a 5x5 Risk Matrix with Risk Severity: High; Likelihood: Moderate; and Risk Level: High"@en ;
    rdf:value 0.48 ;
    rdfs:isDefinedBy dpvo-risk: ;
    sw:term_status "accepted"@en ;
    dpvo:hasLikelihood dpvo-risk:ModerateLikelihood ;
    dpvo:hasRiskLevel dpvo-risk:HighRisk ;
    dpvo:hasSeverity dpvo-risk:HighSeverity .

dpvo-risk:RM5x5S4L4 a owl:NamedIndividual,
        dpvo-risk:RiskMatrix5x5 ;
    rdfs:label "Very High Risk (RM5x5 S:4 L:4)"@en ;
    dct:created "2022-08-17"^^xsd:date ;
    dct:creator "Harshvardhan J. Pandit"^^xsd:string ;
    dct:description "Node in a 5x5 Risk Matrix with Risk Severity: High; Likelihood: High; and Risk Level: VeryHigh"@en ;
    rdf:value 0.64 ;
    rdfs:isDefinedBy dpvo-risk: ;
    sw:term_status "accepted"@en ;
    dpvo:hasLikelihood dpvo-risk:HighLikelihood ;
    dpvo:hasRiskLevel dpvo-risk:VeryHighRisk ;
    dpvo:hasSeverity dpvo-risk:HighSeverity .

dpvo-risk:RM5x5S4L5 a owl:NamedIndividual,
        dpvo-risk:RiskMatrix5x5 ;
    rdfs:label "Very High Risk (RM5x5 S:4 L:5)"@en ;
    dct:created "2022-08-17"^^xsd:date ;
    dct:creator "Harshvardhan J. Pandit"^^xsd:string ;
    dct:description "Node in a 5x5 Risk Matrix with Risk Severity: High; Likelihood: VeryHigh; and Risk Level: VeryHigh"@en ;
    rdf:value 0.80 ;
    rdfs:isDefinedBy dpvo-risk: ;
    sw:term_status "accepted"@en ;
    dpvo:hasLikelihood dpvo-risk:VeryHighLikelihood ;
    dpvo:hasRiskLevel dpvo-risk:VeryHighRisk ;
    dpvo:hasSeverity dpvo-risk:HighSeverity .

dpvo-risk:RM5x5S5L1 a owl:NamedIndividual,
        dpvo-risk:RiskMatrix5x5 ;
    rdfs:label "Low Risk (RM5x5 S:5 L:1)"@en ;
    dct:created "2022-08-17"^^xsd:date ;
    dct:creator "Harshvardhan J. Pandit"^^xsd:string ;
    dct:description "Node in a 5x5 Risk Matrix with Risk Severity: VeryHigh; Likelihood: VeryLow; and Risk Level: Low"@en ;
    rdf:value 0.20 ;
    rdfs:isDefinedBy dpvo-risk: ;
    sw:term_status "accepted"@en ;
    dpvo:hasLikelihood dpvo-risk:VeryLowLikelihood ;
    dpvo:hasRiskLevel dpvo-risk:LowRisk ;
    dpvo:hasSeverity dpvo-risk:VeryHighSeverity .

dpvo-risk:RM5x5S5L2 a owl:NamedIndividual,
        dpvo-risk:RiskMatrix5x5 ;
    rdfs:label "High Risk (RM5x5 S:5 L:2)"@en ;
    dct:created "2022-08-17"^^xsd:date ;
    dct:creator "Harshvardhan J. Pandit"^^xsd:string ;
    dct:description "Node in a 5x5 Risk Matrix with Risk Severity: VeryHigh; Likelihood: Low; and Risk Level: High"@en ;
    rdf:value 0.40 ;
    rdfs:isDefinedBy dpvo-risk: ;
    sw:term_status "accepted"@en ;
    dpvo:hasLikelihood dpvo-risk:LowLikelihood ;
    dpvo:hasRiskLevel dpvo-risk:HighRisk ;
    dpvo:hasSeverity dpvo-risk:VeryHighSeverity .

dpvo-risk:RM5x5S5L3 a owl:NamedIndividual,
        dpvo-risk:RiskMatrix5x5 ;
    rdfs:label "High Risk (RM5x5 S:5 L:3)"@en ;
    dct:created "2022-08-17"^^xsd:date ;
    dct:creator "Harshvardhan J. Pandit"^^xsd:string ;
    dct:description "Node in a 5x5 Risk Matrix with Risk Severity: VeryHigh; Likelihood: Moderate; and Risk Level: High"@en ;
    rdf:value 0.60 ;
    rdfs:isDefinedBy dpvo-risk: ;
    sw:term_status "accepted"@en ;
    dpvo:hasLikelihood dpvo-risk:ModerateLikelihood ;
    dpvo:hasRiskLevel dpvo-risk:HighRisk ;
    dpvo:hasSeverity dpvo-risk:VeryHighSeverity .

dpvo-risk:RM5x5S5L4 a owl:NamedIndividual,
        dpvo-risk:RiskMatrix5x5 ;
    rdfs:label "Very High Risk (RM5x5 S:5 L:4)"@en ;
    dct:created "2022-08-17"^^xsd:date ;
    dct:creator "Harshvardhan J. Pandit"^^xsd:string ;
    dct:description "Node in a 5x5 Risk Matrix with Risk Severity: VeryHigh; Likelihood: High; and Risk Level: VeryHigh"@en ;
    rdf:value 0.80 ;
    rdfs:isDefinedBy dpvo-risk: ;
    sw:term_status "accepted"@en ;
    dpvo:hasLikelihood dpvo-risk:HighLikelihood ;
    dpvo:hasRiskLevel dpvo-risk:VeryHighRisk ;
    dpvo:hasSeverity dpvo-risk:VeryHighSeverity .

dpvo-risk:RM5x5S5L5 a owl:NamedIndividual,
        dpvo-risk:RiskMatrix5x5 ;
    rdfs:label "Very High Risk (RM5x5 S:5 L:5)"@en ;
    dct:created "2022-08-17"^^xsd:date ;
    dct:creator "Harshvardhan J. Pandit"^^xsd:string ;
    dct:description "Node in a 5x5 Risk Matrix with Risk Severity: VeryHigh; Likelihood: VeryHigh; and Risk Level: VeryHigh"@en ;
    rdf:value 1.00 ;
    rdfs:isDefinedBy dpvo-risk: ;
    sw:term_status "accepted"@en ;
    dpvo:hasLikelihood dpvo-risk:VeryHighLikelihood ;
    dpvo:hasRiskLevel dpvo-risk:VeryHighRisk ;
    dpvo:hasSeverity dpvo-risk:VeryHighSeverity .

dpvo-risk:RM7x7S1L1 a owl:NamedIndividual,
        dpvo-risk:RiskMatrix7x7 ;
    rdfs:label "Extremely Low Risk (RM7x7 S:1 L:1)"@en ;
    dct:created "2022-08-17"^^xsd:date ;
    dct:creator "Harshvardhan J. Pandit"^^xsd:string ;
    dct:description "Node in a 7x7 Risk Matrix with Risk Severity: ExtremelyLow; Likelihood: ExtremelyLow; and Risk Level: ExtremelyLow"@en ;
    rdf:value 0.02 ;
    rdfs:isDefinedBy dpvo-risk: ;
    sw:term_status "accepted"@en ;
    dpvo:hasLikelihood dpvo-risk:ExtremelyLowLikelihood ;
    dpvo:hasRiskLevel dpvo-risk:ExtremelyLowRisk ;
    dpvo:hasSeverity dpvo-risk:ExtremelyLowSeverity .

dpvo-risk:RM7x7S1L2 a owl:NamedIndividual,
        dpvo-risk:RiskMatrix7x7 ;
    rdfs:label "Extremely Low Risk (RM7x7 S:1 L:2)"@en ;
    dct:created "2022-08-17"^^xsd:date ;
    dct:creator "Harshvardhan J. Pandit"^^xsd:string ;
    dct:description "Node in a 7x7 Risk Matrix with Risk Severity: ExtremelyLow; Likelihood: VeryLow; and Risk Level: ExtremelyLow"@en ;
    rdf:value 0.04 ;
    rdfs:isDefinedBy dpvo-risk: ;
    sw:term_status "accepted"@en ;
    dpvo:hasLikelihood dpvo-risk:VeryLowLikelihood ;
    dpvo:hasRiskLevel dpvo-risk:ExtremelyLowRisk ;
    dpvo:hasSeverity dpvo-risk:ExtremelyLowSeverity .

dpvo-risk:RM7x7S1L3 a owl:NamedIndividual,
        dpvo-risk:RiskMatrix7x7 ;
    rdfs:label "Extremely Low Risk (RM7x7 S:1 L:3)"@en ;
    dct:created "2022-08-17"^^xsd:date ;
    dct:creator "Harshvardhan J. Pandit"^^xsd:string ;
    dct:description "Node in a 7x7 Risk Matrix with Risk Severity: ExtremelyLow; Likelihood: Low; and Risk Level: ExtremelyLow"@en ;
    rdf:value 0.06 ;
    rdfs:isDefinedBy dpvo-risk: ;
    sw:term_status "accepted"@en ;
    dpvo:hasLikelihood dpvo-risk:LowLikelihood ;
    dpvo:hasRiskLevel dpvo-risk:ExtremelyLowRisk ;
    dpvo:hasSeverity dpvo-risk:ExtremelyLowSeverity .

dpvo-risk:RM7x7S1L4 a owl:NamedIndividual,
        dpvo-risk:RiskMatrix7x7 ;
    rdfs:label "Very Low Risk (RM7x7 S:1 L:4)"@en ;
    dct:created "2022-08-17"^^xsd:date ;
    dct:creator "Harshvardhan J. Pandit"^^xsd:string ;
    dct:description "Node in a 7x7 Risk Matrix with Risk Severity: ExtremelyLow; Likelihood: Moderate; and Risk Level: VeryLow"@en ;
    rdf:value 0.08 ;
    rdfs:isDefinedBy dpvo-risk: ;
    sw:term_status "accepted"@en ;
    dpvo:hasLikelihood dpvo-risk:ModerateLikelihood ;
    dpvo:hasRiskLevel dpvo-risk:VeryLowRisk ;
    dpvo:hasSeverity dpvo-risk:ExtremelyLowSeverity .

dpvo-risk:RM7x7S1L5 a owl:NamedIndividual,
        dpvo-risk:RiskMatrix7x7 ;
    rdfs:label "Very Low Risk (RM7x7 S:1 L:5)"@en ;
    dct:created "2022-08-17"^^xsd:date ;
    dct:creator "Harshvardhan J. Pandit"^^xsd:string ;
    dct:description "Node in a 7x7 Risk Matrix with Risk Severity: ExtremelyLow; Likelihood: High; and Risk Level: VeryLow"@en ;
    rdf:value 0.10 ;
    rdfs:isDefinedBy dpvo-risk: ;
    sw:term_status "accepted"@en ;
    dpvo:hasLikelihood dpvo-risk:HighLikelihood ;
    dpvo:hasRiskLevel dpvo-risk:VeryLowRisk ;
    dpvo:hasSeverity dpvo-risk:ExtremelyLowSeverity .

dpvo-risk:RM7x7S1L6 a owl:NamedIndividual,
        dpvo-risk:RiskMatrix7x7 ;
    rdfs:label "Very Low Risk (RM7x7 S:1 L:6)"@en ;
    dct:created "2022-08-17"^^xsd:date ;
    dct:creator "Harshvardhan J. Pandit"^^xsd:string ;
    dct:description "Node in a 7x7 Risk Matrix with Risk Severity: ExtremelyLow; Likelihood: VeryHigh; and Risk Level: VeryLow"@en ;
    rdf:value 0.12 ;
    rdfs:isDefinedBy dpvo-risk: ;
    sw:term_status "accepted"@en ;
    dpvo:hasLikelihood dpvo-risk:VeryHighLikelihood ;
    dpvo:hasRiskLevel dpvo-risk:VeryLowRisk ;
    dpvo:hasSeverity dpvo-risk:ExtremelyLowSeverity .

dpvo-risk:RM7x7S1L7 a owl:NamedIndividual,
        dpvo-risk:RiskMatrix7x7 ;
    rdfs:label "Low Risk (RM7x7 S:1 L:7)"@en ;
    dct:created "2022-08-17"^^xsd:date ;
    dct:creator "Harshvardhan J. Pandit"^^xsd:string ;
    dct:description "Node in a 7x7 Risk Matrix with Risk Severity: ExtremelyLow; Likelihood: ExtremelyHigh; and Risk Level: Low"@en ;
    rdf:value 0.14 ;
    rdfs:isDefinedBy dpvo-risk: ;
    sw:term_status "accepted"@en ;
    dpvo:hasLikelihood dpvo-risk:ExtremelyHighLikelihood ;
    dpvo:hasRiskLevel dpvo-risk:LowRisk ;
    dpvo:hasSeverity dpvo-risk:ExtremelyLowSeverity .

dpvo-risk:RM7x7S2L1 a owl:NamedIndividual,
        dpvo-risk:RiskMatrix7x7 ;
    rdfs:label "Extremely Low Risk (RM7x7 S:2 L:1)"@en ;
    dct:created "2022-08-17"^^xsd:date ;
    dct:creator "Harshvardhan J. Pandit"^^xsd:string ;
    dct:description "Node in a 7x7 Risk Matrix with Risk Severity: VeryLow; Likelihood: ExtremelyLow; and Risk Level: ExtremelyLow"@en ;
    rdf:value 0.04 ;
    rdfs:isDefinedBy dpvo-risk: ;
    sw:term_status "accepted"@en ;
    dpvo:hasLikelihood dpvo-risk:ExtremelyLowLikelihood ;
    dpvo:hasRiskLevel dpvo-risk:ExtremelyLowRisk ;
    dpvo:hasSeverity dpvo-risk:VeryLowSeverity .

dpvo-risk:RM7x7S2L2 a owl:NamedIndividual,
        dpvo-risk:RiskMatrix7x7 ;
    rdfs:label "Extremely Low Risk (RM7x7 S:2 L:2)"@en ;
    dct:created "2022-08-17"^^xsd:date ;
    dct:creator "Harshvardhan J. Pandit"^^xsd:string ;
    dct:description "Node in a 7x7 Risk Matrix with Risk Severity: VeryLow; Likelihood: VeryLow; and Risk Level: ExtremelyLow"@en ;
    rdf:value 0.08 ;
    rdfs:isDefinedBy dpvo-risk: ;
    sw:term_status "accepted"@en ;
    dpvo:hasLikelihood dpvo-risk:VeryLowLikelihood ;
    dpvo:hasRiskLevel dpvo-risk:ExtremelyLowRisk ;
    dpvo:hasSeverity dpvo-risk:VeryLowSeverity .

dpvo-risk:RM7x7S2L3 a owl:NamedIndividual,
        dpvo-risk:RiskMatrix7x7 ;
    rdfs:label "Very Low Risk (RM7x7 S:2 L:3)"@en ;
    dct:created "2022-08-17"^^xsd:date ;
    dct:creator "Harshvardhan J. Pandit"^^xsd:string ;
    dct:description "Node in a 7x7 Risk Matrix with Risk Severity: VeryLow; Likelihood: Low; and Risk Level: VeryLow"@en ;
    rdf:value 0.12 ;
    rdfs:isDefinedBy dpvo-risk: ;
    sw:term_status "accepted"@en ;
    dpvo:hasLikelihood dpvo-risk:LowLikelihood ;
    dpvo:hasRiskLevel dpvo-risk:VeryLowRisk ;
    dpvo:hasSeverity dpvo-risk:VeryLowSeverity .

dpvo-risk:RM7x7S2L4 a owl:NamedIndividual,
        dpvo-risk:RiskMatrix7x7 ;
    rdfs:label "Low Risk (RM7x7 S:2 L:4)"@en ;
    dct:created "2022-08-17"^^xsd:date ;
    dct:creator "Harshvardhan J. Pandit"^^xsd:string ;
    dct:description "Node in a 7x7 Risk Matrix with Risk Severity: VeryLow; Likelihood: Moderate; and Risk Level: Low"@en ;
    rdf:value 0.16 ;
    rdfs:isDefinedBy dpvo-risk: ;
    sw:term_status "accepted"@en ;
    dpvo:hasLikelihood dpvo-risk:ModerateLikelihood ;
    dpvo:hasRiskLevel dpvo-risk:LowRisk ;
    dpvo:hasSeverity dpvo-risk:VeryLowSeverity .

dpvo-risk:RM7x7S2L5 a owl:NamedIndividual,
        dpvo-risk:RiskMatrix7x7 ;
    rdfs:label "Low Risk (RM7x7 S:2 L:5)"@en ;
    dct:created "2022-08-17"^^xsd:date ;
    dct:creator "Harshvardhan J. Pandit"^^xsd:string ;
    dct:description "Node in a 7x7 Risk Matrix with Risk Severity: VeryLow; Likelihood: High; and Risk Level: Low"@en ;
    rdf:value 0.20 ;
    rdfs:isDefinedBy dpvo-risk: ;
    sw:term_status "accepted"@en ;
    dpvo:hasLikelihood dpvo-risk:HighLikelihood ;
    dpvo:hasRiskLevel dpvo-risk:LowRisk ;
    dpvo:hasSeverity dpvo-risk:VeryLowSeverity .

dpvo-risk:RM7x7S2L6 a owl:NamedIndividual,
        dpvo-risk:RiskMatrix7x7 ;
    rdfs:label "Moderate Risk (RM7x7 S:2 L:6)"@en ;
    dct:created "2022-08-17"^^xsd:date ;
    dct:creator "Harshvardhan J. Pandit"^^xsd:string ;
    dct:description "Node in a 7x7 Risk Matrix with Risk Severity: VeryLow; Likelihood: VeryHigh; and Risk Level: Moderate"@en ;
    rdf:value 0.24 ;
    rdfs:isDefinedBy dpvo-risk: ;
    sw:term_status "accepted"@en ;
    dpvo:hasLikelihood dpvo-risk:VeryHighLikelihood ;
    dpvo:hasRiskLevel dpvo-risk:ModerateRisk ;
    dpvo:hasSeverity dpvo-risk:VeryLowSeverity .

dpvo-risk:RM7x7S2L7 a owl:NamedIndividual,
        dpvo-risk:RiskMatrix7x7 ;
    rdfs:label "Moderate Risk (RM7x7 S:2 L:7)"@en ;
    dct:created "2022-08-17"^^xsd:date ;
    dct:creator "Harshvardhan J. Pandit"^^xsd:string ;
    dct:description "Node in a 7x7 Risk Matrix with Risk Severity: VeryLow; Likelihood: ExtremelyHigh; and Risk Level: Moderate"@en ;
    rdf:value 0.29 ;
    rdfs:isDefinedBy dpvo-risk: ;
    sw:term_status "accepted"@en ;
    dpvo:hasLikelihood dpvo-risk:ExtremelyHighLikelihood ;
    dpvo:hasRiskLevel dpvo-risk:ModerateRisk ;
    dpvo:hasSeverity dpvo-risk:VeryLowSeverity .

dpvo-risk:RM7x7S3L1 a owl:NamedIndividual,
        dpvo-risk:RiskMatrix7x7 ;
    rdfs:label "Extremely Low Risk (RM7x7 S:3 L:1)"@en ;
    dct:created "2022-08-17"^^xsd:date ;
    dct:creator "Harshvardhan J. Pandit"^^xsd:string ;
    dct:description "Node in a 7x7 Risk Matrix with Risk Severity: Low; Likelihood: ExtremelyLow; and Risk Level: ExtremelyLow"@en ;
    rdf:value 0.06 ;
    rdfs:isDefinedBy dpvo-risk: ;
    sw:term_status "accepted"@en ;
    dpvo:hasLikelihood dpvo-risk:ExtremelyLowLikelihood ;
    dpvo:hasRiskLevel dpvo-risk:ExtremelyLowRisk ;
    dpvo:hasSeverity dpvo-risk:LowSeverity .

dpvo-risk:RM7x7S3L2 a owl:NamedIndividual,
        dpvo-risk:RiskMatrix7x7 ;
    rdfs:label "Very Low Risk (RM7x7 S:3 L:2)"@en ;
    dct:created "2022-08-17"^^xsd:date ;
    dct:creator "Harshvardhan J. Pandit"^^xsd:string ;
    dct:description "Node in a 7x7 Risk Matrix with Risk Severity: Low; Likelihood: VeryLow; and Risk Level: VeryLow"@en ;
    rdf:value 0.12 ;
    rdfs:isDefinedBy dpvo-risk: ;
    sw:term_status "accepted"@en ;
    dpvo:hasLikelihood dpvo-risk:VeryLowLikelihood ;
    dpvo:hasRiskLevel dpvo-risk:VeryLowRisk ;
    dpvo:hasSeverity dpvo-risk:LowSeverity .

dpvo-risk:RM7x7S3L3 a owl:NamedIndividual,
        dpvo-risk:RiskMatrix7x7 ;
    rdfs:label "Low Risk (RM7x7 S:3 L:3)"@en ;
    dct:created "2022-08-17"^^xsd:date ;
    dct:creator "Harshvardhan J. Pandit"^^xsd:string ;
    dct:description "Node in a 7x7 Risk Matrix with Risk Severity: Low; Likelihood: Low; and Risk Level: Low"@en ;
    rdf:value 0.18 ;
    rdfs:isDefinedBy dpvo-risk: ;
    sw:term_status "accepted"@en ;
    dpvo:hasLikelihood dpvo-risk:LowLikelihood ;
    dpvo:hasRiskLevel dpvo-risk:LowRisk ;
    dpvo:hasSeverity dpvo-risk:LowSeverity .

dpvo-risk:RM7x7S3L4 a owl:NamedIndividual,
        dpvo-risk:RiskMatrix7x7 ;
    rdfs:label "Moderate Risk (RM7x7 S:3 L:4)"@en ;
    dct:created "2022-08-17"^^xsd:date ;
    dct:creator "Harshvardhan J. Pandit"^^xsd:string ;
    dct:description "Node in a 7x7 Risk Matrix with Risk Severity: Low; Likelihood: Moderate; and Risk Level: Moderate"@en ;
    rdf:value 0.24 ;
    rdfs:isDefinedBy dpvo-risk: ;
    sw:term_status "accepted"@en ;
    dpvo:hasLikelihood dpvo-risk:ModerateLikelihood ;
    dpvo:hasRiskLevel dpvo-risk:ModerateRisk ;
    dpvo:hasSeverity dpvo-risk:LowSeverity .

dpvo-risk:RM7x7S3L5 a owl:NamedIndividual,
        dpvo-risk:RiskMatrix7x7 ;
    rdfs:label "High Risk (RM7x7 S:3 L:5)"@en ;
    dct:created "2022-08-17"^^xsd:date ;
    dct:creator "Harshvardhan J. Pandit"^^xsd:string ;
    dct:description "Node in a 7x7 Risk Matrix with Risk Severity: Low; Likelihood: High; and Risk Level: High"@en ;
    rdf:value 0.31 ;
    rdfs:isDefinedBy dpvo-risk: ;
    sw:term_status "accepted"@en ;
    dpvo:hasLikelihood dpvo-risk:HighLikelihood ;
    dpvo:hasRiskLevel dpvo-risk:HighRisk ;
    dpvo:hasSeverity dpvo-risk:LowSeverity .

dpvo-risk:RM7x7S3L6 a owl:NamedIndividual,
        dpvo-risk:RiskMatrix7x7 ;
    rdfs:label "High Risk (RM7x7 S:3 L:6)"@en ;
    dct:created "2022-08-17"^^xsd:date ;
    dct:creator "Harshvardhan J. Pandit"^^xsd:string ;
    dct:description "Node in a 7x7 Risk Matrix with Risk Severity: Low; Likelihood: VeryHigh; and Risk Level: High"@en ;
    rdf:value 0.37 ;
    rdfs:isDefinedBy dpvo-risk: ;
    sw:term_status "accepted"@en ;
    dpvo:hasLikelihood dpvo-risk:VeryHighLikelihood ;
    dpvo:hasRiskLevel dpvo-risk:HighRisk ;
    dpvo:hasSeverity dpvo-risk:LowSeverity .

dpvo-risk:RM7x7S3L7 a owl:NamedIndividual,
        dpvo-risk:RiskMatrix7x7 ;
    rdfs:label "Very High Risk (RM7x7 S:3 L:7)"@en ;
    dct:created "2022-08-17"^^xsd:date ;
    dct:creator "Harshvardhan J. Pandit"^^xsd:string ;
    dct:description "Node in a 7x7 Risk Matrix with Risk Severity: Low; Likelihood: ExtremelyHigh; and Risk Level: VeryHigh"@en ;
    rdf:value 0.43 ;
    rdfs:isDefinedBy dpvo-risk: ;
    sw:term_status "accepted"@en ;
    dpvo:hasLikelihood dpvo-risk:ExtremelyHighLikelihood ;
    dpvo:hasRiskLevel dpvo-risk:VeryHighRisk ;
    dpvo:hasSeverity dpvo-risk:LowSeverity .

dpvo-risk:RM7x7S4L1 a owl:NamedIndividual,
        dpvo-risk:RiskMatrix7x7 ;
    rdfs:label "Extremely Low Risk (RM7x7 S:4 L:1)"@en ;
    dct:created "2022-08-17"^^xsd:date ;
    dct:creator "Harshvardhan J. Pandit"^^xsd:string ;
    dct:description "Node in a 7x7 Risk Matrix with Risk Severity: Moderate; Likelihood: ExtremelyLow; and Risk Level: ExtremelyLow"@en ;
    rdf:value 0.08 ;
    rdfs:isDefinedBy dpvo-risk: ;
    sw:term_status "accepted"@en ;
    dpvo:hasLikelihood dpvo-risk:ExtremelyLowLikelihood ;
    dpvo:hasRiskLevel dpvo-risk:ExtremelyLowRisk ;
    dpvo:hasSeverity dpvo-risk:ModerateSeverity .

dpvo-risk:RM7x7S4L2 a owl:NamedIndividual,
        dpvo-risk:RiskMatrix7x7 ;
    rdfs:label "Low Risk (RM7x7 S:4 L:2)"@en ;
    dct:created "2022-08-17"^^xsd:date ;
    dct:creator "Harshvardhan J. Pandit"^^xsd:string ;
    dct:description "Node in a 7x7 Risk Matrix with Risk Severity: Moderate; Likelihood: VeryLow; and Risk Level: Low"@en ;
    rdf:value 0.16 ;
    rdfs:isDefinedBy dpvo-risk: ;
    sw:term_status "accepted"@en ;
    dpvo:hasLikelihood dpvo-risk:VeryLowLikelihood ;
    dpvo:hasRiskLevel dpvo-risk:LowRisk ;
    dpvo:hasSeverity dpvo-risk:ModerateSeverity .

dpvo-risk:RM7x7S4L3 a owl:NamedIndividual,
        dpvo-risk:RiskMatrix7x7 ;
    rdfs:label "Moderate Risk (RM7x7 S:4 L:3)"@en ;
    dct:created "2022-08-17"^^xsd:date ;
    dct:creator "Harshvardhan J. Pandit"^^xsd:string ;
    dct:description "Node in a 7x7 Risk Matrix with Risk Severity: Moderate; Likelihood: Low; and Risk Level: Moderate"@en ;
    rdf:value 0.24 ;
    rdfs:isDefinedBy dpvo-risk: ;
    sw:term_status "accepted"@en ;
    dpvo:hasLikelihood dpvo-risk:LowLikelihood ;
    dpvo:hasRiskLevel dpvo-risk:ModerateRisk ;
    dpvo:hasSeverity dpvo-risk:ModerateSeverity .

dpvo-risk:RM7x7S4L4 a owl:NamedIndividual,
        dpvo-risk:RiskMatrix7x7 ;
    rdfs:label "High Risk (RM7x7 S:4 L:4)"@en ;
    dct:created "2022-08-17"^^xsd:date ;
    dct:creator "Harshvardhan J. Pandit"^^xsd:string ;
    dct:description "Node in a 7x7 Risk Matrix with Risk Severity: Moderate; Likelihood: Moderate; and Risk Level: High"@en ;
    rdf:value 0.33 ;
    rdfs:isDefinedBy dpvo-risk: ;
    sw:term_status "accepted"@en ;
    dpvo:hasLikelihood dpvo-risk:ModerateLikelihood ;
    dpvo:hasRiskLevel dpvo-risk:HighRisk ;
    dpvo:hasSeverity dpvo-risk:ModerateSeverity .

dpvo-risk:RM7x7S4L5 a owl:NamedIndividual,
        dpvo-risk:RiskMatrix7x7 ;
    rdfs:label "High Risk (RM7x7 S:4 L:5)"@en ;
    dct:created "2022-08-17"^^xsd:date ;
    dct:creator "Harshvardhan J. Pandit"^^xsd:string ;
    dct:description "Node in a 7x7 Risk Matrix with Risk Severity: Moderate; Likelihood: High; and Risk Level: High"@en ;
    rdf:value 0.41 ;
    rdfs:isDefinedBy dpvo-risk: ;
    sw:term_status "accepted"@en ;
    dpvo:hasLikelihood dpvo-risk:HighLikelihood ;
    dpvo:hasRiskLevel dpvo-risk:HighRisk ;
    dpvo:hasSeverity dpvo-risk:ModerateSeverity .

dpvo-risk:RM7x7S4L6 a owl:NamedIndividual,
        dpvo-risk:RiskMatrix7x7 ;
    rdfs:label "Very High Risk (RM7x7 S:4 L:6)"@en ;
    dct:created "2022-08-17"^^xsd:date ;
    dct:creator "Harshvardhan J. Pandit"^^xsd:string ;
    dct:description "Node in a 7x7 Risk Matrix with Risk Severity: Moderate; Likelihood: VeryHigh; and Risk Level: VeryHigh"@en ;
    rdf:value 0.49 ;
    rdfs:isDefinedBy dpvo-risk: ;
    sw:term_status "accepted"@en ;
    dpvo:hasLikelihood dpvo-risk:VeryHighLikelihood ;
    dpvo:hasRiskLevel dpvo-risk:VeryHighRisk ;
    dpvo:hasSeverity dpvo-risk:ModerateSeverity .

dpvo-risk:RM7x7S4L7 a owl:NamedIndividual,
        dpvo-risk:RiskMatrix7x7 ;
    rdfs:label "Very High Risk (RM7x7 S:4 L:7)"@en ;
    dct:created "2022-08-17"^^xsd:date ;
    dct:creator "Harshvardhan J. Pandit"^^xsd:string ;
    dct:description "Node in a 7x7 Risk Matrix with Risk Severity: Moderate; Likelihood: ExtremelyHigh; and Risk Level: VeryHigh"@en ;
    rdf:value 0.57 ;
    rdfs:isDefinedBy dpvo-risk: ;
    sw:term_status "accepted"@en ;
    dpvo:hasLikelihood dpvo-risk:ExtremelyHighLikelihood ;
    dpvo:hasRiskLevel dpvo-risk:VeryHighRisk ;
    dpvo:hasSeverity dpvo-risk:ModerateSeverity .

dpvo-risk:RM7x7S5L1 a owl:NamedIndividual,
        dpvo-risk:RiskMatrix7x7 ;
    rdfs:label "Very Low Risk (RM7x7 S:5 L:1)"@en ;
    dct:created "2022-08-17"^^xsd:date ;
    dct:creator "Harshvardhan J. Pandit"^^xsd:string ;
    dct:description "Node in a 7x7 Risk Matrix with Risk Severity: High; Likelihood: ExtremelyLow; and Risk Level: VeryLow"@en ;
    rdf:value 0.10 ;
    rdfs:isDefinedBy dpvo-risk: ;
    sw:term_status "accepted"@en ;
    dpvo:hasLikelihood dpvo-risk:ExtremelyLowLikelihood ;
    dpvo:hasRiskLevel dpvo-risk:VeryLowRisk ;
    dpvo:hasSeverity dpvo-risk:HighSeverity .

dpvo-risk:RM7x7S5L2 a owl:NamedIndividual,
        dpvo-risk:RiskMatrix7x7 ;
    rdfs:label "Low Risk (RM7x7 S:5 L:2)"@en ;
    dct:created "2022-08-17"^^xsd:date ;
    dct:creator "Harshvardhan J. Pandit"^^xsd:string ;
    dct:description "Node in a 7x7 Risk Matrix with Risk Severity: High; Likelihood: VeryLow; and Risk Level: Low"@en ;
    rdf:value 0.20 ;
    rdfs:isDefinedBy dpvo-risk: ;
    sw:term_status "accepted"@en ;
    dpvo:hasLikelihood dpvo-risk:VeryLowLikelihood ;
    dpvo:hasRiskLevel dpvo-risk:LowRisk ;
    dpvo:hasSeverity dpvo-risk:HighSeverity .

dpvo-risk:RM7x7S5L3 a owl:NamedIndividual,
        dpvo-risk:RiskMatrix7x7 ;
    rdfs:label "Moderate Risk (RM7x7 S:5 L:3)"@en ;
    dct:created "2022-08-17"^^xsd:date ;
    dct:creator "Harshvardhan J. Pandit"^^xsd:string ;
    dct:description "Node in a 7x7 Risk Matrix with Risk Severity: High; Likelihood: Low; and Risk Level: Moderate"@en ;
    rdf:value 0.31 ;
    rdfs:isDefinedBy dpvo-risk: ;
    sw:term_status "accepted"@en ;
    dpvo:hasLikelihood dpvo-risk:LowLikelihood ;
    dpvo:hasRiskLevel dpvo-risk:ModerateRisk ;
    dpvo:hasSeverity dpvo-risk:HighSeverity .

dpvo-risk:RM7x7S5L4 a owl:NamedIndividual,
        dpvo-risk:RiskMatrix7x7 ;
    rdfs:label "High Risk (RM7x7 S:5 L:4)"@en ;
    dct:created "2022-08-17"^^xsd:date ;
    dct:creator "Harshvardhan J. Pandit"^^xsd:string ;
    dct:description "Node in a 7x7 Risk Matrix with Risk Severity: High; Likelihood: Moderate; and Risk Level: High"@en ;
    rdf:value 0.41 ;
    rdfs:isDefinedBy dpvo-risk: ;
    sw:term_status "accepted"@en ;
    dpvo:hasLikelihood dpvo-risk:ModerateLikelihood ;
    dpvo:hasRiskLevel dpvo-risk:HighRisk ;
    dpvo:hasSeverity dpvo-risk:HighSeverity .

dpvo-risk:RM7x7S5L5 a owl:NamedIndividual,
        dpvo-risk:RiskMatrix7x7 ;
    rdfs:label "Very High Risk (RM7x7 S:5 L:5)"@en ;
    dct:created "2022-08-17"^^xsd:date ;
    dct:creator "Harshvardhan J. Pandit"^^xsd:string ;
    dct:description "Node in a 7x7 Risk Matrix with Risk Severity: High; Likelihood: High; and Risk Level: VeryHigh"@en ;
    rdf:value 0.51 ;
    rdfs:isDefinedBy dpvo-risk: ;
    sw:term_status "accepted"@en ;
    dpvo:hasLikelihood dpvo-risk:HighLikelihood ;
    dpvo:hasRiskLevel dpvo-risk:VeryHighRisk ;
    dpvo:hasSeverity dpvo-risk:HighSeverity .

dpvo-risk:RM7x7S5L6 a owl:NamedIndividual,
        dpvo-risk:RiskMatrix7x7 ;
    rdfs:label "Extremely High Risk (RM7x7 S:5 L:6)"@en ;
    dct:created "2022-08-17"^^xsd:date ;
    dct:creator "Harshvardhan J. Pandit"^^xsd:string ;
    dct:description "Node in a 7x7 Risk Matrix with Risk Severity: High; Likelihood: VeryHigh; and Risk Level: ExtremelyHigh"@en ;
    rdf:value 0.61 ;
    rdfs:isDefinedBy dpvo-risk: ;
    sw:term_status "accepted"@en ;
    dpvo:hasLikelihood dpvo-risk:VeryHighLikelihood ;
    dpvo:hasRiskLevel dpvo-risk:ExtremelyHighRisk ;
    dpvo:hasSeverity dpvo-risk:HighSeverity .

dpvo-risk:RM7x7S5L7 a owl:NamedIndividual,
        dpvo-risk:RiskMatrix7x7 ;
    rdfs:label "Extremely High Risk (RM7x7 S:5 L:7)"@en ;
    dct:created "2022-08-17"^^xsd:date ;
    dct:creator "Harshvardhan J. Pandit"^^xsd:string ;
    dct:description "Node in a 7x7 Risk Matrix with Risk Severity: High; Likelihood: ExtremelyHigh; and Risk Level: ExtremelyHigh"@en ;
    rdf:value 0.71 ;
    rdfs:isDefinedBy dpvo-risk: ;
    sw:term_status "accepted"@en ;
    dpvo:hasLikelihood dpvo-risk:ExtremelyHighLikelihood ;
    dpvo:hasRiskLevel dpvo-risk:ExtremelyHighRisk ;
    dpvo:hasSeverity dpvo-risk:HighSeverity .

dpvo-risk:RM7x7S6L1 a owl:NamedIndividual,
        dpvo-risk:RiskMatrix7x7 ;
    rdfs:label "Very Low Risk (RM7x7 S:6 L:1)"@en ;
    dct:created "2022-08-17"^^xsd:date ;
    dct:creator "Harshvardhan J. Pandit"^^xsd:string ;
    dct:description "Node in a 7x7 Risk Matrix with Risk Severity: VeryHigh; Likelihood: ExtremelyLow; and Risk Level: VeryLow"@en ;
    rdf:value 0.12 ;
    rdfs:isDefinedBy dpvo-risk: ;
    sw:term_status "accepted"@en ;
    dpvo:hasLikelihood dpvo-risk:ExtremelyLowLikelihood ;
    dpvo:hasRiskLevel dpvo-risk:VeryLowRisk ;
    dpvo:hasSeverity dpvo-risk:VeryHighSeverity .

dpvo-risk:RM7x7S6L2 a owl:NamedIndividual,
        dpvo-risk:RiskMatrix7x7 ;
    rdfs:label "Moderate Risk (RM7x7 S:6 L:2)"@en ;
    dct:created "2022-08-17"^^xsd:date ;
    dct:creator "Harshvardhan J. Pandit"^^xsd:string ;
    dct:description "Node in a 7x7 Risk Matrix with Risk Severity: VeryHigh; Likelihood: VeryLow; and Risk Level: Moderate"@en ;
    rdf:value 0.24 ;
    rdfs:isDefinedBy dpvo-risk: ;
    sw:term_status "accepted"@en ;
    dpvo:hasLikelihood dpvo-risk:VeryLowLikelihood ;
    dpvo:hasRiskLevel dpvo-risk:ModerateRisk ;
    dpvo:hasSeverity dpvo-risk:VeryHighSeverity .

dpvo-risk:RM7x7S6L3 a owl:NamedIndividual,
        dpvo-risk:RiskMatrix7x7 ;
    rdfs:label "High Risk (RM7x7 S:6 L:3)"@en ;
    dct:created "2022-08-17"^^xsd:date ;
    dct:creator "Harshvardhan J. Pandit"^^xsd:string ;
    dct:description "Node in a 7x7 Risk Matrix with Risk Severity: VeryHigh; Likelihood: Low; and Risk Level: High"@en ;
    rdf:value 0.37 ;
    rdfs:isDefinedBy dpvo-risk: ;
    sw:term_status "accepted"@en ;
    dpvo:hasLikelihood dpvo-risk:LowLikelihood ;
    dpvo:hasRiskLevel dpvo-risk:HighRisk ;
    dpvo:hasSeverity dpvo-risk:VeryHighSeverity .

dpvo-risk:RM7x7S6L4 a owl:NamedIndividual,
        dpvo-risk:RiskMatrix7x7 ;
    rdfs:label "Very High Risk (RM7x7 S:6 L:4)"@en ;
    dct:created "2022-08-17"^^xsd:date ;
    dct:creator "Harshvardhan J. Pandit"^^xsd:string ;
    dct:description "Node in a 7x7 Risk Matrix with Risk Severity: VeryHigh; Likelihood: Moderate; and Risk Level: VeryHigh"@en ;
    rdf:value 0.49 ;
    rdfs:isDefinedBy dpvo-risk: ;
    sw:term_status "accepted"@en ;
    dpvo:hasLikelihood dpvo-risk:ModerateLikelihood ;
    dpvo:hasRiskLevel dpvo-risk:VeryHighRisk ;
    dpvo:hasSeverity dpvo-risk:VeryHighSeverity .

dpvo-risk:RM7x7S6L5 a owl:NamedIndividual,
        dpvo-risk:RiskMatrix7x7 ;
    rdfs:label "Very High Risk (RM7x7 S:6 L:5)"@en ;
    dct:created "2022-08-17"^^xsd:date ;
    dct:creator "Harshvardhan J. Pandit"^^xsd:string ;
    dct:description "Node in a 7x7 Risk Matrix with Risk Severity: VeryHigh; Likelihood: High; and Risk Level: VeryHigh"@en ;
    rdf:value 0.61 ;
    rdfs:isDefinedBy dpvo-risk: ;
    sw:term_status "accepted"@en ;
    dpvo:hasLikelihood dpvo-risk:HighLikelihood ;
    dpvo:hasRiskLevel dpvo-risk:VeryHighRisk ;
    dpvo:hasSeverity dpvo-risk:VeryHighSeverity .

dpvo-risk:RM7x7S6L6 a owl:NamedIndividual,
        dpvo-risk:RiskMatrix7x7 ;
    rdfs:label "Extremely High Risk (RM7x7 S:6 L:6)"@en ;
    dct:created "2022-08-17"^^xsd:date ;
    dct:creator "Harshvardhan J. Pandit"^^xsd:string ;
    dct:description "Node in a 7x7 Risk Matrix with Risk Severity: VeryHigh; Likelihood: VeryHigh; and Risk Level: ExtremelyHigh"@en ;
    rdf:value 0.73 ;
    rdfs:isDefinedBy dpvo-risk: ;
    sw:term_status "accepted"@en ;
    dpvo:hasLikelihood dpvo-risk:VeryHighLikelihood ;
    dpvo:hasRiskLevel dpvo-risk:ExtremelyHighRisk ;
    dpvo:hasSeverity dpvo-risk:VeryHighSeverity .

dpvo-risk:RM7x7S6L7 a owl:NamedIndividual,
        dpvo-risk:RiskMatrix7x7 ;
    rdfs:label "Extremely High Risk (RM7x7 S:6 L:7)"@en ;
    dct:created "2022-08-17"^^xsd:date ;
    dct:creator "Harshvardhan J. Pandit"^^xsd:string ;
    dct:description "Node in a 7x7 Risk Matrix with Risk Severity: VeryHigh; Likelihood: ExtremelyHigh; and Risk Level: ExtremelyHigh"@en ;
    rdf:value 0.86 ;
    rdfs:isDefinedBy dpvo-risk: ;
    sw:term_status "accepted"@en ;
    dpvo:hasLikelihood dpvo-risk:ExtremelyHighLikelihood ;
    dpvo:hasRiskLevel dpvo-risk:ExtremelyHighRisk ;
    dpvo:hasSeverity dpvo-risk:VeryHighSeverity .

dpvo-risk:RM7x7S7L1 a owl:NamedIndividual,
        dpvo-risk:RiskMatrix7x7 ;
    rdfs:label "Low Risk (RM7x7 S:7 L:1)"@en ;
    dct:created "2022-08-17"^^xsd:date ;
    dct:creator "Harshvardhan J. Pandit"^^xsd:string ;
    dct:description "Node in a 7x7 Risk Matrix with Risk Severity: ExtremelyHigh; Likelihood: ExtremelyLow; and Risk Level: Low"@en ;
    rdf:value 0.14 ;
    rdfs:isDefinedBy dpvo-risk: ;
    sw:term_status "accepted"@en ;
    dpvo:hasLikelihood dpvo-risk:ExtremelyLowLikelihood ;
    dpvo:hasRiskLevel dpvo-risk:LowRisk ;
    dpvo:hasSeverity dpvo-risk:ExtremelyHighSeverity .

dpvo-risk:RM7x7S7L2 a owl:NamedIndividual,
        dpvo-risk:RiskMatrix7x7 ;
    rdfs:label "Moderate Risk (RM7x7 S:7 L:2)"@en ;
    dct:created "2022-08-17"^^xsd:date ;
    dct:creator "Harshvardhan J. Pandit"^^xsd:string ;
    dct:description "Node in a 7x7 Risk Matrix with Risk Severity: ExtremelyHigh; Likelihood: VeryLow; and Risk Level: Moderate"@en ;
    rdf:value 0.29 ;
    rdfs:isDefinedBy dpvo-risk: ;
    sw:term_status "accepted"@en ;
    dpvo:hasLikelihood dpvo-risk:VeryLowLikelihood ;
    dpvo:hasRiskLevel dpvo-risk:ModerateRisk ;
    dpvo:hasSeverity dpvo-risk:ExtremelyHighSeverity .

dpvo-risk:RM7x7S7L3 a owl:NamedIndividual,
        dpvo-risk:RiskMatrix7x7 ;
    rdfs:label "High Risk (RM7x7 S:7 L:3)"@en ;
    dct:created "2022-08-17"^^xsd:date ;
    dct:creator "Harshvardhan J. Pandit"^^xsd:string ;
    dct:description "Node in a 7x7 Risk Matrix with Risk Severity: ExtremelyHigh; Likelihood: Low; and Risk Level: High"@en ;
    rdf:value 0.43 ;
    rdfs:isDefinedBy dpvo-risk: ;
    sw:term_status "accepted"@en ;
    dpvo:hasLikelihood dpvo-risk:LowLikelihood ;
    dpvo:hasRiskLevel dpvo-risk:HighRisk ;
    dpvo:hasSeverity dpvo-risk:ExtremelyHighSeverity .

dpvo-risk:RM7x7S7L4 a owl:NamedIndividual,
        dpvo-risk:RiskMatrix7x7 ;
    rdfs:label "Very High Risk (RM7x7 S:7 L:4)"@en ;
    dct:created "2022-08-17"^^xsd:date ;
    dct:creator "Harshvardhan J. Pandit"^^xsd:string ;
    dct:description "Node in a 7x7 Risk Matrix with Risk Severity: ExtremelyHigh; Likelihood: Moderate; and Risk Level: VeryHigh"@en ;
    rdf:value 0.57 ;
    rdfs:isDefinedBy dpvo-risk: ;
    sw:term_status "accepted"@en ;
    dpvo:hasLikelihood dpvo-risk:ModerateLikelihood ;
    dpvo:hasRiskLevel dpvo-risk:VeryHighRisk ;
    dpvo:hasSeverity dpvo-risk:ExtremelyHighSeverity .

dpvo-risk:RM7x7S7L5 a owl:NamedIndividual,
        dpvo-risk:RiskMatrix7x7 ;
    rdfs:label "Extremely High Risk (RM7x7 S:7 L:5)"@en ;
    dct:created "2022-08-17"^^xsd:date ;
    dct:creator "Harshvardhan J. Pandit"^^xsd:string ;
    dct:description "Node in a 7x7 Risk Matrix with Risk Severity: ExtremelyHigh; Likelihood: High; and Risk Level: ExtremelyHigh"@en ;
    rdf:value 0.71 ;
    rdfs:isDefinedBy dpvo-risk: ;
    sw:term_status "accepted"@en ;
    dpvo:hasLikelihood dpvo-risk:HighLikelihood ;
    dpvo:hasRiskLevel dpvo-risk:ExtremelyHighRisk ;
    dpvo:hasSeverity dpvo-risk:ExtremelyHighSeverity .

dpvo-risk:RM7x7S7L6 a owl:NamedIndividual,
        dpvo-risk:RiskMatrix7x7 ;
    rdfs:label "Extremely High Risk (RM7x7 S:7 L:6)"@en ;
    dct:created "2022-08-17"^^xsd:date ;
    dct:creator "Harshvardhan J. Pandit"^^xsd:string ;
    dct:description "Node in a 7x7 Risk Matrix with Risk Severity: ExtremelyHigh; Likelihood: VeryHigh; and Risk Level: ExtremelyHigh"@en ;
    rdf:value 0.86 ;
    rdfs:isDefinedBy dpvo-risk: ;
    sw:term_status "accepted"@en ;
    dpvo:hasLikelihood dpvo-risk:VeryHighLikelihood ;
    dpvo:hasRiskLevel dpvo-risk:ExtremelyHighRisk ;
    dpvo:hasSeverity dpvo-risk:ExtremelyHighSeverity .

dpvo-risk:RM7x7S7L7 a owl:NamedIndividual,
        dpvo-risk:RiskMatrix7x7 ;
    rdfs:label "Extremely High Risk (RM7x7 S:7 L:7)"@en ;
    dct:created "2022-08-17"^^xsd:date ;
    dct:creator "Harshvardhan J. Pandit"^^xsd:string ;
    dct:description "Node in a 7x7 Risk Matrix with Risk Severity: ExtremelyHigh; Likelihood: ExtremelyHigh; and Risk Level: ExtremelyHigh"@en ;
    rdf:value 1.00 ;
    rdfs:isDefinedBy dpvo-risk: ;
    sw:term_status "accepted"@en ;
    dpvo:hasLikelihood dpvo-risk:ExtremelyHighLikelihood ;
    dpvo:hasRiskLevel dpvo-risk:ExtremelyHighRisk ;
    dpvo:hasSeverity dpvo-risk:ExtremelyHighSeverity .

dpvo-risk:RansomwareAttack a owl:Class ;
    rdfs:label "RansomwareAttack"@en ;
    dct:created "2022-08-17"^^xsd:date ;
    dct:creator "Harshvardhan J. Pandit"^^xsd:string ;
    dct:description "Ransomware is a type of attack where threat actors take control of a target’s assets and demand a ransom in exchange for the return of the asset’s availability and confidentiality"@en ;
    dct:source <https://www.enisa.europa.eu/publications/enisa-threat-landscape-for-ransomware-attacks>,
        <https://www.iso.org/standard/75281.html> ;
    rdfs:isDefinedBy dpvo-risk: ;
    rdfs:subClassOf dpvo:NonMaterialDamage ;
    sw:term_status "accepted"@en .

dpvo-risk:ReduceLikelihood a owl:Class ;
    rdfs:label "Reduce Likelihood"@en ;
    dct:created "2022-08-22"^^xsd:date ;
    dct:creator "Harshvardhan J. Pandit"^^xsd:string ;
    dct:description "Risk Control that reduces the likelihood of an event"@en ;
    rdfs:isDefinedBy dpvo-risk: ;
    rdfs:subClassOf dpvo:RiskMitigationMeasure ;
    sw:term_status "accepted"@en .

dpvo-risk:ReduceSeverity a owl:Class ;
    rdfs:label "Reduce Severity"@en ;
    dct:created "2022-08-23"^^xsd:date ;
    dct:creator "Harshvardhan J. Pandit"^^xsd:string ;
    dct:description "Risk Control that reduces the severity of an event"@en ;
    rdfs:isDefinedBy dpvo-risk: ;
    rdfs:subClassOf dpvo:RiskMitigationMeasure ;
    sw:term_status "accepted"@en .

dpvo-risk:ReliabilityCentredMaintenance a owl:NamedIndividual,
        dpvo-risk:QualitativeRiskAssessmentTechnique,
        dpvo-risk:QuantitativeRiskAssessmentTechnique ;
    rdfs:label "Reliability Centred Maintenance"@en ;
    dct:created "2022-08-18"^^xsd:date ;
    dct:creator "Harshvardhan J. Pandit"^^xsd:string ;
    dct:description "A risk based assessment used to identify the appropriate maintenance tasks for a system and its components."@en ;
    dct:source <https://www.iso.org/standard/72140.html> ;
    rdfs:isDefinedBy dpvo-risk: ;
    sw:term_status "accepted"@en .

dpvo-risk:RemoteSpying a owl:Class ;
    rdfs:label "Remote Spying"@en ;
    dct:created "2022-08-17"^^xsd:date ;
    dct:creator "Harshvardhan J. Pandit"^^xsd:string ;
    dct:description ""@en ;
    dct:source <https://www.iso.org/standard/75281.html> ;
    rdfs:isDefinedBy dpvo-risk: ;
    rdfs:subClassOf dpvo:NonMaterialDamage ;
    sw:term_status "accepted"@en .

dpvo-risk:RemoveConsequence a owl:Class ;
    rdfs:label "Remove Consequence"@en ;
    dct:created "2022-08-27"^^xsd:date ;
    dct:creator "Harshvardhan J. Pandit"^^xsd:string ;
    dct:description "Risk Control that removes Consequence i.e. prevents it from materialising"@en ;
    rdfs:isDefinedBy dpvo-risk: ;
    rdfs:subClassOf dpvo-risk:ControlConsequence ;
    sw:term_status "accepted"@en .

dpvo-risk:RemoveImpact a owl:Class ;
    rdfs:label "Remove Impact"@en ;
    dct:created "2022-08-28"^^xsd:date ;
    dct:creator "Harshvardhan J. Pandit"^^xsd:string ;
    dct:description "Risk Control that removes Impact i.e. prevents it from materialising"@en ;
    rdfs:isDefinedBy dpvo-risk: ;
    rdfs:subClassOf dpvo-risk:ControlConsequence ;
    sw:term_status "accepted"@en .

dpvo-risk:RemoveSource a owl:Class ;
    rdfs:label "Remove Source"@en ;
    dct:created "2022-08-20"^^xsd:date ;
    dct:creator "Harshvardhan J. Pandit"^^xsd:string ;
    dct:description "Risk Control that removes the risk source"@en ;
    rdfs:isDefinedBy dpvo-risk: ;
    rdfs:subClassOf dpvo-risk:ControlRiskSource ;
    sw:term_status "accepted"@en .

dpvo-risk:ReplacementCosts a owl:Class ;
    rdfs:label "Replacement Costs"@en ;
    dct:created "2022-08-17"^^xsd:date ;
    dct:creator "Harshvardhan J. Pandit"^^xsd:string ;
    dct:description ""@en ;
    dct:source <https://www.iso.org/standard/75281.html> ;
    rdfs:isDefinedBy dpvo-risk: ;
    rdfs:subClassOf dpvo:Detriment ;
    sw:term_status "accepted"@en .

dpvo-risk:ReputationTrustImpact a owl:Class ;
    rdfs:label "Reputation and trust impact"@en ;
    dct:created "2022-08-17"^^xsd:date ;
    dct:creator "Harshvardhan J. Pandit"^^xsd:string ;
    dct:description ""@en ;
    dct:source <https://www.enisa.europa.eu/publications/methodology-for-a-sectoral-cybersecurity-assessment> ;
    rdfs:isDefinedBy dpvo-risk: ;
    rdfs:subClassOf dpvo:Impact ;
    sw:term_status "accepted"@en .

dpvo-risk:RetrievalDeletedData a owl:Class ;
    rdfs:label "Retrieval of Deleted Data"@en ;
    dct:created "2022-08-17"^^xsd:date ;
    dct:creator "Harshvardhan J. Pandit"^^xsd:string ;
    dct:description ""@en ;
    dct:source <https://www.iso.org/standard/75281.html> ;
    rdfs:isDefinedBy dpvo-risk: ;
    rdfs:subClassOf dpvo:Detriment ;
    sw:term_status "accepted"@en .

dpvo-risk:RetrievalDiscardedEquipment a owl:Class ;
    rdfs:label "Retrieval of Discarded Equipment"@en ;
    dct:created "2022-08-17"^^xsd:date ;
    dct:creator "Harshvardhan J. Pandit"^^xsd:string ;
    dct:description ""@en ;
    dct:source <https://www.iso.org/standard/75281.html> ;
    rdfs:isDefinedBy dpvo-risk: ;
    rdfs:subClassOf dpvo:Detriment ;
    sw:term_status "accepted"@en .

dpvo-risk:RiskIndices a owl:NamedIndividual,
        dpvo-risk:QuantitativeRiskAssessmentTechnique ;
    rdfs:label "Risk Indices"@en ;
    dct:created "2022-08-18"^^xsd:date ;
    dct:creator "Harshvardhan J. Pandit"^^xsd:string ;
    dct:description "Rates the significance of risks based on ratings applied to factors which are believed to influence the magnitude of the risk."@en ;
    dct:source <https://www.iso.org/standard/72140.html> ;
    rdfs:isDefinedBy dpvo-risk: ;
    sw:term_status "accepted"@en .

dpvo-risk:RiskRegisters a owl:NamedIndividual,
        dpvo-risk:QualitativeRiskAssessmentTechnique ;
    rdfs:label "Risk Registers"@en ;
    dct:created "2022-08-18"^^xsd:date ;
    dct:creator "Harshvardhan J. Pandit"^^xsd:string ;
    dct:description "A means of recording information about risks and tracking actions."@en ;
    dct:source <https://www.iso.org/standard/72140.html> ;
    rdfs:isDefinedBy dpvo-risk: ;
    sw:term_status "accepted"@en .

dpvo-risk:SCurves a owl:NamedIndividual,
        dpvo-risk:QuantitativeRiskAssessmentTechnique ;
    rdfs:label "S-curves"@en ;
    dct:created "2022-08-18"^^xsd:date ;
    dct:creator "Harshvardhan J. Pandit"^^xsd:string ;
    dct:description "A means of displaying the relationship between consequences and their likelihood plotted as a cumulative distribution function (S-curve)."@en ;
    dct:source <https://www.iso.org/standard/72140.html> ;
    rdfs:isDefinedBy dpvo-risk: ;
    sw:term_status "accepted"@en .

dpvo-risk:SFAIRP a owl:NamedIndividual,
        dpvo-risk:QualitativeRiskAssessmentTechnique,
        dpvo-risk:QuantitativeRiskAssessmentTechnique ;
    rdfs:label "SFAIRP"@en ;
    dct:created "2022-08-18"^^xsd:date ;
    dct:creator "Harshvardhan J. Pandit"^^xsd:string ;
    dct:description "So far as is Resonably Practiceable (ALARP) - A criteria for deciding significance of risk and means of evaluating tolerability of risk"@en ;
    dct:source <https://www.iso.org/standard/72140.html> ;
    rdfs:isDefinedBy dpvo-risk: ;
    sw:term_status "accepted"@en .

dpvo-risk:SWIFT a owl:NamedIndividual,
        dpvo-risk:QualitativeRiskAssessmentTechnique ;
    rdfs:label "Structured \"What If?\" (SWIFT)"@en ;
    dct:created "2022-08-18"^^xsd:date ;
    dct:creator "Harshvardhan J. Pandit"^^xsd:string ;
    dct:description "A simpler form of HAZOP with prompts of \"what if\" to identify deviations from the expected."@en ;
    dct:source <https://www.iso.org/standard/72140.html> ;
    rdfs:isDefinedBy dpvo-risk: ;
    sw:term_status "accepted"@en .

dpvo-risk:Sabotage a owl:Class ;
    rdfs:label "Sabotage"@en ;
    dct:created "2022-08-17"^^xsd:date ;
    dct:creator "Harshvardhan J. Pandit"^^xsd:string ;
    dct:description ""@en ;
    dct:source <https://www.enisa.europa.eu/publications/reference-incident-classification-taxonomy/> ;
    rdfs:isDefinedBy dpvo-risk: ;
    rdfs:subClassOf dpvo:Harm ;
    sw:term_status "accepted"@en .

dpvo-risk:Scam a owl:Class ;
    rdfs:label "Scam"@en ;
    dct:created "2022-08-17"^^xsd:date ;
    dct:creator "Harshvardhan J. Pandit"^^xsd:string ;
    dct:description ""@en ;
    dct:source <https://www.iso.org/standard/75281.html> ;
    rdfs:isDefinedBy dpvo-risk: ;
    rdfs:subClassOf dpvo:Harm ;
    sw:term_status "accepted"@en .

dpvo-risk:ScenarioAnalysis a owl:NamedIndividual,
        dpvo-risk:QualitativeRiskAssessmentTechnique ;
    rdfs:label "Scenario Analysis"@en ;
    dct:created "2022-08-18"^^xsd:date ;
    dct:creator "Harshvardhan J. Pandit"^^xsd:string ;
    dct:description "Identifies possible future scenarios through imagination, extrapolation from the present or modelling. Risk is then considered for each of these scenarios."@en ;
    dct:source <https://www.iso.org/standard/72140.html> ;
    rdfs:isDefinedBy dpvo-risk: ;
    sw:term_status "accepted"@en .

dpvo-risk:SecurityBreach a owl:Class ;
    rdfs:label "Security Breach"@en ;
    dct:created "2022-08-17"^^xsd:date ;
    dct:creator "Harshvardhan J. Pandit"^^xsd:string ;
    dct:description ""@en ;
    dct:source <https://www.iso.org/standard/75281.html> ;
    rdfs:isDefinedBy dpvo-risk: ;
    rdfs:subClassOf dpvo:Consequence ;
    sw:term_status "accepted"@en .

dpvo-risk:ServiceInterruption a owl:Class ;
    rdfs:label "Service Interruption"@en ;
    dct:created "2022-08-17"^^xsd:date ;
    dct:creator "Harshvardhan J. Pandit"^^xsd:string ;
    dct:description ""@en ;
    dct:source <https://www.iso.org/standard/75281.html> ;
    rdfs:isDefinedBy dpvo-risk: ;
    rdfs:subClassOf dpvo:Detriment ;
    sw:term_status "accepted"@en .

dpvo-risk:SexualViolence a owl:Class ;
    rdfs:label "Sexual Violence"@en ;
    dct:created "2022-08-17"^^xsd:date ;
    dct:creator "Harshvardhan J. Pandit"^^xsd:string ;
    dct:description ""@en ;
    dct:source <https://www.enisa.europa.eu/publications/reference-incident-classification-taxonomy/> ;
    rdfs:isDefinedBy dpvo-risk: ;
    rdfs:subClassOf dpvo:Harm ;
    sw:term_status "accepted"@en .

dpvo-risk:ShareRisk a owl:Class ;
    rdfs:label "Share Risk"@en ;
    dct:created "2022-08-29"^^xsd:date ;
    dct:creator "Harshvardhan J. Pandit"^^xsd:string ;
    dct:description "Risk Mitigation Measure that shares Risk e.g. amongst stakeholders"@en ;
    rdfs:isDefinedBy dpvo-risk: ;
    rdfs:subClassOf dpvo:RiskMitigationMeasure ;
    sw:term_status "accepted"@en .

dpvo-risk:SocialDisadvantage a owl:Class ;
    rdfs:label "Social Disadvantage"@en ;
    dct:created "2022-08-19"^^xsd:date ;
    dct:creator "Georg P Krog"^^xsd:string ;
    dct:description ""@en ;
    rdfs:isDefinedBy dpvo-risk: ;
    rdfs:subClassOf dpvo:Impact ;
    sw:term_status "accepted"@en .

dpvo-risk:Spam a owl:Class ;
    rdfs:label "Spam"@en ;
    dct:created "2022-08-17"^^xsd:date ;
    dct:creator "Harshvardhan J. Pandit"^^xsd:string ;
    dct:description ""@en ;
    dct:source <https://www.enisa.europa.eu/publications/reference-incident-classification-taxonomy/> ;
    rdfs:isDefinedBy dpvo-risk: ;
    rdfs:subClassOf dpvo:Harm ;
    sw:term_status "accepted"@en .

dpvo-risk:Spoofing a owl:Class ;
    rdfs:label "Spoofing"@en ;
    dct:created "2022-08-17"^^xsd:date ;
    dct:creator "Harshvardhan J. Pandit"^^xsd:string ;
    dct:description ""@en ;
    dct:source <https://www.iso.org/standard/75281.html> ;
    rdfs:isDefinedBy dpvo-risk: ;
    rdfs:subClassOf dpvo:Harm ;
    sw:term_status "accepted"@en .

dpvo-risk:Spying a owl:Class ;
    rdfs:label "Spying"@en ;
    dct:created "2022-08-17"^^xsd:date ;
    dct:creator "Harshvardhan J. Pandit"^^xsd:string ;
    dct:description ""@en ;
    dct:source <https://www.iso.org/standard/75281.html> ;
    rdfs:isDefinedBy dpvo-risk: ;
    rdfs:subClassOf dpvo:NonMaterialDamage ;
    sw:term_status "accepted"@en .

dpvo-risk:Stalking a owl:Class ;
    rdfs:label "Stalking"@en ;
    dct:created "2022-08-17"^^xsd:date ;
    dct:creator "Harshvardhan J. Pandit"^^xsd:string ;
    dct:description ""@en ;
    dct:source <https://www.iso.org/standard/75281.html> ;
    rdfs:isDefinedBy dpvo-risk: ;
    rdfs:subClassOf dpvo:NonMaterialDamage ;
    sw:term_status "accepted"@en .

dpvo-risk:Surveys a owl:NamedIndividual,
        dpvo-risk:QualitativeRiskAssessmentTechnique ;
    rdfs:label "Surveys"@en ;
    dct:created "2022-08-18"^^xsd:date ;
    dct:creator "Harshvardhan J. Pandit"^^xsd:string ;
    dct:description "Paper- or computer-based questionnaires to elicit views."@en ;
    dct:source <https://www.iso.org/standard/72140.html> ;
    rdfs:isDefinedBy dpvo-risk: ;
    sw:term_status "accepted"@en .

dpvo-risk:SystemFailure a owl:Class ;
    rdfs:label "System Failure"@en ;
    dct:created "2022-08-17"^^xsd:date ;
    dct:creator "Harshvardhan J. Pandit"^^xsd:string ;
    dct:description ""@en ;
    dct:source <https://www.enisa.europa.eu/publications/enisa-threat-landscape-for-ransomware-attacks> ;
    rdfs:isDefinedBy dpvo-risk: ;
    rdfs:subClassOf dpvo:Detriment ;
    sw:term_status "accepted"@en .

dpvo-risk:SystemIntrusion a owl:Class ;
    rdfs:label "System Intrusion"@en ;
    dct:created "2022-08-17"^^xsd:date ;
    dct:creator "Harshvardhan J. Pandit"^^xsd:string ;
    dct:description ""@en ;
    dct:source <https://www.enisa.europa.eu/publications/reference-incident-classification-taxonomy/> ;
    rdfs:isDefinedBy dpvo-risk: ;
    rdfs:subClassOf dpvo:Detriment ;
    sw:term_status "accepted"@en .

dpvo-risk:SystemMalfunction a owl:Class ;
    rdfs:label "System Malfunction"@en ;
    dct:created "2022-08-17"^^xsd:date ;
    dct:creator "Harshvardhan J. Pandit"^^xsd:string ;
    dct:description ""@en ;
    dct:source <https://www.iso.org/standard/75281.html> ;
    rdfs:isDefinedBy dpvo-risk: ;
    rdfs:subClassOf dpvo:Detriment ;
    sw:term_status "accepted"@en .

dpvo-risk:Taxonomies a owl:NamedIndividual,
        dpvo-risk:QualitativeRiskAssessmentTechnique ;
    rdfs:label "Taxonomies"@en ;
    dct:created "2022-08-18"^^xsd:date ;
    dct:creator "Harshvardhan J. Pandit"^^xsd:string ;
    dct:description "A taxonomy based on experience or on concepts and models that can be used to help identify risks or controls."@en ;
    dct:source <https://www.iso.org/standard/72140.html> ;
    rdfs:isDefinedBy dpvo-risk: ;
    sw:term_status "accepted"@en .

dpvo-risk:Terrorism a owl:Class ;
    rdfs:label "Terrorism"@en ;
    dct:created "2022-08-17"^^xsd:date ;
    dct:creator "Harshvardhan J. Pandit"^^xsd:string ;
    dct:description ""@en ;
    dct:source <https://www.iso.org/standard/75281.html> ;
    rdfs:isDefinedBy dpvo-risk: ;
    rdfs:subClassOf dpvo:Harm ;
    sw:term_status "accepted"@en .

dpvo-risk:Theft a owl:Class ;
    rdfs:label "Theft"@en ;
    dct:created "2022-08-17"^^xsd:date ;
    dct:creator "Harshvardhan J. Pandit"^^xsd:string ;
    dct:description ""@en ;
    dct:source <https://www.iso.org/standard/75281.html> ;
    rdfs:isDefinedBy dpvo-risk: ;
    rdfs:subClassOf dpvo:MaterialDamage ;
    sw:term_status "accepted"@en .

dpvo-risk:TheftEquipment a owl:Class ;
    rdfs:label "Theft of Equipment"@en ;
    dct:created "2022-08-17"^^xsd:date ;
    dct:creator "Harshvardhan J. Pandit"^^xsd:string ;
    dct:description ""@en ;
    dct:source <https://www.iso.org/standard/75281.html> ;
    rdfs:isDefinedBy dpvo-risk: ;
    rdfs:subClassOf dpvo:MaterialDamage ;
    sw:term_status "accepted"@en .

dpvo-risk:TheftMedia a owl:Class ;
    rdfs:label "Theft of Media"@en ;
    dct:created "2022-08-17"^^xsd:date ;
    dct:creator "Harshvardhan J. Pandit"^^xsd:string ;
    dct:description ""@en ;
    dct:source <https://www.iso.org/standard/75281.html> ;
    rdfs:isDefinedBy dpvo-risk: ;
    rdfs:subClassOf dpvo:MaterialDamage ;
    sw:term_status "accepted"@en .

dpvo-risk:ThirdPartyOperationDisruption a owl:Class ;
    rdfs:label "Third Party Operation Disruption"@en ;
    dct:created "2022-08-17"^^xsd:date ;
    dct:creator "Harshvardhan J. Pandit"^^xsd:string ;
    dct:description ""@en ;
    dct:source <https://www.iso.org/standard/75281.html> ;
    rdfs:isDefinedBy dpvo-risk: ;
    rdfs:subClassOf dpvo:Detriment ;
    sw:term_status "accepted"@en .

dpvo-risk:Toxicological a owl:NamedIndividual,
        dpvo-risk:QuantitativeRiskAssessmentTechnique ;
    rdfs:label "Toxicological Risk Assessment"@en ;
    dct:created "2022-08-18"^^xsd:date ;
    dct:creator "Harshvardhan J. Pandit"^^xsd:string ;
    dct:description "A series of steps taken to obtain a measure for the risk to humans or ecological systems due to exposure to chemicals."@en ;
    dct:source <https://www.iso.org/standard/72140.html> ;
    rdfs:isDefinedBy dpvo-risk: ;
    sw:term_status "accepted"@en .

dpvo-risk:UnauthorisedAccesstoPremises a owl:Class ;
    rdfs:label "Unauthorised Access to Premises"@en ;
    dct:created "2022-08-17"^^xsd:date ;
    dct:creator "Harshvardhan J. Pandit"^^xsd:string ;
    dct:description ""@en ;
    dct:source <https://www.iso.org/standard/75281.html> ;
    rdfs:isDefinedBy dpvo-risk: ;
    rdfs:subClassOf dpvo:Detriment ;
    sw:term_status "accepted"@en .

dpvo-risk:UnauthorisedCodeAccess a owl:Class ;
    rdfs:label "Unauthorised Code Access"@en ;
    dct:created "2022-08-17"^^xsd:date ;
    dct:creator "Harshvardhan J. Pandit"^^xsd:string ;
    dct:description ""@en ;
    dct:source <https://www.enisa.europa.eu/publications/methodology-for-a-sectoral-cybersecurity-assessment> ;
    rdfs:isDefinedBy dpvo-risk: ;
    rdfs:subClassOf dpvo:Detriment ;
    sw:term_status "accepted"@en .

dpvo-risk:UnauthorisedCodeDisclosure a owl:Class ;
    rdfs:label "Unauthorised Code Disclosure"@en ;
    dct:created "2022-08-17"^^xsd:date ;
    dct:creator "Harshvardhan J. Pandit"^^xsd:string ;
    dct:description ""@en ;
    dct:source <https://www.enisa.europa.eu/publications/methodology-for-a-sectoral-cybersecurity-assessment> ;
    rdfs:isDefinedBy dpvo-risk: ;
    rdfs:subClassOf dpvo:Detriment ;
    sw:term_status "accepted"@en .

dpvo-risk:UnauthorisedCodeModification a owl:Class ;
    rdfs:label "Unauthorised Code Modification"@en ;
    dct:created "2022-08-17"^^xsd:date ;
    dct:creator "Harshvardhan J. Pandit"^^xsd:string ;
    dct:description ""@en ;
    dct:source <https://www.enisa.europa.eu/publications/methodology-for-a-sectoral-cybersecurity-assessment> ;
    rdfs:isDefinedBy dpvo-risk: ;
    rdfs:subClassOf dpvo:Damage ;
    sw:term_status "accepted"@en .

dpvo-risk:UnauthorisedDataAccess a owl:Class ;
    rdfs:label "Unauthorised Data Access"@en ;
    dct:created "2022-08-17"^^xsd:date ;
    dct:creator "Harshvardhan J. Pandit"^^xsd:string ;
    dct:description ""@en ;
    dct:source <https://www.enisa.europa.eu/publications/reference-incident-classification-taxonomy/> ;
    rdfs:isDefinedBy dpvo-risk: ;
    rdfs:subClassOf dpvo:Detriment ;
    sw:term_status "accepted"@en .

dpvo-risk:UnauthorisedDataDisclosure a owl:Class ;
    rdfs:label "Unauthorised Data Disclosure"@en ;
    dct:created "2022-08-17"^^xsd:date ;
    dct:creator "Harshvardhan J. Pandit"^^xsd:string ;
    dct:description ""@en ;
    dct:source <https://www.iso.org/standard/75281.html> ;
    rdfs:isDefinedBy dpvo-risk: ;
    rdfs:subClassOf dpvo:Detriment ;
    sw:term_status "accepted"@en .

dpvo-risk:UnauthorisedDataModification a owl:Class ;
    rdfs:label "Unauthorised Data Modification"@en ;
    dct:created "2022-08-17"^^xsd:date ;
    dct:creator "Harshvardhan J. Pandit"^^xsd:string ;
    dct:description ""@en ;
    dct:source <https://www.enisa.europa.eu/publications/reference-incident-classification-taxonomy/> ;
    rdfs:isDefinedBy dpvo-risk: ;
    rdfs:subClassOf dpvo:NonMaterialDamage ;
    sw:term_status "accepted"@en .

dpvo-risk:UnauthorisedImpersonation a owl:Class ;
    rdfs:label "Unauthorised Impersonation"@en ;
    dct:created "2022-08-17"^^xsd:date ;
    dct:creator "Harshvardhan J. Pandit"^^xsd:string ;
    dct:description ""@en ;
    dct:source <https://www.iso.org/standard/75281.html> ;
    rdfs:isDefinedBy dpvo-risk: ;
    rdfs:subClassOf dpvo:NonMaterialDamage ;
    sw:term_status "accepted"@en .

dpvo-risk:UnauthorisedInformationDisclosure a owl:Class ;
    rdfs:label "Unauthorised Information Disclosure"@en ;
    dct:created "2022-08-17"^^xsd:date ;
    dct:creator "Harshvardhan J. Pandit"^^xsd:string ;
    dct:description ""@en ;
    dct:source <https://www.enisa.europa.eu/publications/reference-incident-classification-taxonomy/> ;
    rdfs:isDefinedBy dpvo-risk: ;
    rdfs:subClassOf dpvo:Detriment ;
    sw:term_status "accepted"@en .

dpvo-risk:UnauthorisedReIdentification a owl:Class ;
    rdfs:label "Unauthorised Re-Identification"@en ;
    dct:created "2022-08-19"^^xsd:date ;
    dct:creator "Georg P Krog"^^xsd:string ;
    dct:description ""@en ;
    rdfs:isDefinedBy dpvo-risk: ;
    rdfs:subClassOf dpvo:Consequence ;
    sw:term_status "accepted"@en .

dpvo-risk:UnauthorisedResourceUse a owl:Class ;
    rdfs:label "Unauthorised Resource Use"@en ;
    dct:created "2022-08-17"^^xsd:date ;
    dct:creator "Harshvardhan J. Pandit"^^xsd:string ;
    dct:description ""@en ;
    dct:source <https://www.iso.org/standard/75281.html> ;
    rdfs:isDefinedBy dpvo-risk: ;
    rdfs:subClassOf dpvo:Detriment ;
    sw:term_status "accepted"@en .

dpvo-risk:UnauthorisedSystemAccess a owl:Class ;
    rdfs:label "Unauthorised System Access"@en ;
    dct:created "2022-08-17"^^xsd:date ;
    dct:creator "Harshvardhan J. Pandit"^^xsd:string ;
    dct:description ""@en ;
    dct:source <https://www.iso.org/standard/75281.html> ;
    rdfs:isDefinedBy dpvo-risk: ;
    rdfs:subClassOf dpvo:Detriment ;
    sw:term_status "accepted"@en .

dpvo-risk:UnauthorisedSystemModification a owl:Class ;
    rdfs:label "Unauthorised System Modification"@en ;
    dct:created "2022-08-17"^^xsd:date ;
    dct:creator "Harshvardhan J. Pandit"^^xsd:string ;
    dct:description ""@en ;
    dct:source <https://www.enisa.europa.eu/publications/methodology-for-a-sectoral-cybersecurity-assessment> ;
    rdfs:isDefinedBy dpvo-risk: ;
    rdfs:subClassOf dpvo:Damage ;
    sw:term_status "accepted"@en .

dpvo-risk:UnknownVulnerabilityExploited a owl:Class ;
    rdfs:label "Unknown Vulnerability Exploited"@en ;
    dct:created "2022-08-17"^^xsd:date ;
    dct:creator "Harshvardhan J. Pandit"^^xsd:string ;
    dct:description ""@en ;
    dct:source <https://www.enisa.europa.eu/publications/reference-incident-classification-taxonomy/> ;
    rdfs:isDefinedBy dpvo-risk: ;
    rdfs:subClassOf dpvo:Detriment ;
    sw:term_status "accepted"@en .

dpvo-risk:UnwantedCodeDeletion a owl:Class ;
    rdfs:label "Unwanted Code Deletion"@en ;
    dct:created "2022-08-17"^^xsd:date ;
    dct:creator "Harshvardhan J. Pandit"^^xsd:string ;
    dct:description ""@en ;
    dct:source <https://www.enisa.europa.eu/publications/methodology-for-a-sectoral-cybersecurity-assessment> ;
    rdfs:isDefinedBy dpvo-risk: ;
    rdfs:subClassOf dpvo:Damage ;
    sw:term_status "accepted"@en .

dpvo-risk:UnwantedDataDeletion a owl:Class ;
    rdfs:label "Unwanted Data Deletion"@en ;
    dct:created "2022-08-17"^^xsd:date ;
    dct:creator "Harshvardhan J. Pandit"^^xsd:string ;
    dct:description ""@en ;
    dct:source <https://www.iso.org/standard/75281.html> ;
    rdfs:isDefinedBy dpvo-risk: ;
    rdfs:subClassOf dpvo:Damage ;
    sw:term_status "accepted"@en .

dpvo-risk:UnwantedDisclosureData a owl:Class ;
    rdfs:label "Unwanted Disclosure of Data"@en ;
    dct:created "2022-08-17"^^xsd:date ;
    dct:creator "Harshvardhan J. Pandit"^^xsd:string ;
    dct:description ""@en ;
    dct:source <https://www.iso.org/standard/75281.html> ;
    rdfs:isDefinedBy dpvo-risk: ;
    rdfs:subClassOf dpvo:Detriment ;
    sw:term_status "accepted"@en .

dpvo-risk:VaR a owl:NamedIndividual,
        dpvo-risk:QuantitativeRiskAssessmentTechnique ;
    rdfs:label "Value At Risk (VaR)"@en ;
    dct:created "2022-08-18"^^xsd:date ;
    dct:creator "Harshvardhan J. Pandit"^^xsd:string ;
    dct:description "Financial measure of risk that uses an assumed probability distribution of losses in a stable market condition to calculate the value of a loss that might occur with a specified probability within a defined time span."@en ;
    dct:source <https://www.iso.org/standard/72140.html> ;
    rdfs:isDefinedBy dpvo-risk: ;
    sw:term_status "accepted"@en .

dpvo-risk:Vandalism a owl:Class ;
    rdfs:label "Vandalism"@en ;
    dct:created "2022-08-17"^^xsd:date ;
    dct:creator "Harshvardhan J. Pandit"^^xsd:string ;
    dct:description ""@en ;
    dct:source <https://www.enisa.europa.eu/topics/threat-risk-management/threats-and-trends/enisa-threat-landscape/threat-taxonomy/view> ;
    rdfs:isDefinedBy dpvo-risk: ;
    rdfs:subClassOf dpvo:Damage ;
    sw:term_status "accepted"@en .

dpvo-risk:ViolationCodeConduct a owl:Class ;
    rdfs:label "Violation of Code of Conduct"@en ;
    dct:created "2022-08-17"^^xsd:date ;
    dct:creator "Harshvardhan J. Pandit"^^xsd:string ;
    dct:description ""@en ;
    dct:source <https://www.iso.org/standard/75281.html> ;
    rdfs:isDefinedBy dpvo-risk: ;
    rdfs:subClassOf dpvo:Damage ;
    sw:term_status "accepted"@en .

dpvo-risk:ViolationContractualObligations a owl:Class ;
    rdfs:label "Violation of Contractual Obligations"@en ;
    dct:created "2022-08-17"^^xsd:date ;
    dct:creator "Harshvardhan J. Pandit"^^xsd:string ;
    dct:description ""@en ;
    dct:source <https://www.iso.org/standard/75281.html> ;
    rdfs:isDefinedBy dpvo-risk: ;
    rdfs:subClassOf dpvo:Damage ;
    sw:term_status "accepted"@en .

dpvo-risk:ViolationEthicalCode a owl:Class ;
    rdfs:label "Violation of Ethical Code"@en ;
    dct:created "2022-08-17"^^xsd:date ;
    dct:creator "Harshvardhan J. Pandit"^^xsd:string ;
    dct:description ""@en ;
    dct:source <https://www.iso.org/standard/75281.html> ;
    rdfs:isDefinedBy dpvo-risk: ;
    rdfs:subClassOf dpvo:Damage ;
    sw:term_status "accepted"@en .

dpvo-risk:ViolationOfRights a owl:Class ;
    rdfs:label "Violation of Rights"@en ;
    dct:created "2022-08-18"^^xsd:date ;
    dct:creator "Georg P Krog"^^xsd:string,
        "Harshvardhan J. Pandit"^^xsd:string ;
    dct:description ""@en ;
    rdfs:isDefinedBy dpvo-risk: ;
    rdfs:subClassOf dpvo:Harm ;
    sw:term_status "accepted"@en .

dpvo-risk:ViolationRegulatoryObligations a owl:Class ;
    rdfs:label "Violation of Regulatory Obligations"@en ;
    dct:created "2022-08-17"^^xsd:date ;
    dct:creator "Harshvardhan J. Pandit"^^xsd:string ;
    dct:description ""@en ;
    dct:source <https://www.iso.org/standard/75281.html> ;
    rdfs:isDefinedBy dpvo-risk: ;
    rdfs:subClassOf dpvo:Damage ;
    sw:term_status "accepted"@en .

dpvo-risk:ViolationStatutoryObligations a owl:Class ;
    rdfs:label "Violation of Statutory Obligations"@en ;
    dct:created "2022-08-17"^^xsd:date ;
    dct:creator "Harshvardhan J. Pandit"^^xsd:string ;
    dct:description ""@en ;
    dct:source <https://www.iso.org/standard/75281.html> ;
    rdfs:isDefinedBy dpvo-risk: ;
    rdfs:subClassOf dpvo:Damage ;
    sw:term_status "accepted"@en .

dpvo-risk:VulnerabilityCreated a owl:Class ;
    rdfs:label "Vulnerability Created"@en ;
    dct:created "2022-08-17"^^xsd:date ;
    dct:creator "Harshvardhan J. Pandit"^^xsd:string ;
    dct:description ""@en ;
    dct:source <https://www.iso.org/standard/75281.html> ;
    rdfs:isDefinedBy dpvo-risk: ;
    rdfs:subClassOf dpvo:Detriment ;
    sw:term_status "accepted"@en .

dpvo-risk:VulnerabilityExploited a owl:Class ;
    rdfs:label "Vulnerability Exploited"@en ;
    dct:created "2022-08-17"^^xsd:date ;
    dct:creator "Harshvardhan J. Pandit"^^xsd:string ;
    dct:description ""@en ;
    dct:source <https://www.enisa.europa.eu/publications/reference-incident-classification-taxonomy/> ;
    rdfs:isDefinedBy dpvo-risk: ;
    rdfs:subClassOf dpvo:Detriment ;
    sw:term_status "accepted"@en .

dpvo-risk:RiskAssessmentTechnique a owl:Class ;
    rdfs:label "Risk Assessment Technique"@en ;
    dct:created "2022-08-18"^^xsd:date ;
    dct:creator "Harshvardhan J. Pandit"^^xsd:string ;
    dct:description "A technique or method used to analyse and identify risk levels, sources, likelihoods, severities, and other necessary information required to conduct risk management procedures"@en ;
    dct:source <https://www.iso.org/standard/72140.html> ;
    rdfs:isDefinedBy dpvo-risk: ;
    rdfs:subClassOf dpvo:RiskManagementProcedure ;
    sw:term_status "accepted"@en .

dpvo-risk:3LikelihoodLevels a owl:Class ;
    rdfs:label "3 Likelihood Levels"@en ;
    dct:created "2022-08-18"^^xsd:date ;
    dct:creator "Harshvardhan J. Pandit"^^xsd:string ;
    dct:description "Scale with 3 Likelihood Levels from High to Low"@en ;
    rdfs:isDefinedBy dpvo-risk: ;
    rdfs:subClassOf dpvo:Likelihood ;
    sw:term_status "accepted"@en .

dpvo-risk:3RiskLevels a owl:Class ;
    rdfs:label "3 Risk Levels"@en ;
    dct:created "2022-08-18"^^xsd:date ;
    dct:creator "Harshvardhan J. Pandit"^^xsd:string ;
    dct:description "Scale with 3 Risk Levels from High to Low"@en ;
    rdfs:isDefinedBy dpvo-risk: ;
    rdfs:subClassOf dpvo:RiskLevel ;
    sw:term_status "accepted"@en .

dpvo-risk:3SeverityLevels a owl:Class ;
    rdfs:label "3 Severity Levels"@en ;
    dct:created "2022-08-18"^^xsd:date ;
    dct:creator "Harshvardhan J. Pandit"^^xsd:string ;
    dct:description "Scale with 3 Severity Levels from High to Low"@en ;
    rdfs:isDefinedBy dpvo-risk: ;
    rdfs:subClassOf dpvo:Severity ;
    sw:term_status "accepted"@en .

dpvo-risk:ControlRiskSource a owl:Class ;
    rdfs:label "Control Risk Source"@en ;
    dct:created "2022-08-18"^^xsd:date ;
    dct:creator "Harshvardhan J. Pandit"^^xsd:string ;
    dct:description "Risk Mitigation Measure that controls the Risk Source"@en ;
    rdfs:isDefinedBy dpvo-risk: ;
    rdfs:subClassOf dpvo:RiskMitigationMeasure ;
    sw:term_status "accepted"@en .

dpvo-risk:RiskMatrix a owl:NamedIndividual,
        dpvo-risk:QualitativeRiskAssessmentTechnique,
        dpvo-risk:QuantitativeRiskAssessmentTechnique ;
    rdfs:label "Risk Matrix"@en ;
    dct:created "2022-08-18"^^xsd:date ;
    dct:creator "Harshvardhan J. Pandit"^^xsd:string ;
    dct:description "Compares individual risks by selecting a consequence/ likelihood pair and displaying them on a matrix with consequence on one axis and likelihood on the other."@en ;
    dct:source <https://www.iso.org/standard/72140.html> ;
    rdfs:isDefinedBy dpvo-risk: ;
    sw:term_status "accepted"@en .

dpvo-risk:ControlConsequence a owl:Class ;
    rdfs:label "Control Consequence"@en ;
    dct:created "2022-08-24"^^xsd:date ;
    dct:creator "Harshvardhan J. Pandit"^^xsd:string ;
    dct:description "Risk Mitigation Measure that controls the Consequences and Impacts"@en ;
    rdfs:isDefinedBy dpvo-risk: ;
    rdfs:subClassOf dpvo:RiskMitigationMeasure ;
    sw:term_status "accepted"@en .

dpvo-risk:5LikelihoodLevels a owl:Class ;
    rdfs:label "5 Likelihood Levels"@en ;
    dct:created "2022-08-18"^^xsd:date ;
    dct:creator "Harshvardhan J. Pandit"^^xsd:string ;
    dct:description "Scale with 5 Likelihood Levels from Very High to Very Low"@en ;
    rdfs:isDefinedBy dpvo-risk: ;
    rdfs:subClassOf dpvo:Likelihood ;
    sw:term_status "accepted"@en .

dpvo-risk:5RiskLevels a owl:Class ;
    rdfs:label "5 Risk Levels"@en ;
    dct:created "2022-08-18"^^xsd:date ;
    dct:creator "Harshvardhan J. Pandit"^^xsd:string ;
    dct:description "Scale with 5 Risk Levels from Very High to Very Low"@en ;
    rdfs:isDefinedBy dpvo-risk: ;
    rdfs:subClassOf dpvo:RiskLevel ;
    sw:term_status "accepted"@en .

dpvo-risk:5SeverityLevels a owl:Class ;
    rdfs:label "5 Severity Levels"@en ;
    dct:created "2022-08-18"^^xsd:date ;
    dct:creator "Harshvardhan J. Pandit"^^xsd:string ;
    dct:description "Scale with 5 Severity Levels from Very High to Very Low"@en ;
    rdfs:isDefinedBy dpvo-risk: ;
    rdfs:subClassOf dpvo:Severity ;
    sw:term_status "accepted"@en .

dpvo-risk:ControlMonitors a owl:Class ;
    rdfs:label "Control Monitors"@en ;
    dct:created "2022-08-30"^^xsd:date ;
    dct:creator "Harshvardhan J. Pandit"^^xsd:string ;
    dct:description "Risk Mitigation Measure that uses controls to monitor events"@en ;
    rdfs:comment "Monitoring can be associated with characteristics such as assessing or detecting whether something is active, operational, performant, effective, has potential to materialise, is materialising, or has already materialised."@en ;
    rdfs:isDefinedBy dpvo-risk: ;
    rdfs:subClassOf dpvo:RiskMitigationMeasure ;
    sw:term_status "accepted"@en .

dpvo-risk:7LikelihoodLevels a owl:Class ;
    rdfs:label "7 Likelihood Levels"@en ;
    dct:created "2022-08-18"^^xsd:date ;
    dct:creator "Harshvardhan J. Pandit"^^xsd:string ;
    dct:description "Scale with 7 Likelihood Levels from Extremely High to Extremely Low"@en ;
    rdfs:isDefinedBy dpvo-risk: ;
    rdfs:subClassOf dpvo:Likelihood ;
    sw:term_status "accepted"@en .

dpvo-risk:7RiskLevels a owl:Class ;
    rdfs:label "7 Risk Levels"@en ;
    dct:created "2022-08-18"^^xsd:date ;
    dct:creator "Harshvardhan J. Pandit"^^xsd:string ;
    dct:description "Scale with 7 Risk Levels from Extremely High to Extremely Low"@en ;
    rdfs:isDefinedBy dpvo-risk: ;
    rdfs:subClassOf dpvo:RiskLevel ;
    sw:term_status "accepted"@en .

dpvo-risk:7SeverityLevels a owl:Class ;
    rdfs:label "7 Severity Levels"@en ;
    dct:created "2022-08-18"^^xsd:date ;
    dct:creator "Harshvardhan J. Pandit"^^xsd:string ;
    dct:description "Scale with 7 Severity Levels from Extremely High to Extremely Low"@en ;
    rdfs:isDefinedBy dpvo-risk: ;
    rdfs:subClassOf dpvo:Severity ;
    sw:term_status "accepted"@en .

dpvo-risk:ExtremelyHighLikelihood a owl:NamedIndividual,
        dpvo:Likelihood,
        dpvo-risk:7LikelihoodLevels ;
    rdfs:label "Extremely High Likelihood"@en ;
    dct:created "2022-08-18"^^xsd:date ;
    dct:creator "Harshvardhan J. Pandit"^^xsd:string ;
    dct:description "Level where Likelihood is Extremely High"@en ;
    rdf:value 0.99 ;
    rdfs:comment "The suggested quantitative value for this concept is 0.99 on a scale of 0 to 1"@en ;
    rdfs:isDefinedBy dpvo-risk: ;
    sw:term_status "accepted"@en .

dpvo-risk:ExtremelyHighRisk a owl:NamedIndividual,
        dpvo:RiskLevel,
        dpvo-risk:7RiskLevels ;
    rdfs:label "Extremely High Risk"@en ;
    dct:created "2022-08-18"^^xsd:date ;
    dct:creator "Harshvardhan J. Pandit"^^xsd:string ;
    dct:description "Level where Risk is Extremely High"@en ;
    rdf:value 0.99 ;
    rdfs:comment "The suggested quantitative value for this concept is 0.99 on a scale of 0 to 1"@en ;
    rdfs:isDefinedBy dpvo-risk: ;
    sw:term_status "accepted"@en .

dpvo-risk:ExtremelyHighSeverity a owl:NamedIndividual,
        dpvo:Severity,
        dpvo-risk:7SeverityLevels ;
    rdfs:label "Extremely High Severity"@en ;
    dct:created "2022-08-18"^^xsd:date ;
    dct:creator "Harshvardhan J. Pandit"^^xsd:string ;
    dct:description "Level where Severity is Extremely High"@en ;
    rdf:value 0.99 ;
    rdfs:comment "The suggested quantitative value for this concept is 0.99 on a scale of 0 to 1"@en ;
    rdfs:isDefinedBy dpvo-risk: ;
    sw:term_status "accepted"@en .

dpvo-risk:ExtremelyLowLikelihood a owl:NamedIndividual,
        dpvo:Likelihood,
        dpvo-risk:7LikelihoodLevels ;
    rdfs:label "Extremely Low Likelihood"@en ;
    dct:created "2022-08-18"^^xsd:date ;
    dct:creator "Harshvardhan J. Pandit"^^xsd:string ;
    dct:description "Level where Likelihood is Extremely Low"@en ;
    rdf:value 0.01 ;
    rdfs:comment "The suggested quantitative value for this concept is 0.01 on a scale of 0 to 1"@en ;
    rdfs:isDefinedBy dpvo-risk: ;
    sw:term_status "accepted"@en .

dpvo-risk:ExtremelyLowRisk a owl:NamedIndividual,
        dpvo:RiskLevel,
        dpvo-risk:7RiskLevels ;
    rdfs:label "Extremely Low Risk"@en ;
    dct:created "2022-08-18"^^xsd:date ;
    dct:creator "Harshvardhan J. Pandit"^^xsd:string ;
    dct:description "Level where Risk is Extremely Low"@en ;
    rdf:value 0.01 ;
    rdfs:comment "The suggested quantitative value for this concept is 0.01 on a scale of 0 to 1"@en ;
    rdfs:isDefinedBy dpvo-risk: ;
    sw:term_status "accepted"@en .

dpvo-risk:ExtremelyLowSeverity a owl:NamedIndividual,
        dpvo:Severity,
        dpvo-risk:7SeverityLevels ;
    rdfs:label "Extremely Low Severity"@en ;
    dct:created "2022-08-18"^^xsd:date ;
    dct:creator "Harshvardhan J. Pandit"^^xsd:string ;
    dct:description "Level where Severity is Extremely Low"@en ;
    rdf:value 0.01 ;
    rdfs:comment "The suggested quantitative value for this concept is 0.01 on a scale of 0 to 1"@en ;
    rdfs:isDefinedBy dpvo-risk: ;
    sw:term_status "accepted"@en .

dpvo-risk:RiskMatrix3x3 a owl:Class ;
    rdfs:label "Risk Matrix 3x3"@en ;
    dct:created "2022-08-17"^^xsd:date ;
    dct:creator "Harshvardhan J. Pandit"^^xsd:string ;
    dct:description "A Risk Matrix with 3 Likelihood, 3 Severity, and 3 Risk Level types"@en ;
    rdfs:isDefinedBy dpvo-risk: ;
    rdfs:subClassOf dpvo-risk:RiskMatrix ;
    sw:term_status "accepted"@en .

dpvo-risk:VeryHighLikelihood a owl:NamedIndividual,
        dpvo:Likelihood,
        dpvo-risk:5LikelihoodLevels,
        dpvo-risk:7LikelihoodLevels ;
    rdfs:label "Very High Likelihood"@en ;
    dct:created "2022-08-18"^^xsd:date ;
    dct:creator "Harshvardhan J. Pandit"^^xsd:string ;
    dct:description "Level where Likelihood is Very High"@en ;
    rdf:value 0.9 ;
    rdfs:comment "The suggested quantitative value for this concept is 0.9 on a scale of 0 to 1"@en ;
    rdfs:isDefinedBy dpvo-risk: ;
    sw:term_status "accepted"@en .

dpvo-risk:VeryHighRisk a owl:NamedIndividual,
        dpvo:RiskLevel,
        dpvo-risk:5RiskLevels,
        dpvo-risk:7RiskLevels ;
    rdfs:label "Very High Risk"@en ;
    dct:created "2022-08-18"^^xsd:date ;
    dct:creator "Harshvardhan J. Pandit"^^xsd:string ;
    dct:description "Level where Risk is Very High"@en ;
    rdf:value 0.9 ;
    rdfs:comment "The suggested quantitative value for this concept is 0.9 on a scale of 0 to 1"@en ;
    rdfs:isDefinedBy dpvo-risk: ;
    sw:term_status "accepted"@en .

dpvo-risk:VeryHighSeverity a owl:NamedIndividual,
        dpvo:Severity,
        dpvo-risk:5SeverityLevels,
        dpvo-risk:7SeverityLevels ;
    rdfs:label "Very High Severity"@en ;
    dct:created "2022-08-18"^^xsd:date ;
    dct:creator "Harshvardhan J. Pandit"^^xsd:string ;
    dct:description "Level where Severity is Very High"@en ;
    rdf:value 0.9 ;
    rdfs:comment "The suggested quantitative value for this concept is 0.9 on a scale of 0 to 1"@en ;
    rdfs:isDefinedBy dpvo-risk: ;
    sw:term_status "accepted"@en .

dpvo-risk:VeryLowLikelihood a owl:NamedIndividual,
        dpvo:Likelihood,
        dpvo-risk:5LikelihoodLevels,
        dpvo-risk:7LikelihoodLevels ;
    rdfs:label "Very Low Likelihood"@en ;
    dct:created "2022-08-18"^^xsd:date ;
    dct:creator "Harshvardhan J. Pandit"^^xsd:string ;
    dct:description "Level where Likelihood is Very Low"@en ;
    rdf:value 0.1 ;
    rdfs:comment "The suggested quantitative value for this concept is 0.1 on a scale of 0 to 1"@en ;
    rdfs:isDefinedBy dpvo-risk: ;
    sw:term_status "accepted"@en .

dpvo-risk:VeryLowRisk a owl:NamedIndividual,
        dpvo:RiskLevel,
        dpvo-risk:5RiskLevels,
        dpvo-risk:7RiskLevels ;
    rdfs:label "Very Low Risk"@en ;
    dct:created "2022-08-18"^^xsd:date ;
    dct:creator "Harshvardhan J. Pandit"^^xsd:string ;
    dct:description "Level where Risk is Very Low"@en ;
    rdf:value 0.1 ;
    rdfs:comment "The suggested quantitative value for this concept is 0.1 on a scale of 0 to 1"@en ;
    rdfs:isDefinedBy dpvo-risk: ;
    sw:term_status "accepted"@en .

dpvo-risk:VeryLowSeverity a owl:NamedIndividual,
        dpvo:Severity,
        dpvo-risk:5SeverityLevels,
        dpvo-risk:7SeverityLevels ;
    rdfs:label "Very Low Severity"@en ;
    dct:created "2022-08-18"^^xsd:date ;
    dct:creator "Harshvardhan J. Pandit"^^xsd:string ;
    dct:description "Level where Severity is Very Low"@en ;
    rdf:value 0.1 ;
    rdfs:comment "The suggested quantitative value for this concept is 0.1 on a scale of 0 to 1"@en ;
    rdfs:isDefinedBy dpvo-risk: ;
    sw:term_status "accepted"@en .

dpvo-risk:HighLikelihood a owl:NamedIndividual,
        dpvo:Likelihood,
        dpvo-risk:3LikelihoodLevels,
        dpvo-risk:5LikelihoodLevels,
        dpvo-risk:7LikelihoodLevels ;
    rdfs:label "High Likelihood"@en ;
    dct:created "2022-08-18"^^xsd:date ;
    dct:creator "Harshvardhan J. Pandit"^^xsd:string ;
    dct:description "Level where Likelihood is High"@en ;
    rdf:value 0.75 ;
    rdfs:comment "The suggested quantitative value for this concept is 0.75 on a scale of 0 to 1"@en ;
    rdfs:isDefinedBy dpvo-risk: ;
    sw:term_status "accepted"@en .

dpvo-risk:HighRisk a owl:NamedIndividual,
        dpvo:RiskLevel,
        dpvo-risk:3RiskLevels,
        dpvo-risk:5RiskLevels,
        dpvo-risk:7RiskLevels ;
    rdfs:label "High Risk"@en ;
    dct:created "2022-08-18"^^xsd:date ;
    dct:creator "Harshvardhan J. Pandit"^^xsd:string ;
    dct:description "Level where Risk is High"@en ;
    rdf:value 0.75 ;
    rdfs:comment "The suggested quantitative value for this concept is 0.75 on a scale of 0 to 1"@en ;
    rdfs:isDefinedBy dpvo-risk: ;
    sw:term_status "accepted"@en .

dpvo-risk:HighSeverity a owl:NamedIndividual,
        dpvo:Severity,
        dpvo-risk:3SeverityLevels,
        dpvo-risk:5SeverityLevels,
        dpvo-risk:7SeverityLevels ;
    rdfs:label "High Severity"@en ;
    dct:created "2022-08-18"^^xsd:date ;
    dct:creator "Harshvardhan J. Pandit"^^xsd:string ;
    dct:description "Level where Severity is High"@en ;
    rdf:value 0.75 ;
    rdfs:comment "The suggested quantitative value for this concept is 0.75 on a scale of 0 to 1"@en ;
    rdfs:isDefinedBy dpvo-risk: ;
    sw:term_status "accepted"@en .

dpvo-risk:LowLikelihood a owl:NamedIndividual,
        dpvo:Likelihood,
        dpvo-risk:3LikelihoodLevels,
        dpvo-risk:5LikelihoodLevels,
        dpvo-risk:7LikelihoodLevels ;
    rdfs:label "Low Likelihood"@en ;
    dct:created "2022-08-18"^^xsd:date ;
    dct:creator "Harshvardhan J. Pandit"^^xsd:string ;
    dct:description "Level where Likelihood is Low"@en ;
    rdf:value 0.25 ;
    rdfs:comment "The suggested quantitative value for this concept is 0.25 on a scale of 0 to 1"@en ;
    rdfs:isDefinedBy dpvo-risk: ;
    sw:term_status "accepted"@en .

dpvo-risk:LowRisk a owl:NamedIndividual,
        dpvo:RiskLevel,
        dpvo-risk:3RiskLevels,
        dpvo-risk:5RiskLevels,
        dpvo-risk:7RiskLevels ;
    rdfs:label "Low Risk"@en ;
    dct:created "2022-08-18"^^xsd:date ;
    dct:creator "Harshvardhan J. Pandit"^^xsd:string ;
    dct:description "Level where Risk is Low"@en ;
    rdf:value 0.25 ;
    rdfs:comment "The suggested quantitative value for this concept is 0.25 on a scale of 0 to 1"@en ;
    rdfs:isDefinedBy dpvo-risk: ;
    sw:term_status "accepted"@en .

dpvo-risk:LowSeverity a owl:NamedIndividual,
        dpvo:Severity,
        dpvo-risk:3SeverityLevels,
        dpvo-risk:5SeverityLevels,
        dpvo-risk:7SeverityLevels ;
    rdfs:label "Low Severity"@en ;
    dct:created "2022-08-18"^^xsd:date ;
    dct:creator "Harshvardhan J. Pandit"^^xsd:string ;
    dct:description "Level where Severity is Low"@en ;
    rdf:value 0.25 ;
    rdfs:comment "The suggested quantitative value for this concept is 0.25 on a scale of 0 to 1"@en ;
    rdfs:isDefinedBy dpvo-risk: ;
    sw:term_status "accepted"@en .

dpvo-risk:ModerateLikelihood a owl:NamedIndividual,
        dpvo:Likelihood,
        dpvo-risk:3LikelihoodLevels,
        dpvo-risk:5LikelihoodLevels,
        dpvo-risk:7LikelihoodLevels ;
    rdfs:label "Moderate Likelihood"@en ;
    dct:created "2022-08-18"^^xsd:date ;
    dct:creator "Harshvardhan J. Pandit"^^xsd:string ;
    dct:description "Level where Likelihood is Moderate"@en ;
    rdf:value 0.5 ;
    rdfs:comment "The suggested quantitative value for this concept is 0.5 on a scale of 0 to 1"@en ;
    rdfs:isDefinedBy dpvo-risk: ;
    sw:term_status "accepted"@en .

dpvo-risk:ModerateRisk a owl:NamedIndividual,
        dpvo:RiskLevel,
        dpvo-risk:3RiskLevels,
        dpvo-risk:5RiskLevels,
        dpvo-risk:7RiskLevels ;
    rdfs:label "Moderate Risk"@en ;
    dct:created "2022-08-18"^^xsd:date ;
    dct:creator "Harshvardhan J. Pandit"^^xsd:string ;
    dct:description "Level where Risk is Moderate"@en ;
    rdf:value 0.5 ;
    rdfs:comment "The suggested quantitative value for this concept is 0.5 on a scale of 0 to 1"@en ;
    rdfs:isDefinedBy dpvo-risk: ;
    sw:term_status "accepted"@en .

dpvo-risk:ModerateSeverity a owl:NamedIndividual,
        dpvo:Severity,
        dpvo-risk:3SeverityLevels,
        dpvo-risk:5SeverityLevels,
        dpvo-risk:7SeverityLevels ;
    rdfs:label "Moderate Severity"@en ;
    dct:created "2022-08-18"^^xsd:date ;
    dct:creator "Harshvardhan J. Pandit"^^xsd:string ;
    dct:description "Level where Severity is Moderate"@en ;
    rdf:value 0.5 ;
    rdfs:comment "The suggested quantitative value for this concept is 0.5 on a scale of 0 to 1"@en ;
    rdfs:isDefinedBy dpvo-risk: ;
    sw:term_status "accepted"@en .

dpvo-risk:RiskMatrix5x5 a owl:Class ;
    rdfs:label "Risk Matrix 5x5"@en ;
    dct:created "2022-08-17"^^xsd:date ;
    dct:creator "Harshvardhan J. Pandit"^^xsd:string ;
    dct:description "A Risk Matrix with 5 Likelihood, 5 Severity, and 5 Risk Level types"@en ;
    rdfs:isDefinedBy dpvo-risk: ;
    rdfs:subClassOf dpvo-risk:RiskMatrix ;
    sw:term_status "accepted"@en .

dpvo-risk:QuantitativeRiskAssessmentTechnique a owl:Class ;
    rdfs:label "Quantitative Risk Assessment Technique"@en ;
    dct:created "2022-08-18"^^xsd:date ;
    dct:creator "Harshvardhan J. Pandit"^^xsd:string ;
    dct:description "A risk assessment technique that uses quantitative methods"@en ;
    dct:source <https://www.iso.org/standard/72140.html> ;
    rdfs:isDefinedBy dpvo-risk: ;
    rdfs:subClassOf dpvo-risk:RiskAssessmentTechnique ;
    sw:term_status "accepted"@en .

dpvo-risk:QualitativeRiskAssessmentTechnique a owl:Class ;
    rdfs:label "Qualitative Risk Assessment Technique"@en ;
    dct:created "2022-08-18"^^xsd:date ;
    dct:creator "Harshvardhan J. Pandit"^^xsd:string ;
    dct:description "A risk assessment technique that uses qualitative methods"@en ;
    dct:source <https://www.iso.org/standard/72140.html> ;
    rdfs:isDefinedBy dpvo-risk: ;
    rdfs:subClassOf dpvo-risk:RiskAssessmentTechnique ;
    sw:term_status "accepted"@en .

dpvo-risk:RiskManagementMethodology a owl:Class ;
    rdfs:label "Risk Management Methodology"@en ;
    dct:created "2022-08-18"^^xsd:date ;
    dct:creator "Harshvardhan J. Pandit"^^xsd:string ;
    dct:description "A risk management framework or methodology addresses the main functional components related to identification, assessment, treatment, and monitoring regarding risks"@en ;
    dct:source <https://www.enisa.europa.eu/publications/compendium-of-risk-management-frameworks> ;
    rdfs:isDefinedBy dpvo-risk: ;
    rdfs:subClassOf dpvo:RiskManagementProcedure ;
    sw:term_status "accepted"@en .

dpvo-risk:RiskMatrix7x7 a owl:Class ;
    rdfs:label "Risk Matrix 7x7"@en ;
    dct:created "2022-08-17"^^xsd:date ;
    dct:creator "Harshvardhan J. Pandit"^^xsd:string ;
    dct:description "A Risk Matrix with 7 Likelihood, 7 Severity, and 7 Risk Level types"@en ;
    rdfs:isDefinedBy dpvo-risk: ;
    rdfs:subClassOf dpvo-risk:RiskMatrix ;
    sw:term_status "accepted"@en .

